move to typeclass assumptions

src/Std/Data/ExtDHashMap/Basic.lean
@@ -24,7 +24,7 @@ universe u v w
 
 variable {α : Type u} {β : α → Type v} {γ : α → Type w}
 
-variable {_ : BEq α} {_ : Hashable α} {_ : EquivBEq α} {_ : LawfulHashable α}
+variable {_ : BEq α} {_ : Hashable α}
 
 open scoped Std.DHashMap
 
@@ -56,40 +56,45 @@ be used in nested inductive types. For these use cases, `Std.DHashMap.Raw` and
 `Std.DHashMap.Raw.WF` unbundle the invariant from the hash map. When in doubt, prefer
 `DHashMap` over `DHashMap.Raw`.
 -/
-def ExtDHashMap (α : Type u) (β : α → Type v) [BEq α] [Hashable α] [EquivBEq α] [LawfulHashable α] :=
+def ExtDHashMap (α : Type u) (β : α → Type v) [BEq α] [Hashable α] :=
   Quotient (DHashMap.isSetoid α β)
 
 namespace ExtDHashMap
 
 @[inline, inherit_doc DHashMap.emptyWithCapacity]
-def emptyWithCapacity [BEq α] [Hashable α] [EquivBEq α] [LawfulHashable α]
+def emptyWithCapacity [BEq α] [Hashable α]
     (capacity := 8) : ExtDHashMap α β :=
   Quotient.mk' (DHashMap.emptyWithCapacity capacity)
 
-instance [BEq α] [Hashable α] [EquivBEq α] [LawfulHashable α] : EmptyCollection (ExtDHashMap α β) where
+instance [BEq α] [Hashable α] : EmptyCollection (ExtDHashMap α β) where
   emptyCollection := emptyWithCapacity
 
-instance [BEq α] [Hashable α] [EquivBEq α] [LawfulHashable α] : Inhabited (DHashMap α β) where
+instance [BEq α] [Hashable α] : Inhabited (DHashMap α β) where
   default := ∅
 
-@[inline, inherit_doc DHashMap.insert] def insert (m : ExtDHashMap α β) (a : α)
+@[inline, inherit_doc DHashMap.insert]
+def insert [EquivBEq α] [LawfulHashable α] (m : ExtDHashMap α β) (a : α)
     (b : β a) : ExtDHashMap α β :=
   m.lift (fun m => Quotient.mk' (m.insert a b))
     (fun m m' (h : m ~m m') => Quotient.sound (h.insert a b))
 
-instance : Singleton ((a : α) × β a) (ExtDHashMap α β) := ⟨fun ⟨a, b⟩ => (∅ : ExtDHashMap α β).insert a b⟩
+instance [EquivBEq α] [LawfulHashable α] : Singleton ((a : α) × β a) (ExtDHashMap α β) where
+  singleton | ⟨a, b⟩ => (∅ : ExtDHashMap α β).insert a b
 
-instance : Insert ((a : α) × β a) (ExtDHashMap α β) := ⟨fun ⟨a, b⟩ s => s.insert a b⟩
+instance [EquivBEq α] [LawfulHashable α] : Insert ((a : α) × β a) (ExtDHashMap α β) where
+  insert | ⟨a, b⟩, s => s.insert a b
 
-instance : LawfulSingleton ((a : α) × β a) (ExtDHashMap α β) :=
+instance [EquivBEq α] [LawfulHashable α] : LawfulSingleton ((a : α) × β a) (ExtDHashMap α β) :=
   ⟨fun _ => rfl⟩
 
-@[inline, inherit_doc DHashMap.insertIfNew] def insertIfNew (m : ExtDHashMap α β)
+@[inline, inherit_doc DHashMap.insertIfNew]
+def insertIfNew [EquivBEq α] [LawfulHashable α] (m : ExtDHashMap α β)
     (a : α) (b : β a) : ExtDHashMap α β :=
   m.lift (fun m => Quotient.mk' (m.insertIfNew a b))
     (fun m m' (h : m ~m m') => Quotient.sound (h.insertIfNew a b))
 
-@[inline, inherit_doc DHashMap.containsThenInsert] def containsThenInsert
+@[inline, inherit_doc DHashMap.containsThenInsert]
+def containsThenInsert [EquivBEq α] [LawfulHashable α]
     (m : ExtDHashMap α β) (a : α) (b : β a) : Bool × ExtDHashMap α β :=
   m.lift (fun m => let m' := m.containsThenInsert a b; ⟨m'.1, Quotient.mk' m'.2⟩)
     (fun m m' (h : m ~m m') =>
@@ -98,7 +103,8 @@ instance : LawfulSingleton ((a : α) × β a) (ExtDHashMap α β) :=
         (Quotient.sound <|
           m.containsThenInsert_snd.symm ▸ m'.containsThenInsert_snd.symm ▸ h.insert a b))
 
-@[inline, inherit_doc DHashMap.containsThenInsertIfNew] def containsThenInsertIfNew
+@[inline, inherit_doc DHashMap.containsThenInsertIfNew]
+def containsThenInsertIfNew [EquivBEq α] [LawfulHashable α]
     (m : ExtDHashMap α β) (a : α) (b : β a) : Bool × ExtDHashMap α β :=
   m.lift (fun m => let m' := m.containsThenInsertIfNew a b; ⟨m'.1, Quotient.mk' m'.2⟩)
     (fun m m' (h : m ~m m') =>
@@ -107,7 +113,8 @@ instance : LawfulSingleton ((a : α) × β a) (ExtDHashMap α β) :=
         (Quotient.sound <|
           m.containsThenInsertIfNew_snd.symm ▸ m'.containsThenInsertIfNew_snd.symm ▸ h.insertIfNew a b))
 
-@[inline, inherit_doc DHashMap.getThenInsertIfNew?] def getThenInsertIfNew? [LawfulBEq α]
+@[inline, inherit_doc DHashMap.getThenInsertIfNew?]
+def getThenInsertIfNew? [LawfulBEq α]
     (m : ExtDHashMap α β) (a : α) (b : β a) : Option (β a) × ExtDHashMap α β :=
   m.lift (fun m => let m' := m.getThenInsertIfNew? a b; ⟨m'.1, Quotient.mk' m'.2⟩)
     (fun m m' (h : m ~m m') =>
@@ -116,34 +123,40 @@ instance : LawfulSingleton ((a : α) × β a) (ExtDHashMap α β) :=
         (Quotient.sound <|
           m.getThenInsertIfNew?_snd.symm ▸ m'.getThenInsertIfNew?_snd.symm ▸ h.insertIfNew a b))
 
-@[inline, inherit_doc DHashMap.get?] def get? [LawfulBEq α] (m : ExtDHashMap α β)
+@[inline, inherit_doc DHashMap.get?]
+def get? [LawfulBEq α] (m : ExtDHashMap α β)
     (a : α) : Option (β a) :=
   m.lift (fun m => m.get? a) (fun m m' (h : m ~m m') => h.get?_eq)
 
-@[inline, inherit_doc DHashMap.contains] def contains (m : ExtDHashMap α β) (a : α) :
+@[inline, inherit_doc DHashMap.contains]
+def contains [EquivBEq α] [LawfulHashable α] (m : ExtDHashMap α β) (a : α) :
     Bool :=
   m.lift (fun m => m.contains a) (fun m m' (h : m ~m m') => h.contains_eq)
 
-instance : Membership α (ExtDHashMap α β) where
+instance [EquivBEq α] [LawfulHashable α] : Membership α (ExtDHashMap α β) where
   mem m a := m.contains a
 
-instance {m : ExtDHashMap α β} {a : α} : Decidable (a ∈ m) :=
+instance [EquivBEq α] [LawfulHashable α] {m : ExtDHashMap α β} {a : α} : Decidable (a ∈ m) :=
   inferInstanceAs <| Decidable (m.contains a)
 
-@[inline, inherit_doc DHashMap.get] def get [LawfulBEq α] (m : ExtDHashMap α β) (a : α)
+@[inline, inherit_doc DHashMap.get]
+def get [LawfulBEq α] (m : ExtDHashMap α β) (a : α)
     (h : a ∈ m) : β a :=
   m.pliftOn (fun m h' => m.get a (h' ▸ h :))
     (fun m m' _ _ (h : m ~m m') => h.get_eq _)
 
-@[inline, inherit_doc DHashMap.get!] def get! [LawfulBEq α] (m : ExtDHashMap α β)
+@[inline, inherit_doc DHashMap.get!]
+def get! [LawfulBEq α] (m : ExtDHashMap α β)
     (a : α) [Inhabited (β a)] : β a :=
   m.lift (fun m => m.get! a) (fun m m' (h : m ~m m') => h.get!_eq)
 
-@[inline, inherit_doc DHashMap.getD] def getD [LawfulBEq α] (m : ExtDHashMap α β)
+@[inline, inherit_doc DHashMap.getD]
+def getD [LawfulBEq α] (m : ExtDHashMap α β)
     (a : α) (fallback : β a) : β a :=
   m.lift (fun m => m.getD a fallback) (fun m m' (h : m ~m m') => h.getD_eq)
 
-@[inline, inherit_doc DHashMap.erase] def erase (m : ExtDHashMap α β) (a : α) :
+@[inline, inherit_doc DHashMap.erase]
+def erase [EquivBEq α] [LawfulHashable α] (m : ExtDHashMap α β) (a : α) :
     ExtDHashMap α β :=
   m.lift (fun m => Quotient.mk' (m.erase a))
     (fun m m' (h : m ~m m') => Quotient.sound (h.erase a))
@@ -152,27 +165,32 @@ namespace Const
 
 variable {β : Type v}
 
-@[inline, inherit_doc DHashMap.Const.get?] def get?
+@[inline, inherit_doc DHashMap.Const.get?]
+def get? [EquivBEq α] [LawfulHashable α]
     (m : ExtDHashMap α (fun _ => β)) (a : α) : Option β :=
   m.lift (fun m => DHashMap.Const.get? m a)
     (fun m m' (h : m ~m m') => h.constGet?_eq)
 
-@[inline, inherit_doc DHashMap.Const.get] def get
+@[inline, inherit_doc DHashMap.Const.get]
+def get [EquivBEq α] [LawfulHashable α]
     (m : ExtDHashMap α (fun _ => β)) (a : α) (h : a ∈ m) : β :=
   m.pliftOn (fun m h' => DHashMap.Const.get m a (h' ▸ h :))
     (fun m m' _ _ (h : m ~m m') => h.constGet_eq _)
 
-@[inline, inherit_doc DHashMap.Const.getD] def getD
+@[inline, inherit_doc DHashMap.Const.getD]
+def getD [EquivBEq α] [LawfulHashable α]
     (m : ExtDHashMap α (fun _ => β)) (a : α) (fallback : β) : β :=
   m.lift (fun m => DHashMap.Const.getD m a fallback)
     (fun m m' (h : m ~m m') => h.constGetD_eq)
 
-@[inline, inherit_doc DHashMap.Const.get!] def get! [Inhabited β]
+@[inline, inherit_doc DHashMap.Const.get!]
+def get! [EquivBEq α] [LawfulHashable α] [Inhabited β]
     (m : ExtDHashMap α (fun _ => β)) (a : α) : β :=
   m.lift (fun m => DHashMap.Const.get! m a)
     (fun m m' (h : m ~m m') => h.constGet!_eq)
 
-@[inline, inherit_doc DHashMap.Const.getThenInsertIfNew?] def getThenInsertIfNew?
+@[inline, inherit_doc DHashMap.Const.getThenInsertIfNew?]
+def getThenInsertIfNew? [EquivBEq α] [LawfulHashable α]
     (m : ExtDHashMap α (fun _ => β)) (a : α) (b : β) :
     Option β × ExtDHashMap α (fun _ => β) :=
   m.lift (fun m =>
@@ -188,59 +206,72 @@ variable {β : Type v}
 
 end Const
 
-@[inline, inherit_doc DHashMap.getKey?] def getKey? (m : ExtDHashMap α β) (a : α) : Option α :=
+@[inline, inherit_doc DHashMap.getKey?]
+def getKey? [EquivBEq α] [LawfulHashable α] (m : ExtDHashMap α β) (a : α) : Option α :=
   m.lift (fun m => m.getKey? a) (fun m m' (h : m ~m m') => h.getKey?_eq)
 
-@[inline, inherit_doc DHashMap.getKey] def getKey (m : ExtDHashMap α β) (a : α) (h : a ∈ m) : α :=
+@[inline, inherit_doc DHashMap.getKey]
+def getKey [EquivBEq α] [LawfulHashable α] (m : ExtDHashMap α β) (a : α) (h : a ∈ m) : α :=
   m.pliftOn (fun m h' => m.getKey a (h' ▸ h :))
     (fun m m' _ _ (h : m ~m m') => h.getKey_eq _)
 
-@[inline, inherit_doc DHashMap.getKey!] def getKey! [Inhabited α] (m : ExtDHashMap α β) (a : α) : α :=
+@[inline, inherit_doc DHashMap.getKey!]
+def getKey! [EquivBEq α] [LawfulHashable α] [Inhabited α] (m : ExtDHashMap α β) (a : α) : α :=
   m.lift (fun m => m.getKey! a) (fun m m' (h : m ~m m') => h.getKey!_eq)
 
-@[inline, inherit_doc DHashMap.getKeyD] def getKeyD (m : ExtDHashMap α β) (a : α) (fallback : α) : α :=
+@[inline, inherit_doc DHashMap.getKeyD]
+def getKeyD [EquivBEq α] [LawfulHashable α] (m : ExtDHashMap α β) (a : α) (fallback : α) : α :=
   m.lift (fun m => m.getKeyD a fallback)
     (fun m m' (h : m ~m m') => h.getKeyD_eq)
 
-@[inline, inherit_doc DHashMap.size] def size (m : ExtDHashMap α β) : Nat :=
+@[inline, inherit_doc DHashMap.size]
+def size [EquivBEq α] [LawfulHashable α] (m : ExtDHashMap α β) : Nat :=
   m.lift (fun m => m.size) (fun m m' (h : m ~m m') => h.size_eq)
 
-@[inline, inherit_doc DHashMap.isEmpty] def isEmpty (m : ExtDHashMap α β) : Bool :=
+@[inline, inherit_doc DHashMap.isEmpty]
+def isEmpty [EquivBEq α] [LawfulHashable α] (m : ExtDHashMap α β) : Bool :=
   m.lift (fun m => m.isEmpty) (fun m m' (h : m ~m m') => h.isEmpty_eq)
 
 -- TODO: add fold similar to `Finset.fold`
 
-@[inline, inherit_doc DHashMap.filter] def filter (f : (a : α) → β a → Bool)
+@[inline, inherit_doc DHashMap.filter]
+def filter [EquivBEq α] [LawfulHashable α] (f : (a : α) → β a → Bool)
     (m : ExtDHashMap α β) : ExtDHashMap α β :=
   m.lift (fun m => Quotient.mk' (m.filter f))
     (fun m m' (h : m ~m m') => Quotient.sound (h.filter f))
 
-@[inline, inherit_doc DHashMap.map] def map (f : (a : α) → β a → γ a)
+@[inline, inherit_doc DHashMap.map]
+def map [EquivBEq α] [LawfulHashable α] (f : (a : α) → β a → γ a)
     (m : ExtDHashMap α β) : ExtDHashMap α γ :=
   m.lift (fun m => Quotient.mk' (m.map f))
     (fun m m' (h : m ~m m') => Quotient.sound (h.map f))
 
-@[inline, inherit_doc DHashMap.filterMap] def filterMap (f : (a : α) → β a → Option (γ a))
+@[inline, inherit_doc DHashMap.filterMap]
+def filterMap [EquivBEq α] [LawfulHashable α] (f : (a : α) → β a → Option (γ a))
     (m : ExtDHashMap α β) : ExtDHashMap α γ :=
   m.lift (fun m => Quotient.mk' (m.filterMap f))
     (fun m m' (h : m ~m m') => Quotient.sound (h.filterMap f))
 
-@[inline, inherit_doc DHashMap.modify] def modify [LawfulBEq α] (m : ExtDHashMap α β)
+@[inline, inherit_doc DHashMap.modify]
+def modify [LawfulBEq α] (m : ExtDHashMap α β)
     (a : α) (f : β a → β a) : ExtDHashMap α β :=
   m.lift (fun m => Quotient.mk' (m.modify a f))
     (fun m m' (h : m ~m m') => Quotient.sound (h.modify a f))
 
-@[inline, inherit_doc DHashMap.modify] def Const.modify {β : Type v} (m : ExtDHashMap α (fun _ => β))
+@[inline, inherit_doc DHashMap.Const.modify]
+def Const.modify [EquivBEq α] [LawfulHashable α] {β : Type v} (m : ExtDHashMap α (fun _ => β))
     (a : α) (f : β → β) : ExtDHashMap α (fun _ => β) :=
   m.lift (fun m => Quotient.mk' (DHashMap.Const.modify m a f))
     (fun m m' (h : m ~m m') => Quotient.sound (h.constModify a f))
 
-@[inline, inherit_doc DHashMap.alter] def alter [LawfulBEq α] (m : ExtDHashMap α β)
+@[inline, inherit_doc DHashMap.alter]
+def alter [LawfulBEq α] (m : ExtDHashMap α β)
     (a : α) (f : Option (β a) → Option (β a)) : ExtDHashMap α β :=
   m.lift (fun m => Quotient.mk' (m.alter a f))
     (fun m m' (h : m ~m m') => Quotient.sound (h.alter a f))
 
-@[inline, inherit_doc DHashMap.alter] def Const.alter {β : Type v} (m : ExtDHashMap α (fun _ => β))
+@[inline, inherit_doc DHashMap.Const.alter]
+def Const.alter [EquivBEq α] [LawfulHashable α] {β : Type v} (m : ExtDHashMap α (fun _ => β))
     (a : α) (f : Option β → Option β) : ExtDHashMap α (fun _ => β) :=
   m.lift (fun m => Quotient.mk' (DHashMap.Const.alter m a f))
     (fun m m' (h : m ~m m') => Quotient.sound (h.constAlter a f))
@@ -250,7 +281,8 @@ Note: We can't use the existing functions because weird (noncomputable) `ForIn` 
 can break congruence. The subtype is still used to provide the `insertMany_ind` theorem.
 -/
 
-@[inline, inherit_doc DHashMap.insertMany] def insertMany {ρ : Type w}
+@[inline, inherit_doc DHashMap.insertMany]
+def insertMany [EquivBEq α] [LawfulHashable α] {ρ : Type w}
     [ForIn Id ρ ((a : α) × β a)] (m : ExtDHashMap α β) (l : ρ) : ExtDHashMap α β := Id.run do
   let mut m : { x // ∀ P : ExtDHashMap α β → Prop,
     P m → (∀ {m a b}, P m → P (m.insert a b)) → P x } := ⟨m, fun _ h _ => h⟩
@@ -258,7 +290,8 @@ can break congruence. The subtype is still used to provide the `insertMany_ind` 
     m := ⟨m.1.insert a b, fun _ init step => step (m.2 _ init step)⟩
   return m.1
 
-@[inline, inherit_doc DHashMap.Const.insertMany] def Const.insertMany {β : Type v} {ρ : Type w}
+@[inline, inherit_doc DHashMap.Const.insertMany]
+def Const.insertMany [EquivBEq α] [LawfulHashable α] {β : Type v} {ρ : Type w}
     [ForIn Id ρ (α × β)] (m : ExtDHashMap α (fun _ => β))
     (l : ρ) : ExtDHashMap α (fun _ => β) := Id.run do
   let mut m : { x // ∀ P : ExtDHashMap α (fun _ => β) → Prop,
@@ -267,7 +300,8 @@ can break congruence. The subtype is still used to provide the `insertMany_ind` 
     m := ⟨m.1.insert a b, fun _ init step => step (m.2 _ init step)⟩
   return m.1
 
-@[inline, inherit_doc DHashMap.Const.insertManyIfNewUnit] def Const.insertManyIfNewUnit {ρ : Type w}
+@[inline, inherit_doc DHashMap.Const.insertManyIfNewUnit]
+def Const.insertManyIfNewUnit [EquivBEq α] [LawfulHashable α] {ρ : Type w}
     [ForIn Id ρ α] (m : ExtDHashMap α (fun _ => Unit))
     (l : ρ) : ExtDHashMap α (fun _ => Unit) := Id.run do
   let mut m : { x // ∀ P : ExtDHashMap α (fun _ => Unit) → Prop,
@@ -278,24 +312,25 @@ can break congruence. The subtype is still used to provide the `insertMany_ind` 
 
 -- TODO (after verification): partition, union
 
-/-
-Note: we could use `ofList` here but we want the connection of `ofList` and `insertMany`.
--/
-
-@[inline, inherit_doc DHashMap.ofList] def ofList
-    [BEq α] [Hashable α] [EquivBEq α] [LawfulHashable α] (l : List ((a : α) × β a)) :
-    ExtDHashMap α β :=
-  insertMany ∅ l
-
-@[inline, inherit_doc DHashMap.Const.ofList] def Const.ofList {β : Type v}
-    [BEq α] [Hashable α] [EquivBEq α] [LawfulHashable α] (l : List (α × β)) :
-    ExtDHashMap α (fun _ => β) :=
-  Const.insertMany ∅ l
-
-@[inline, inherit_doc DHashMap.Const.unitOfList] def Const.unitOfList
-    [BEq α] [Hashable α] [EquivBEq α] [LawfulHashable α] (l : List α) :
+@[inline, inherit_doc DHashMap.Const.unitOfArray]
+def Const.unitOfArray [BEq α] [Hashable α] (l : Array α) :
     ExtDHashMap α (fun _ => Unit) :=
-  Const.insertManyIfNewUnit ∅ l
+  Quotient.mk' (DHashMap.Const.unitOfArray l)
+
+@[inline, inherit_doc DHashMap.ofList]
+def ofList [BEq α] [Hashable α] (l : List ((a : α) × β a)) :
+    ExtDHashMap α β :=
+  Quotient.mk' (DHashMap.ofList l)
+
+@[inline, inherit_doc DHashMap.Const.ofList]
+def Const.ofList {β : Type v} [BEq α] [Hashable α] (l : List (α × β)) :
+    ExtDHashMap α (fun _ => β) :=
+  Quotient.mk' (DHashMap.Const.ofList l)
+
+@[inline, inherit_doc DHashMap.Const.unitOfList]
+def Const.unitOfList [BEq α] [Hashable α] (l : List α) :
+    ExtDHashMap α (fun _ => Unit) :=
+  Quotient.mk' (DHashMap.Const.unitOfList l)
 
 end ExtDHashMap
 
