src/Std/Data/ExtDHashMap/Lemmas.lean
@@ -19,7 +19,7 @@ attribute [local instance] Std.DHashMap.isSetoid
 
 universe u v w w'
 
-variable {α : Type u} {_ : BEq α} {_ : Hashable α} {_ : EquivBEq α} {_ : LawfulHashable α}
+variable {α : Type u} {_ : BEq α} {_ : Hashable α}
 variable {β : α → Type v} {γ : α → Type w}
 
 namespace Std.ExtDHashMap
@@ -27,99 +27,103 @@ namespace Std.ExtDHashMap
 variable {m : ExtDHashMap α β}
 
 @[simp]
-theorem isEmpty_iff : m.isEmpty ↔ m = ∅ := by
+theorem isEmpty_iff [EquivBEq α] [LawfulHashable α] : m.isEmpty ↔ m = ∅ := by
   rcases m with ⟨m⟩
   refine m.equiv_empty_iff_isEmpty.symm.trans ?_
   exact ⟨fun h => Quotient.sound h, Quotient.exact⟩
 
 @[simp]
-theorem isEmpty_eq_false_iff : m.isEmpty = false ↔ ¬m = ∅ :=
+theorem isEmpty_eq_false_iff [EquivBEq α] [LawfulHashable α] : m.isEmpty = false ↔ ¬m = ∅ :=
   (Bool.not_eq_true _).symm.to_iff.trans (not_congr isEmpty_iff)
 
 @[simp]
 theorem empty_eq : ∅ = m ↔ m = ∅ := eq_comm
 
 @[simp]
-theorem emptyWithCapacity_eq {c} : (emptyWithCapacity c : ExtDHashMap α β) = ∅ :=
+theorem emptyWithCapacity_eq [EquivBEq α] [LawfulHashable α] {c} : (emptyWithCapacity c : ExtDHashMap α β) = ∅ :=
   isEmpty_iff.mp DHashMap.isEmpty_emptyWithCapacity
 
 @[simp]
-theorem not_insert_eq_empty {k : α} {v : β k} :
+theorem not_insert_eq_empty [EquivBEq α] [LawfulHashable α] {k : α} {v : β k} :
     ¬m.insert k v = ∅ :=
   m.inductionOn fun _ => isEmpty_eq_false_iff.mp DHashMap.isEmpty_insert
 
-theorem mem_iff_contains {a : α} : a ∈ m ↔ m.contains a :=
+theorem mem_iff_contains [EquivBEq α] [LawfulHashable α] {a : α} : a ∈ m ↔ m.contains a :=
   Iff.rfl
 
-theorem contains_congr {a b : α} (hab : a == b) : m.contains a = m.contains b :=
+theorem contains_congr [EquivBEq α] [LawfulHashable α] {a b : α} (hab : a == b) : m.contains a = m.contains b :=
   m.inductionOn fun _ => DHashMap.contains_congr hab
 
-theorem mem_congr {a b : α} (hab : a == b) : a ∈ m ↔ b ∈ m :=
+theorem mem_congr [EquivBEq α] [LawfulHashable α] {a b : α} (hab : a == b) : a ∈ m ↔ b ∈ m :=
   m.inductionOn fun _ => DHashMap.mem_congr hab
 
 @[simp]
-theorem contains_empty {a : α} : (∅ : DHashMap α β).contains a = false :=
+theorem contains_empty [EquivBEq α] [LawfulHashable α] {a : α} : (∅ : DHashMap α β).contains a = false :=
   DHashMap.contains_empty
 
 @[simp]
-theorem not_mem_empty {a : α} : ¬a ∈ (∅ : DHashMap α β) :=
+theorem not_mem_empty [EquivBEq α] [LawfulHashable α] {a : α} : ¬a ∈ (∅ : DHashMap α β) :=
   DHashMap.not_mem_empty
 
-theorem eq_empty_iff_forall_contains : m = ∅ ↔ ∀ a, m.contains a = false :=
+theorem eq_empty_iff_forall_contains [EquivBEq α] [LawfulHashable α] : m = ∅ ↔ ∀ a, m.contains a = false :=
   isEmpty_iff.symm.trans <| m.inductionOn fun _ => DHashMap.isEmpty_iff_forall_contains
 
-theorem eq_empty_iff_forall_not_mem : m = ∅ ↔ ∀ a, ¬a ∈ m :=
+theorem eq_empty_iff_forall_not_mem [EquivBEq α] [LawfulHashable α] : m = ∅ ↔ ∀ a, ¬a ∈ m :=
   isEmpty_iff.symm.trans <| m.inductionOn fun _ => DHashMap.isEmpty_iff_forall_not_mem
 
-@[simp] theorem insert_eq_insert {p : (a : α) × β a} : Insert.insert p m = m.insert p.1 p.2 := rfl
+@[simp]
+theorem insert_eq_insert [EquivBEq α] [LawfulHashable α] {p : (a : α) × β a} :
+    Insert.insert p m = m.insert p.1 p.2 :=
+  rfl
 
-@[simp] theorem singleton_eq_insert {p : (a : α) × β a} :
+@[simp]
+theorem singleton_eq_insert [EquivBEq α] [LawfulHashable α] {p : (a : α) × β a} :
     Singleton.singleton p = (∅ : DHashMap α β).insert p.1 p.2 :=
   rfl
 
 @[simp]
-theorem contains_insert {k a : α} {v : β k} :
+theorem contains_insert [EquivBEq α] [LawfulHashable α] {k a : α} {v : β k} :
     (m.insert k v).contains a = (k == a || m.contains a) :=
   m.inductionOn fun _ => DHashMap.contains_insert
 
 @[simp]
-theorem mem_insert {k a : α} {v : β k} : a ∈ m.insert k v ↔ k == a ∨ a ∈ m :=
+theorem mem_insert [EquivBEq α] [LawfulHashable α] {k a : α} {v : β k} : a ∈ m.insert k v ↔ k == a ∨ a ∈ m :=
   m.inductionOn fun _ => DHashMap.mem_insert
 
-theorem contains_of_contains_insert {k a : α} {v : β k} :
+theorem contains_of_contains_insert [EquivBEq α] [LawfulHashable α] {k a : α} {v : β k} :
     (m.insert k v).contains a → (k == a) = false → m.contains a :=
   m.inductionOn fun _ => DHashMap.contains_of_contains_insert
 
-theorem mem_of_mem_insert {k a : α} {v : β k} : a ∈ m.insert k v → (k == a) = false → a ∈ m :=
+theorem mem_of_mem_insert [EquivBEq α] [LawfulHashable α] {k a : α} {v : β k} : a ∈ m.insert k v → (k == a) = false → a ∈ m :=
   m.inductionOn fun _ => DHashMap.mem_of_mem_insert
 
-theorem contains_insert_self {k : α} {v : β k} : (m.insert k v).contains k := by simp
+theorem contains_insert_self [EquivBEq α] [LawfulHashable α] {k : α} {v : β k} : (m.insert k v).contains k := by simp
 
-theorem mem_insert_self {k : α} {v : β k} : k ∈ m.insert k v := by simp
+theorem mem_insert_self [EquivBEq α] [LawfulHashable α] {k : α} {v : β k} : k ∈ m.insert k v := by simp
 
 @[simp]
-theorem size_empty : (∅ : ExtDHashMap α β).size = 0 := rfl
+theorem size_empty [EquivBEq α] [LawfulHashable α] : (∅ : ExtDHashMap α β).size = 0 := rfl
 
-theorem eq_empty_iff_size_eq_zero : m = ∅ ↔ m.size = 0 :=
+theorem eq_empty_iff_size_eq_zero [EquivBEq α] [LawfulHashable α] : m = ∅ ↔ m.size = 0 :=
   isEmpty_iff.symm.trans <| m.inductionOn fun _ =>
     (Bool.eq_iff_iff.mp DHashMap.isEmpty_eq_size_eq_zero).trans beq_iff_eq
 
-theorem size_insert {k : α} {v : β k} :
+theorem size_insert [EquivBEq α] [LawfulHashable α] {k : α} {v : β k} :
     (m.insert k v).size = if k ∈ m then m.size else m.size + 1 :=
   m.inductionOn fun _ => DHashMap.size_insert
 
-theorem size_le_size_insert {k : α} {v : β k} : m.size ≤ (m.insert k v).size :=
+theorem size_le_size_insert [EquivBEq α] [LawfulHashable α] {k : α} {v : β k} : m.size ≤ (m.insert k v).size :=
   m.inductionOn fun _ => DHashMap.size_le_size_insert
 
-theorem size_insert_le {k : α} {v : β k} : (m.insert k v).size ≤ m.size + 1 :=
+theorem size_insert_le [EquivBEq α] [LawfulHashable α] {k : α} {v : β k} : (m.insert k v).size ≤ m.size + 1 :=
   m.inductionOn fun _ => DHashMap.size_insert_le
 
 @[simp]
-theorem erase_empty {k : α} : (∅ : ExtDHashMap α β).erase k = ∅ :=
+theorem erase_empty [EquivBEq α] [LawfulHashable α] {k : α} : (∅ : ExtDHashMap α β).erase k = ∅ :=
   congrArg Quotient.mk' DHashMap.erase_empty
 
 @[simp]
-theorem erase_eq_empty_iff {k : α} : m.erase k = ∅ ↔ m = ∅ ∨ m.size = 1 ∧ k ∈ m := by
+theorem erase_eq_empty_iff [EquivBEq α] [LawfulHashable α] {k : α} : m.erase k = ∅ ↔ m = ∅ ∨ m.size = 1 ∧ k ∈ m := by
   apply isEmpty_iff.symm.trans
   rcases m with ⟨m⟩
   rw [← isEmpty_iff]
@@ -128,48 +132,48 @@ theorem erase_eq_empty_iff {k : α} : m.erase k = ∅ ↔ m = ∅ ∨ m.size = 1
   rfl
 
 @[simp]
-theorem contains_erase {k a : α} :
+theorem contains_erase [EquivBEq α] [LawfulHashable α] {k a : α} :
     (m.erase k).contains a = (!(k == a) && m.contains a) :=
   m.inductionOn fun _ => DHashMap.contains_erase
 
 @[simp]
-theorem mem_erase {k a : α} :
+theorem mem_erase [EquivBEq α] [LawfulHashable α] {k a : α} :
     a ∈ m.erase k ↔ (k == a) = false ∧ a ∈ m := by
   simp [mem_iff_contains, contains_erase]
 
-theorem contains_of_contains_erase {k a : α} :
+theorem contains_of_contains_erase [EquivBEq α] [LawfulHashable α] {k a : α} :
     (m.erase k).contains a → m.contains a :=
   m.inductionOn fun _ => DHashMap.contains_of_contains_erase
 
-theorem mem_of_mem_erase {k a : α} : a ∈ m.erase k → a ∈ m := by
+theorem mem_of_mem_erase [EquivBEq α] [LawfulHashable α] {k a : α} : a ∈ m.erase k → a ∈ m := by
   simp
 
-theorem size_erase {k : α} :
+theorem size_erase [EquivBEq α] [LawfulHashable α] {k : α} :
     (m.erase k).size = if k ∈ m then m.size - 1 else m.size :=
   m.inductionOn fun _ => DHashMap.size_erase
 
-theorem size_erase_le {k : α} : (m.erase k).size ≤ m.size :=
+theorem size_erase_le [EquivBEq α] [LawfulHashable α] {k : α} : (m.erase k).size ≤ m.size :=
   m.inductionOn fun _ => DHashMap.size_erase_le
 
-theorem size_le_size_erase {k : α} :
+theorem size_le_size_erase [EquivBEq α] [LawfulHashable α] {k : α} :
     m.size ≤ (m.erase k).size + 1 :=
   m.inductionOn fun _ => DHashMap.size_le_size_erase
 
 @[simp]
-theorem containsThenInsert_fst {k : α} {v : β k} : (m.containsThenInsert k v).1 = m.contains k :=
+theorem containsThenInsert_fst [EquivBEq α] [LawfulHashable α] {k : α} {v : β k} : (m.containsThenInsert k v).1 = m.contains k :=
   m.inductionOn fun _ => DHashMap.containsThenInsert_fst
 
 @[simp]
-theorem containsThenInsert_snd {k : α} {v : β k} : (m.containsThenInsert k v).2 = m.insert k v :=
+theorem containsThenInsert_snd [EquivBEq α] [LawfulHashable α] {k : α} {v : β k} : (m.containsThenInsert k v).2 = m.insert k v :=
   m.inductionOn fun _ => congrArg Quotient.mk' DHashMap.containsThenInsert_snd
 
 @[simp]
-theorem containsThenInsertIfNew_fst {k : α} {v : β k} :
+theorem containsThenInsertIfNew_fst [EquivBEq α] [LawfulHashable α] {k : α} {v : β k} :
     (m.containsThenInsertIfNew k v).1 = m.contains k :=
   m.inductionOn fun _ => DHashMap.containsThenInsertIfNew_fst
 
 @[simp]
-theorem containsThenInsertIfNew_snd {k : α} {v : β k} :
+theorem containsThenInsertIfNew_snd [EquivBEq α] [LawfulHashable α] {k : α} {v : β k} :
     (m.containsThenInsertIfNew k v).2 = m.insertIfNew k v :=
   m.inductionOn fun _ => congrArg Quotient.mk' DHashMap.containsThenInsertIfNew_snd
 
@@ -211,44 +215,44 @@ namespace Const
 variable {β : Type v} {m : ExtDHashMap α (fun _ => β)}
 
 @[simp]
-theorem get?_empty {a : α} : get? (∅ : ExtDHashMap α (fun _ => β)) a = none :=
+theorem get?_empty [EquivBEq α] [LawfulHashable α] {a : α} : get? (∅ : ExtDHashMap α (fun _ => β)) a = none :=
   DHashMap.Const.get?_empty
 
-theorem get?_insert {k a : α} {v : β} :
+theorem get?_insert [EquivBEq α] [LawfulHashable α] {k a : α} {v : β} :
     get? (m.insert k v) a = if k == a then some v else get? m a :=
   m.inductionOn fun _ => DHashMap.Const.get?_insert
 
 @[simp]
-theorem get?_insert_self {k : α} {v : β} :
+theorem get?_insert_self [EquivBEq α] [LawfulHashable α] {k : α} {v : β} :
     get? (m.insert k v) k = some v :=
   m.inductionOn fun _ => DHashMap.Const.get?_insert_self
 
-theorem contains_eq_isSome_get? {a : α} :
+theorem contains_eq_isSome_get? [EquivBEq α] [LawfulHashable α] {a : α} :
     m.contains a = (get? m a).isSome :=
   m.inductionOn fun _ => DHashMap.Const.contains_eq_isSome_get?
 
-theorem mem_iff_isSome_get? {a : α} : a ∈ m ↔ (get? m a).isSome :=
+theorem mem_iff_isSome_get? [EquivBEq α] [LawfulHashable α] {a : α} : a ∈ m ↔ (get? m a).isSome :=
   m.inductionOn fun _ => DHashMap.Const.mem_iff_isSome_get?
 
-theorem get?_eq_none_of_contains_eq_false {a : α} :
+theorem get?_eq_none_of_contains_eq_false [EquivBEq α] [LawfulHashable α] {a : α} :
     m.contains a = false → get? m a = none :=
   m.inductionOn fun _ => DHashMap.Const.get?_eq_none_of_contains_eq_false
 
-theorem get?_eq_none {a : α} : ¬a ∈ m → get? m a = none := by
+theorem get?_eq_none [EquivBEq α] [LawfulHashable α] {a : α} : ¬a ∈ m → get? m a = none := by
   simpa [mem_iff_contains] using get?_eq_none_of_contains_eq_false
 
-theorem get?_erase {k a : α} :
+theorem get?_erase [EquivBEq α] [LawfulHashable α] {k a : α} :
     Const.get? (m.erase k) a = if k == a then none else get? m a :=
   m.inductionOn fun _ => DHashMap.Const.get?_erase
 
 @[simp]
-theorem get?_erase_self {k : α} : get? (m.erase k) k = none :=
+theorem get?_erase_self [EquivBEq α] [LawfulHashable α] {k : α} : get? (m.erase k) k = none :=
   m.inductionOn fun _ => DHashMap.Const.get?_erase_self
 
 theorem get?_eq_get? [LawfulBEq α] {a : α} : get? m a = m.get? a :=
   m.inductionOn fun _ => DHashMap.Const.get?_eq_get?
 
-theorem get?_congr {a b : α} (hab : a == b) : get? m a = get? m b :=
+theorem get?_congr [EquivBEq α] [LawfulHashable α] {a b : α} (hab : a == b) : get? m a = get? m b :=
   m.inductionOn fun _ => DHashMap.Const.get?_congr hab
 
 end Const
@@ -286,37 +290,37 @@ namespace Const
 
 variable {β : Type v} {m : ExtDHashMap α (fun _ => β)}
 
-theorem get_insert {k a : α} {v : β} {h₁} :
+theorem get_insert [EquivBEq α] [LawfulHashable α] {k a : α} {v : β} {h₁} :
     get (m.insert k v) a h₁ =
       if h₂ : k == a then v else get m a (mem_of_mem_insert h₁ (Bool.eq_false_iff.2 h₂)) :=
   m.inductionOn (fun _ _ => DHashMap.Const.get_insert) h₁
 
 @[simp]
-theorem get_insert_self {k : α} {v : β} :
+theorem get_insert_self [EquivBEq α] [LawfulHashable α] {k : α} {v : β} :
     get (m.insert k v) k mem_insert_self = v :=
   m.inductionOn fun _ => DHashMap.Const.get_insert_self
 
 @[simp]
-theorem get_erase {k a : α} {h'} :
+theorem get_erase [EquivBEq α] [LawfulHashable α] {k a : α} {h'} :
     get (m.erase k) a h' = get m a (mem_of_mem_erase h') :=
   m.inductionOn (fun _ _ => DHashMap.Const.get_erase) h'
 
-theorem get?_eq_some_get {a : α} (h) :
+theorem get?_eq_some_get [EquivBEq α] [LawfulHashable α] {a : α} (h) :
     get? m a = some (get m a h) :=
   m.inductionOn (fun _ h => DHashMap.Const.get?_eq_some_get h) h
 
-theorem get_eq_get_get? {a : α} {h} :
+theorem get_eq_get_get? [EquivBEq α] [LawfulHashable α] {a : α} {h} :
     get m a h = (get? m a).get (mem_iff_isSome_get?.mp h) :=
   m.inductionOn (fun _ _ => DHashMap.Const.get_eq_get_get?) h
 
-theorem get_get? {a : α} {h} :
+theorem get_get? [EquivBEq α] [LawfulHashable α] {a : α} {h} :
     (get? m a).get h = get m a (mem_iff_isSome_get?.mpr h) :=
   m.inductionOn (fun _ _ => DHashMap.Const.get_get?) h
 
 theorem get_eq_get [LawfulBEq α] {a : α} {h} : get m a h = m.get a h :=
   m.inductionOn (fun _ _ => DHashMap.Const.get_eq_get) h
 
-theorem get_congr {a b : α} (hab : a == b) {h'} :
+theorem get_congr [EquivBEq α] [LawfulHashable α] {a b : α} (hab : a == b) {h'} :
     get m a h' = get m b ((mem_congr hab).1 h') :=
   m.inductionOn (fun _ hab _ => DHashMap.Const.get_congr hab) hab h'
 
@@ -375,48 +379,48 @@ namespace Const
 variable {β : Type v} {m : ExtDHashMap α (fun _ => β)}
 
 @[simp]
-theorem get!_empty [Inhabited β] {a : α} : get! (∅ : ExtDHashMap α (fun _ => β)) a = default :=
+theorem get!_empty [EquivBEq α] [LawfulHashable α] [Inhabited β] {a : α} : get! (∅ : ExtDHashMap α (fun _ => β)) a = default :=
   DHashMap.Const.get!_empty
 
-theorem get!_insert [Inhabited β] {k a : α} {v : β} :
+theorem get!_insert [EquivBEq α] [LawfulHashable α] [Inhabited β] {k a : α} {v : β} :
     get! (m.insert k v) a = if k == a then v else get! m a :=
   m.inductionOn fun _ => DHashMap.Const.get!_insert
 
 @[simp]
-theorem get!_insert_self [Inhabited β] {k : α} {v : β} :
+theorem get!_insert_self [EquivBEq α] [LawfulHashable α] [Inhabited β] {k : α} {v : β} :
     get! (m.insert k v) k = v :=
   m.inductionOn fun _ => DHashMap.Const.get!_insert_self
 
-theorem get!_eq_default_of_contains_eq_false [Inhabited β] {a : α} :
+theorem get!_eq_default_of_contains_eq_false [EquivBEq α] [LawfulHashable α] [Inhabited β] {a : α} :
     m.contains a = false → get! m a = default :=
   m.inductionOn fun _ => DHashMap.Const.get!_eq_default_of_contains_eq_false
 
-theorem get!_eq_default [Inhabited β] {a : α} :
+theorem get!_eq_default [EquivBEq α] [LawfulHashable α] [Inhabited β] {a : α} :
     ¬a ∈ m → get! m a = default :=
   m.inductionOn fun _ => DHashMap.Const.get!_eq_default
 
-theorem get!_erase [Inhabited β] {k a : α} :
+theorem get!_erase [EquivBEq α] [LawfulHashable α] [Inhabited β] {k a : α} :
     get! (m.erase k) a = if k == a then default else get! m a :=
   m.inductionOn fun _ => DHashMap.Const.get!_erase
 
 @[simp]
-theorem get!_erase_self [Inhabited β] {k : α} :
+theorem get!_erase_self [EquivBEq α] [LawfulHashable α] [Inhabited β] {k : α} :
     get! (m.erase k) k = default :=
   m.inductionOn fun _ => DHashMap.Const.get!_erase_self
 
-theorem get?_eq_some_get!_of_contains [Inhabited β] {a : α} :
+theorem get?_eq_some_get!_of_contains [EquivBEq α] [LawfulHashable α] [Inhabited β] {a : α} :
     m.contains a = true → get? m a = some (get! m a) :=
   m.inductionOn fun _ => DHashMap.Const.get?_eq_some_get!_of_contains
 
-theorem get?_eq_some_get! [Inhabited β] {a : α} :
+theorem get?_eq_some_get! [EquivBEq α] [LawfulHashable α] [Inhabited β] {a : α} :
     a ∈ m → get? m a = some (get! m a) :=
   m.inductionOn fun _ => DHashMap.Const.get?_eq_some_get!
 
-theorem get!_eq_get!_get? [Inhabited β] {a : α} :
+theorem get!_eq_get!_get? [EquivBEq α] [LawfulHashable α] [Inhabited β] {a : α} :
     get! m a = (get? m a).get! :=
   m.inductionOn fun _ => DHashMap.Const.get!_eq_get!_get?
 
-theorem get_eq_get! [Inhabited β] {a : α} {h} :
+theorem get_eq_get! [EquivBEq α] [LawfulHashable α] [Inhabited β] {a : α} {h} :
     get m a h = get! m a :=
   m.inductionOn (fun _ _ => DHashMap.Const.get_eq_get!) h
 
@@ -424,7 +428,7 @@ theorem get!_eq_get! [LawfulBEq α] [Inhabited β] {a : α} :
     get! m a = m.get! a :=
   m.inductionOn fun _ => DHashMap.Const.get!_eq_get!
 
-theorem get!_congr [Inhabited β] {a b : α} (hab : a == b) :
+theorem get!_congr [EquivBEq α] [LawfulHashable α] [Inhabited β] {a b : α} (hab : a == b) :
     get! m a = get! m b :=
   m.inductionOn (fun _ hab => DHashMap.Const.get!_congr hab) hab
 
@@ -487,53 +491,53 @@ namespace Const
 variable {β : Type v} {m : ExtDHashMap α (fun _ => β)}
 
 @[simp]
-theorem getD_empty {a : α} {fallback : β} :
+theorem getD_empty [EquivBEq α] [LawfulHashable α] {a : α} {fallback : β} :
     getD (∅ : ExtDHashMap α (fun _ => β)) a fallback = fallback :=
   DHashMap.Const.getD_empty
 
-theorem getD_insert {k a : α} {fallback v : β} :
+theorem getD_insert [EquivBEq α] [LawfulHashable α] {k a : α} {fallback v : β} :
     getD (m.insert k v) a fallback = if k == a then v else getD m a fallback :=
   m.inductionOn fun _ => DHashMap.Const.getD_insert
 
 @[simp]
-theorem getD_insert_self {k : α} {fallback v : β} :
+theorem getD_insert_self [EquivBEq α] [LawfulHashable α] {k : α} {fallback v : β} :
    getD (m.insert k v) k fallback = v :=
   m.inductionOn fun _ => DHashMap.Const.getD_insert_self
 
-theorem getD_eq_fallback_of_contains_eq_false {a : α}
+theorem getD_eq_fallback_of_contains_eq_false [EquivBEq α] [LawfulHashable α] {a : α}
     {fallback : β} : m.contains a = false → getD m a fallback = fallback :=
   m.inductionOn fun _ => DHashMap.Const.getD_eq_fallback_of_contains_eq_false
 
-theorem getD_eq_fallback {a : α} {fallback : β} :
+theorem getD_eq_fallback [EquivBEq α] [LawfulHashable α] {a : α} {fallback : β} :
     ¬a ∈ m → getD m a fallback = fallback :=
   m.inductionOn fun _ => DHashMap.Const.getD_eq_fallback
 
-theorem getD_erase {k a : α} {fallback : β} :
+theorem getD_erase [EquivBEq α] [LawfulHashable α] {k a : α} {fallback : β} :
     getD (m.erase k) a fallback = if k == a then fallback else getD m a fallback :=
   m.inductionOn fun _ => DHashMap.Const.getD_erase
 
 @[simp]
-theorem getD_erase_self {k : α} {fallback : β} :
+theorem getD_erase_self [EquivBEq α] [LawfulHashable α] {k : α} {fallback : β} :
     getD (m.erase k) k fallback = fallback :=
   m.inductionOn fun _ => DHashMap.Const.getD_erase_self
 
-theorem get?_eq_some_getD_of_contains {a : α} {fallback : β} :
+theorem get?_eq_some_getD_of_contains [EquivBEq α] [LawfulHashable α] {a : α} {fallback : β} :
     m.contains a = true → get? m a = some (getD m a fallback) :=
   m.inductionOn fun _ => DHashMap.Const.get?_eq_some_getD_of_contains
 
-theorem get?_eq_some_getD {a : α} {fallback : β} :
+theorem get?_eq_some_getD [EquivBEq α] [LawfulHashable α] {a : α} {fallback : β} :
     a ∈ m → get? m a = some (getD m a fallback) :=
   m.inductionOn fun _ => DHashMap.Const.get?_eq_some_getD
 
-theorem getD_eq_getD_get? {a : α} {fallback : β} :
+theorem getD_eq_getD_get? [EquivBEq α] [LawfulHashable α] {a : α} {fallback : β} :
     getD m a fallback = (get? m a).getD fallback :=
   m.inductionOn fun _ => DHashMap.Const.getD_eq_getD_get?
 
-theorem get_eq_getD {a : α} {fallback : β} {h} :
+theorem get_eq_getD [EquivBEq α] [LawfulHashable α] {a : α} {fallback : β} {h} :
     get m a h = getD m a fallback :=
   m.inductionOn (fun _ _ => DHashMap.Const.get_eq_getD) h
 
-theorem get!_eq_getD_default [Inhabited β] {a : α} :
+theorem get!_eq_getD_default [EquivBEq α] [LawfulHashable α] [Inhabited β] {a : α} :
     get! m a = getD m a default :=
   m.inductionOn fun _ => DHashMap.Const.get!_eq_getD_default
 
@@ -541,57 +545,57 @@ theorem getD_eq_getD [LawfulBEq α] {a : α} {fallback : β} :
     getD m a fallback = m.getD a fallback :=
   m.inductionOn fun _ => DHashMap.Const.getD_eq_getD
 
-theorem getD_congr {a b : α} {fallback : β} (hab : a == b) :
+theorem getD_congr [EquivBEq α] [LawfulHashable α] {a b : α} {fallback : β} (hab : a == b) :
     getD m a fallback = getD m b fallback :=
   m.inductionOn (fun _ hab => DHashMap.Const.getD_congr hab) hab
 
 end Const
 
 @[simp]
-theorem getKey?_empty {a : α} : (∅ : ExtDHashMap α β).getKey? a = none :=
+theorem getKey?_empty [EquivBEq α] [LawfulHashable α] {a : α} : (∅ : ExtDHashMap α β).getKey? a = none :=
   DHashMap.getKey?_empty
 
-theorem getKey?_insert {a k : α} {v : β k} :
+theorem getKey?_insert [EquivBEq α] [LawfulHashable α] {a k : α} {v : β k} :
     (m.insert k v).getKey? a = if k == a then some k else m.getKey? a :=
   m.inductionOn fun _ => DHashMap.getKey?_insert
 
 @[simp]
-theorem getKey?_insert_self {k : α} {v : β k} :
+theorem getKey?_insert_self [EquivBEq α] [LawfulHashable α] {k : α} {v : β k} :
     (m.insert k v).getKey? k = some k :=
   m.inductionOn fun _ => DHashMap.getKey?_insert_self
 
-theorem contains_eq_isSome_getKey? {a : α} :
+theorem contains_eq_isSome_getKey? [EquivBEq α] [LawfulHashable α] {a : α} :
     m.contains a = (m.getKey? a).isSome :=
   m.inductionOn fun _ => DHashMap.contains_eq_isSome_getKey?
 
-theorem mem_iff_isSome_getKey? {a : α} :
+theorem mem_iff_isSome_getKey? [EquivBEq α] [LawfulHashable α] {a : α} :
     a ∈ m ↔ (m.getKey? a).isSome :=
   m.inductionOn fun _ => DHashMap.mem_iff_isSome_getKey?
 
-theorem mem_of_getKey?_eq_some {k k' : α}
+theorem mem_of_getKey?_eq_some [EquivBEq α] [LawfulHashable α] {k k' : α}
     (h : m.getKey? k = some k') : k' ∈ m :=
   m.inductionOn (fun _ h => DHashMap.mem_of_getKey?_eq_some h) h
 
-theorem getKey?_eq_none_of_contains_eq_false {a : α} :
+theorem getKey?_eq_none_of_contains_eq_false [EquivBEq α] [LawfulHashable α] {a : α} :
     m.contains a = false → m.getKey? a = none :=
   m.inductionOn fun _ => DHashMap.getKey?_eq_none_of_contains_eq_false
 
-theorem getKey?_eq_none {a : α} : ¬a ∈ m → m.getKey? a = none :=
+theorem getKey?_eq_none [EquivBEq α] [LawfulHashable α] {a : α} : ¬a ∈ m → m.getKey? a = none :=
   m.inductionOn fun _ => DHashMap.getKey?_eq_none
 
-theorem getKey?_erase {k a : α} :
+theorem getKey?_erase [EquivBEq α] [LawfulHashable α] {k a : α} :
     (m.erase k).getKey? a = if k == a then none else m.getKey? a :=
   m.inductionOn fun _ => DHashMap.getKey?_erase
 
 @[simp]
-theorem getKey?_erase_self {k : α} : (m.erase k).getKey? k = none :=
+theorem getKey?_erase_self [EquivBEq α] [LawfulHashable α] {k : α} : (m.erase k).getKey? k = none :=
   m.inductionOn fun _ => DHashMap.getKey?_erase_self
 
-theorem getKey?_beq {k : α} :
+theorem getKey?_beq [EquivBEq α] [LawfulHashable α] {k : α} :
     (m.getKey? k).all (· == k) :=
   m.inductionOn fun _ => DHashMap.getKey?_beq
 
-theorem getKey?_congr {k k' : α} (h : k == k') :
+theorem getKey?_congr [EquivBEq α] [LawfulHashable α] {k k' : α} (h : k == k') :
     m.getKey? k = m.getKey? k' :=
   m.inductionOn (fun _ h => DHashMap.getKey?_congr h) h
 
@@ -602,7 +606,7 @@ theorem getKey?_eq_some_of_contains [LawfulBEq α] {k : α} (h : m.contains k) :
 theorem getKey?_eq_some [LawfulBEq α] {k : α} (h : k ∈ m) : m.getKey? k = some k :=
   m.inductionOn (fun _ h => DHashMap.getKey?_eq_some h) h
 
-theorem getKey_insert {k a : α} {v : β k} {h₁} :
+theorem getKey_insert [EquivBEq α] [LawfulHashable α] {k a : α} {v : β k} {h₁} :
     (m.insert k v).getKey a h₁ =
       if h₂ : k == a then
         k
@@ -611,31 +615,31 @@ theorem getKey_insert {k a : α} {v : β k} {h₁} :
   m.inductionOn (fun _ _ => DHashMap.getKey_insert) h₁
 
 @[simp]
-theorem getKey_insert_self {k : α} {v : β k} :
+theorem getKey_insert_self [EquivBEq α] [LawfulHashable α] {k : α} {v : β k} :
     (m.insert k v).getKey k mem_insert_self = k :=
   m.inductionOn fun _ => DHashMap.getKey_insert_self
 
 @[simp]
-theorem getKey_erase {k a : α} {h'} :
+theorem getKey_erase [EquivBEq α] [LawfulHashable α] {k a : α} {h'} :
     (m.erase k).getKey a h' = m.getKey a (mem_of_mem_erase h') :=
   m.inductionOn (fun _ _ => DHashMap.getKey_erase) h'
 
-theorem getKey?_eq_some_getKey {a : α} (h) :
+theorem getKey?_eq_some_getKey [EquivBEq α] [LawfulHashable α] {a : α} (h) :
     m.getKey? a = some (m.getKey a h) :=
   m.inductionOn (fun _ h => DHashMap.getKey?_eq_some_getKey h) h
 
-theorem getKey_eq_get_getKey? {a : α} {h} :
+theorem getKey_eq_get_getKey? [EquivBEq α] [LawfulHashable α] {a : α} {h} :
     m.getKey a h = (m.getKey? a).get (mem_iff_isSome_getKey?.mp h) :=
   m.inductionOn (fun _ _ => DHashMap.getKey_eq_get_getKey?) h
 
-theorem get_getKey? {a : α} {h} :
+theorem get_getKey? [EquivBEq α] [LawfulHashable α] {a : α} {h} :
     (m.getKey? a).get h = m.getKey a (mem_iff_isSome_getKey?.mpr h) :=
   m.inductionOn (fun _ _ => DHashMap.get_getKey?) h
 
-theorem getKey_beq {k : α} (h : k ∈ m) : m.getKey k h == k :=
+theorem getKey_beq [EquivBEq α] [LawfulHashable α] {k : α} (h : k ∈ m) : m.getKey k h == k :=
   m.inductionOn (fun _ h => DHashMap.getKey_beq h) h
 
-theorem getKey_congr {k₁ k₂ : α} (h : k₁ == k₂)
+theorem getKey_congr [EquivBEq α] [LawfulHashable α] {k₁ k₂ : α} (h : k₁ == k₂)
     (h₁ : k₁ ∈ m) : m.getKey k₁ h₁ = m.getKey k₂ ((mem_congr h).mp h₁) :=
   m.inductionOn (fun _ h h₁ => DHashMap.getKey_congr h h₁) h h₁
 
@@ -643,55 +647,55 @@ theorem getKey_eq [LawfulBEq α] {k : α} (h : k ∈ m) : m.getKey k h = k :=
   m.inductionOn (fun _ h => DHashMap.getKey_eq h) h
 
 @[simp]
-theorem getKey!_empty [Inhabited α] {a : α} :
+theorem getKey!_empty [EquivBEq α] [LawfulHashable α] [Inhabited α] {a : α} :
     (∅ : ExtDHashMap α β).getKey! a = default :=
   DHashMap.getKey!_empty
 
-theorem getKey!_insert [Inhabited α] {k a : α} {v : β k} :
+theorem getKey!_insert [EquivBEq α] [LawfulHashable α] [Inhabited α] {k a : α} {v : β k} :
     (m.insert k v).getKey! a =
       if k == a then k else m.getKey! a :=
   m.inductionOn fun _ => DHashMap.getKey!_insert
 
 @[simp]
-theorem getKey!_insert_self [Inhabited α] {a : α} {b : β a} :
+theorem getKey!_insert_self [EquivBEq α] [LawfulHashable α] [Inhabited α] {a : α} {b : β a} :
     (m.insert a b).getKey! a = a :=
   m.inductionOn fun _ => DHashMap.getKey!_insert_self
 
-theorem getKey!_eq_default_of_contains_eq_false [Inhabited α]
+theorem getKey!_eq_default_of_contains_eq_false [EquivBEq α] [LawfulHashable α] [Inhabited α]
     {a : α} :
     m.contains a = false → m.getKey! a = default :=
   m.inductionOn fun _ => DHashMap.getKey!_eq_default_of_contains_eq_false
 
-theorem getKey!_eq_default [Inhabited α] {a : α} :
+theorem getKey!_eq_default [EquivBEq α] [LawfulHashable α] [Inhabited α] {a : α} :
     ¬a ∈ m → m.getKey! a = default :=
   m.inductionOn fun _ => DHashMap.getKey!_eq_default
 
-theorem getKey!_erase [Inhabited α] {k a : α} :
+theorem getKey!_erase [EquivBEq α] [LawfulHashable α] [Inhabited α] {k a : α} :
     (m.erase k).getKey! a = if k == a then default else m.getKey! a :=
   m.inductionOn fun _ => DHashMap.getKey!_erase
 
 @[simp]
-theorem getKey!_erase_self [Inhabited α] {k : α} :
+theorem getKey!_erase_self [EquivBEq α] [LawfulHashable α] [Inhabited α] {k : α} :
     (m.erase k).getKey! k = default :=
   m.inductionOn fun _ => DHashMap.getKey!_erase_self
 
-theorem getKey?_eq_some_getKey!_of_contains [Inhabited α] {a : α} :
+theorem getKey?_eq_some_getKey!_of_contains [EquivBEq α] [LawfulHashable α] [Inhabited α] {a : α} :
     m.contains a = true → m.getKey? a = some (m.getKey! a) :=
   m.inductionOn fun _ => DHashMap.getKey?_eq_some_getKey!_of_contains
 
-theorem getKey?_eq_some_getKey! [Inhabited α] {a : α} :
+theorem getKey?_eq_some_getKey! [EquivBEq α] [LawfulHashable α] [Inhabited α] {a : α} :
     a ∈ m → m.getKey? a = some (m.getKey! a) :=
   m.inductionOn fun _ => DHashMap.getKey?_eq_some_getKey!
 
-theorem getKey!_eq_get!_getKey? [Inhabited α] {a : α} :
+theorem getKey!_eq_get!_getKey? [EquivBEq α] [LawfulHashable α] [Inhabited α] {a : α} :
     m.getKey! a = (m.getKey? a).get! :=
   m.inductionOn fun _ => DHashMap.getKey!_eq_get!_getKey?
 
-theorem getKey_eq_getKey! [Inhabited α] {a : α} {h} :
+theorem getKey_eq_getKey! [EquivBEq α] [LawfulHashable α] [Inhabited α] {a : α} {h} :
     m.getKey a h = m.getKey! a :=
   m.inductionOn (fun _ _ => DHashMap.getKey_eq_getKey!) h
 
-theorem getKey!_congr [Inhabited α] {k k' : α} (h : k == k') :
+theorem getKey!_congr [EquivBEq α] [LawfulHashable α] [Inhabited α] {k k' : α} (h : k == k') :
     m.getKey! k = m.getKey! k' :=
   m.inductionOn (fun _ h => DHashMap.getKey!_congr h) h
 
@@ -703,59 +707,59 @@ theorem getKey!_eq_of_mem [LawfulBEq α] [Inhabited α] {k : α} (h : k ∈ m) :
   m.inductionOn (fun _ h => DHashMap.getKey!_eq_of_mem h) h
 
 @[simp]
-theorem getKeyD_empty {a fallback : α} :
+theorem getKeyD_empty [EquivBEq α] [LawfulHashable α] {a fallback : α} :
     (∅ : ExtDHashMap α β).getKeyD a fallback = fallback :=
   DHashMap.getKeyD_empty
 
-theorem getKeyD_insert {k a fallback : α} {v : β k} :
+theorem getKeyD_insert [EquivBEq α] [LawfulHashable α] {k a fallback : α} {v : β k} :
     (m.insert k v).getKeyD a fallback =
       if k == a then k else m.getKeyD a fallback :=
   m.inductionOn fun _ => DHashMap.getKeyD_insert
 
 @[simp]
-theorem getKeyD_insert_self {k fallback : α} {v : β k} :
+theorem getKeyD_insert_self [EquivBEq α] [LawfulHashable α] {k fallback : α} {v : β k} :
     (m.insert k v).getKeyD k fallback = k :=
   m.inductionOn fun _ => DHashMap.getKeyD_insert_self
 
-theorem getKeyD_eq_fallback_of_contains_eq_false {a : α}
+theorem getKeyD_eq_fallback_of_contains_eq_false [EquivBEq α] [LawfulHashable α] {a : α}
     {fallback : α} :
     m.contains a = false → m.getKeyD a fallback = fallback :=
   m.inductionOn fun _ => DHashMap.getKeyD_eq_fallback_of_contains_eq_false
 
-theorem getKeyD_eq_fallback {a fallback : α} :
+theorem getKeyD_eq_fallback [EquivBEq α] [LawfulHashable α] {a fallback : α} :
     ¬a ∈ m → m.getKeyD a fallback = fallback :=
   m.inductionOn fun _ => DHashMap.getKeyD_eq_fallback
 
-theorem getKeyD_erase {k a fallback : α} :
+theorem getKeyD_erase [EquivBEq α] [LawfulHashable α] {k a fallback : α} :
     (m.erase k).getKeyD a fallback = if k == a then fallback else m.getKeyD a fallback :=
   m.inductionOn fun _ => DHashMap.getKeyD_erase
 
 @[simp]
-theorem getKeyD_erase_self {k fallback : α} :
+theorem getKeyD_erase_self [EquivBEq α] [LawfulHashable α] {k fallback : α} :
     (m.erase k).getKeyD k fallback = fallback :=
   m.inductionOn fun _ => DHashMap.getKeyD_erase_self
 
-theorem getKey?_eq_some_getKeyD_of_contains {a fallback : α} :
+theorem getKey?_eq_some_getKeyD_of_contains [EquivBEq α] [LawfulHashable α] {a fallback : α} :
     m.contains a = true → m.getKey? a = some (m.getKeyD a fallback) :=
   m.inductionOn fun _ => DHashMap.getKey?_eq_some_getKeyD_of_contains
 
-theorem getKey?_eq_some_getKeyD {a fallback : α} :
+theorem getKey?_eq_some_getKeyD [EquivBEq α] [LawfulHashable α] {a fallback : α} :
     a ∈ m → m.getKey? a = some (m.getKeyD a fallback) :=
   m.inductionOn fun _ => DHashMap.getKey?_eq_some_getKeyD
 
-theorem getKeyD_eq_getD_getKey? {a fallback : α} :
+theorem getKeyD_eq_getD_getKey? [EquivBEq α] [LawfulHashable α] {a fallback : α} :
     m.getKeyD a fallback = (m.getKey? a).getD fallback :=
   m.inductionOn fun _ => DHashMap.getKeyD_eq_getD_getKey?
 
-theorem getKey_eq_getKeyD {a fallback : α} {h} :
+theorem getKey_eq_getKeyD [EquivBEq α] [LawfulHashable α] {a fallback : α} {h} :
     m.getKey a h = m.getKeyD a fallback :=
   m.inductionOn (fun _ _ => DHashMap.getKey_eq_getKeyD) h
 
-theorem getKey!_eq_getKeyD_default [Inhabited α] {a : α} :
+theorem getKey!_eq_getKeyD_default [EquivBEq α] [LawfulHashable α] [Inhabited α] {a : α} :
     m.getKey! a = m.getKeyD a default :=
   m.inductionOn fun _ => DHashMap.getKey!_eq_getKeyD_default
 
-theorem getKeyD_congr {k k' fallback : α}
+theorem getKeyD_congr [EquivBEq α] [LawfulHashable α] {k k' fallback : α}
     (h : k == k') : m.getKeyD k fallback = m.getKeyD k' fallback :=
   m.inductionOn (fun _ h => DHashMap.getKeyD_congr h) h
 
@@ -768,57 +772,57 @@ theorem getKeyD_eq_of_mem [LawfulBEq α] {k fallback : α} (h : k ∈ m) :
   m.inductionOn (fun _ h => DHashMap.getKeyD_eq_of_mem h) h
 
 @[simp]
-theorem not_insertIfNew_eq_empty {k : α} {v : β k} :
+theorem not_insertIfNew_eq_empty [EquivBEq α] [LawfulHashable α] {k : α} {v : β k} :
     ¬m.insertIfNew k v = ∅ :=
   isEmpty_eq_false_iff.mp <| m.inductionOn fun _ => DHashMap.isEmpty_insertIfNew
 
 @[simp]
-theorem contains_insertIfNew {k a : α} {v : β k} :
+theorem contains_insertIfNew [EquivBEq α] [LawfulHashable α] {k a : α} {v : β k} :
     (m.insertIfNew k v).contains a = (k == a || m.contains a) :=
   m.inductionOn fun _ => DHashMap.contains_insertIfNew
 
 @[simp]
-theorem mem_insertIfNew {k a : α} {v : β k} :
+theorem mem_insertIfNew [EquivBEq α] [LawfulHashable α] {k a : α} {v : β k} :
     a ∈ m.insertIfNew k v ↔ k == a ∨ a ∈ m :=
   m.inductionOn fun _ => DHashMap.mem_insertIfNew
 
-theorem contains_insertIfNew_self {k : α} {v : β k} :
+theorem contains_insertIfNew_self [EquivBEq α] [LawfulHashable α] {k : α} {v : β k} :
     (m.insertIfNew k v).contains k :=
   m.inductionOn fun _ => DHashMap.contains_insertIfNew_self
 
-theorem mem_insertIfNew_self {k : α} {v : β k} :
+theorem mem_insertIfNew_self [EquivBEq α] [LawfulHashable α] {k : α} {v : β k} :
     k ∈ m.insertIfNew k v :=
   m.inductionOn fun _ => DHashMap.mem_insertIfNew_self
 
-theorem contains_of_contains_insertIfNew {k a : α} {v : β k} :
+theorem contains_of_contains_insertIfNew [EquivBEq α] [LawfulHashable α] {k a : α} {v : β k} :
     (m.insertIfNew k v).contains a → (k == a) = false → m.contains a :=
   m.inductionOn fun _ => DHashMap.contains_of_contains_insertIfNew
 
-theorem mem_of_mem_insertIfNew {k a : α} {v : β k} :
+theorem mem_of_mem_insertIfNew [EquivBEq α] [LawfulHashable α] {k a : α} {v : β k} :
     a ∈ m.insertIfNew k v → (k == a) = false → a ∈ m :=
   m.inductionOn fun _ => DHashMap.mem_of_mem_insertIfNew
 
 /-- This is a restatement of `contains_of_contains_insertIfNew` that is written to exactly match the proof
 obligation in the statement of `get_insertIfNew`. -/
-theorem contains_of_contains_insertIfNew' {k a : α} {v : β k} :
+theorem contains_of_contains_insertIfNew' [EquivBEq α] [LawfulHashable α] {k a : α} {v : β k} :
     (m.insertIfNew k v).contains a → ¬((k == a) ∧ m.contains k = false) → m.contains a :=
   m.inductionOn fun _ => DHashMap.contains_of_contains_insertIfNew'
 
 /-- This is a restatement of `mem_of_mem_insertIfNew` that is written to exactly match the proof obligation
 in the statement of `get_insertIfNew`. -/
-theorem mem_of_mem_insertIfNew' {k a : α} {v : β k} :
+theorem mem_of_mem_insertIfNew' [EquivBEq α] [LawfulHashable α] {k a : α} {v : β k} :
     a ∈ m.insertIfNew k v → ¬((k == a) ∧ ¬k ∈ m) → a ∈ m :=
   m.inductionOn fun _ => DHashMap.mem_of_mem_insertIfNew'
 
-theorem size_insertIfNew {k : α} {v : β k} :
+theorem size_insertIfNew [EquivBEq α] [LawfulHashable α] {k : α} {v : β k} :
     (m.insertIfNew k v).size = if k ∈ m then m.size else m.size + 1 :=
   m.inductionOn fun _ => DHashMap.size_insertIfNew
 
-theorem size_le_size_insertIfNew {k : α} {v : β k} :
+theorem size_le_size_insertIfNew [EquivBEq α] [LawfulHashable α] {k : α} {v : β k} :
     m.size ≤ (m.insertIfNew k v).size :=
   m.inductionOn fun _ => DHashMap.size_le_size_insertIfNew
 
-theorem size_insertIfNew_le {k : α} {v : β k} :
+theorem size_insertIfNew_le [EquivBEq α] [LawfulHashable α] {k : α} {v : β k} :
     (m.insertIfNew k v).size ≤ m.size + 1 :=
   m.inductionOn fun _ => DHashMap.size_insertIfNew_le
 
@@ -846,40 +850,40 @@ namespace Const
 
 variable {β : Type v} {m : ExtDHashMap α (fun _ => β)}
 
-theorem get?_insertIfNew {k a : α} {v : β} :
+theorem get?_insertIfNew [EquivBEq α] [LawfulHashable α] {k a : α} {v : β} :
     get? (m.insertIfNew k v) a = if k == a ∧ ¬k ∈ m then some v else get? m a :=
   m.inductionOn fun _ => DHashMap.Const.get?_insertIfNew
 
-theorem get_insertIfNew {k a : α} {v : β} {h₁} :
+theorem get_insertIfNew [EquivBEq α] [LawfulHashable α] {k a : α} {v : β} {h₁} :
     get (m.insertIfNew k v) a h₁ =
       if h₂ : k == a ∧ ¬k ∈ m then v else get m a (mem_of_mem_insertIfNew' h₁ h₂) :=
   m.inductionOn (fun _ _ => DHashMap.Const.get_insertIfNew) h₁
 
-theorem get!_insertIfNew [Inhabited β] {k a : α} {v : β} :
+theorem get!_insertIfNew [EquivBEq α] [LawfulHashable α] [Inhabited β] {k a : α} {v : β} :
     get! (m.insertIfNew k v) a = if k == a ∧ ¬k ∈ m then v else get! m a :=
   m.inductionOn fun _ => DHashMap.Const.get!_insertIfNew
 
-theorem getD_insertIfNew {k a : α} {fallback v : β} :
+theorem getD_insertIfNew [EquivBEq α] [LawfulHashable α] {k a : α} {fallback v : β} :
     getD (m.insertIfNew k v) a fallback =
       if k == a ∧ ¬k ∈ m then v else getD m a fallback :=
   m.inductionOn fun _ => DHashMap.Const.getD_insertIfNew
 
 end Const
 
-theorem getKey?_insertIfNew {k a : α} {v : β k} :
+theorem getKey?_insertIfNew [EquivBEq α] [LawfulHashable α] {k a : α} {v : β k} :
     getKey? (m.insertIfNew k v) a = if k == a ∧ ¬k ∈ m then some k else getKey? m a :=
   m.inductionOn fun _ => DHashMap.getKey?_insertIfNew
 
-theorem getKey_insertIfNew {k a : α} {v : β k} {h₁} :
+theorem getKey_insertIfNew [EquivBEq α] [LawfulHashable α] {k a : α} {v : β k} {h₁} :
     getKey (m.insertIfNew k v) a h₁ =
       if h₂ : k == a ∧ ¬k ∈ m then k else getKey m a (mem_of_mem_insertIfNew' h₁ h₂) :=
   m.inductionOn (fun _ _ => DHashMap.getKey_insertIfNew) h₁
 
-theorem getKey!_insertIfNew [Inhabited α] {k a : α} {v : β k} :
+theorem getKey!_insertIfNew [EquivBEq α] [LawfulHashable α] [Inhabited α] {k a : α} {v : β k} :
     getKey! (m.insertIfNew k v) a = if k == a ∧ ¬k ∈ m then k else getKey! m a :=
   m.inductionOn fun _ => DHashMap.getKey!_insertIfNew
 
-theorem getKeyD_insertIfNew {k a fallback : α} {v : β k} :
+theorem getKeyD_insertIfNew [EquivBEq α] [LawfulHashable α] {k a fallback : α} {v : β k} :
     getKeyD (m.insertIfNew k v) a fallback =
       if k == a ∧ ¬k ∈ m then k else getKeyD m a fallback :=
   m.inductionOn fun _ => DHashMap.getKeyD_insertIfNew
@@ -899,11 +903,11 @@ namespace Const
 variable {β : Type v} {m : ExtDHashMap α (fun _ => β)}
 
 @[simp]
-theorem getThenInsertIfNew?_fst {k : α} {v : β} : (getThenInsertIfNew? m k v).1 = get? m k :=
+theorem getThenInsertIfNew?_fst [EquivBEq α] [LawfulHashable α] {k : α} {v : β} : (getThenInsertIfNew? m k v).1 = get? m k :=
   m.inductionOn fun _ => DHashMap.Const.getThenInsertIfNew?_fst
 
 @[simp]
-theorem getThenInsertIfNew?_snd {k : α} {v : β} :
+theorem getThenInsertIfNew?_snd [EquivBEq α] [LawfulHashable α] {k : α} {v : β} :
     (getThenInsertIfNew? m k v).2 = m.insertIfNew k v :=
   m.inductionOn fun _ => congrArg Quotient.mk' DHashMap.Const.getThenInsertIfNew?_snd
 
@@ -914,13 +918,14 @@ section insertMany
 variable {ρ : Type w} [ForIn Id ρ ((a : α) × β a)]
 
 @[simp]
-theorem insertMany_nil : m.insertMany [] = m := rfl
+theorem insertMany_nil [EquivBEq α] [LawfulHashable α] : m.insertMany [] = m := rfl
 
 @[simp]
-theorem insertMany_list_singleton {k : α} {v : β k} :
+theorem insertMany_list_singleton [EquivBEq α] [LawfulHashable α] {k : α} {v : β k} :
     m.insertMany [⟨k, v⟩] = m.insert k v := rfl
 
-theorem insertMany_cons {l : List ((a : α) × β a)} {p : (a : α) × β a} :
+theorem insertMany_cons [EquivBEq α] [LawfulHashable α]
+    {l : List ((a : α) × β a)} {p : (a : α) × β a} :
     m.insertMany (p :: l) = (m.insert p.1 p.2).insertMany l := by
   rcases p with ⟨k, v⟩
   unfold insertMany
@@ -929,7 +934,8 @@ theorem insertMany_cons {l : List ((a : α) × β a)} {p : (a : α) × β a} :
   exact (List.foldl_hom (f := Subtype.val) fun x y => rfl).symm
   exact (List.foldl_hom (f := Subtype.val) fun x y => rfl).symm
 
-private theorem insertMany_list_mk {m : DHashMap α β} {l : List ((a : α) × β a)} :
+private theorem insertMany_list_mk [EquivBEq α] [LawfulHashable α]
+    {m : DHashMap α β} {l : List ((a : α) × β a)} :
     (ExtDHashMap.insertMany (Quotient.mk _ m) l : ExtDHashMap α β) = Quotient.mk _ (m.insertMany l) := by
   simp only [Quotient.mk]
   induction l generalizing m with
@@ -940,14 +946,14 @@ private theorem insertMany_list_mk {m : DHashMap α β} {l : List ((a : α) × �
       Quotient.mk', Quotient.mk, Quotient.lift, ih]
 
 @[elab_as_elim]
-theorem insertMany_ind {motive : ExtDHashMap α β → Prop} (m : ExtDHashMap α β) (l : ρ)
+theorem insertMany_ind [EquivBEq α] [LawfulHashable α] {motive : ExtDHashMap α β → Prop} (m : ExtDHashMap α β) (l : ρ)
     (init : motive m) (insert : ∀ m a b, motive m → motive (m.insert a b)) :
     motive (m.insertMany l) := by
   change motive (Subtype.val ?my_mvar)
   exact Subtype.property ?my_mvar motive init (insert _ _ _)
 
 @[simp]
-theorem contains_insertMany_list
+theorem contains_insertMany_list [EquivBEq α] [LawfulHashable α]
     {l : List ((a : α) × β a)} {k : α} :
     (m.insertMany l).contains k = (m.contains k || (l.map Sigma.fst).contains k) := by
   refine m.inductionOn fun _ => ?_
@@ -955,14 +961,14 @@ theorem contains_insertMany_list
   exact DHashMap.contains_insertMany_list
 
 @[simp]
-theorem mem_insertMany_list
+theorem mem_insertMany_list [EquivBEq α] [LawfulHashable α]
     {l : List ((a : α) × β a)} {k : α} :
     k ∈ m.insertMany l ↔ k ∈ m ∨ (l.map Sigma.fst).contains k := by
   refine m.inductionOn fun _ => ?_
   simp only [insertMany_list_mk]
   exact DHashMap.mem_insertMany_list
 
-theorem mem_of_mem_insertMany_list
+theorem mem_of_mem_insertMany_list [EquivBEq α] [LawfulHashable α]
     {l : List ((a : α) × β a)} {k : α} (mem : k ∈ m.insertMany l)
     (contains_eq_false : (l.map Sigma.fst).contains k = false) :
     k ∈ m := by
@@ -970,7 +976,7 @@ theorem mem_of_mem_insertMany_list
   simp only [insertMany_list_mk] at mem
   exact DHashMap.mem_of_mem_insertMany_list mem contains_eq_false
 
-theorem mem_insertMany_of_mem {l : ρ} {k : α} (h' : k ∈ m) : k ∈ m.insertMany l :=
+theorem mem_insertMany_of_mem [EquivBEq α] [LawfulHashable α] {l : ρ} {k : α} (h' : k ∈ m) : k ∈ m.insertMany l :=
   insertMany_ind m l h' fun _ _ _ h => mem_insert.mpr (.inr h)
 
 theorem get?_insertMany_list_of_contains_eq_false [LawfulBEq α]
@@ -1044,7 +1050,7 @@ theorem getD_insertMany_list_of_mem [LawfulBEq α]
   simp only [insertMany_list_mk]
   exact DHashMap.getD_insertMany_list_of_mem k_beq distinct mem
 
-theorem getKey?_insertMany_list_of_contains_eq_false
+theorem getKey?_insertMany_list_of_contains_eq_false [EquivBEq α] [LawfulHashable α]
     {l : List ((a : α) × β a)} {k : α}
     (contains_eq_false : (l.map Sigma.fst).contains k = false) :
     (m.insertMany l).getKey? k = m.getKey? k := by
@@ -1052,7 +1058,7 @@ theorem getKey?_insertMany_list_of_contains_eq_false
   simp only [insertMany_list_mk]
   exact DHashMap.getKey?_insertMany_list_of_contains_eq_false contains_eq_false
 
-theorem getKey?_insertMany_list_of_mem
+theorem getKey?_insertMany_list_of_mem [EquivBEq α] [LawfulHashable α]
     {l : List ((a : α) × β a)}
     {k k' : α} (k_beq : k == k')
     (distinct : l.Pairwise (fun a b => (a.1 == b.1) = false))
@@ -1062,7 +1068,7 @@ theorem getKey?_insertMany_list_of_mem
   simp only [insertMany_list_mk]
   exact DHashMap.getKey?_insertMany_list_of_mem k_beq distinct mem
 
-theorem getKey_insertMany_list_of_contains_eq_false
+theorem getKey_insertMany_list_of_contains_eq_false [EquivBEq α] [LawfulHashable α]
     {l : List ((a : α) × β a)} {k : α}
     (contains_eq_false : (l.map Sigma.fst).contains k = false)
     {h} :
@@ -1072,7 +1078,7 @@ theorem getKey_insertMany_list_of_contains_eq_false
   simp only [insertMany_list_mk]
   exact DHashMap.getKey_insertMany_list_of_contains_eq_false contains_eq_false
 
-theorem getKey_insertMany_list_of_mem
+theorem getKey_insertMany_list_of_mem [EquivBEq α] [LawfulHashable α]
     {l : List ((a : α) × β a)}
     {k k' : α} (k_beq : k == k')
     (distinct : l.Pairwise (fun a b => (a.1 == b.1) = false))
@@ -1083,7 +1089,7 @@ theorem getKey_insertMany_list_of_mem
   simp only [insertMany_list_mk]
   exact DHashMap.getKey_insertMany_list_of_mem k_beq distinct mem
 
-theorem getKey!_insertMany_list_of_contains_eq_false [Inhabited α]
+theorem getKey!_insertMany_list_of_contains_eq_false [EquivBEq α] [LawfulHashable α] [Inhabited α]
     {l : List ((a : α) × β a)} {k : α}
     (contains_eq_false : (l.map Sigma.fst).contains k = false) :
     (m.insertMany l).getKey! k = m.getKey! k := by
@@ -1091,7 +1097,7 @@ theorem getKey!_insertMany_list_of_contains_eq_false [Inhabited α]
   simp only [insertMany_list_mk]
   exact DHashMap.getKey!_insertMany_list_of_contains_eq_false contains_eq_false
 
-theorem getKey!_insertMany_list_of_mem [Inhabited α]
+theorem getKey!_insertMany_list_of_mem [EquivBEq α] [LawfulHashable α] [Inhabited α]
     {l : List ((a : α) × β a)}
     {k k' : α} (k_beq : k == k')
     (distinct : l.Pairwise (fun a b => (a.1 == b.1) = false))
@@ -1101,7 +1107,7 @@ theorem getKey!_insertMany_list_of_mem [Inhabited α]
   simp only [insertMany_list_mk]
   exact DHashMap.getKey!_insertMany_list_of_mem k_beq distinct mem
 
-theorem getKeyD_insertMany_list_of_contains_eq_false
+theorem getKeyD_insertMany_list_of_contains_eq_false [EquivBEq α] [LawfulHashable α]
     {l : List ((a : α) × β a)} {k fallback : α}
     (contains_eq_false : (l.map Sigma.fst).contains k = false) :
     (m.insertMany l).getKeyD k fallback = m.getKeyD k fallback := by
@@ -1109,7 +1115,7 @@ theorem getKeyD_insertMany_list_of_contains_eq_false
   simp only [insertMany_list_mk]
   exact DHashMap.getKeyD_insertMany_list_of_contains_eq_false contains_eq_false
 
-theorem getKeyD_insertMany_list_of_mem
+theorem getKeyD_insertMany_list_of_mem [EquivBEq α] [LawfulHashable α]
     {l : List ((a : α) × β a)}
     {k k' fallback : α} (k_beq : k == k')
     (distinct : l.Pairwise (fun a b => (a.1 == b.1) = false))
@@ -1119,7 +1125,7 @@ theorem getKeyD_insertMany_list_of_mem
   simp only [insertMany_list_mk]
   exact DHashMap.getKeyD_insertMany_list_of_mem k_beq distinct mem
 
-theorem size_insertMany_list
+theorem size_insertMany_list [EquivBEq α] [LawfulHashable α]
     {l : List ((a : α) × β a)} (distinct : l.Pairwise (fun a b => (a.1 == b.1) = false)) :
     (∀ (a : α), a ∈ m → (l.map Sigma.fst).contains a = false) →
       (m.insertMany l).size = m.size + l.length := by
@@ -1127,17 +1133,17 @@ theorem size_insertMany_list
   simp only [insertMany_list_mk]
   exact DHashMap.size_insertMany_list distinct
 
-theorem size_le_size_insertMany_list
+theorem size_le_size_insertMany_list [EquivBEq α] [LawfulHashable α]
     {l : List ((a : α) × β a)} :
     m.size ≤ (m.insertMany l).size := by
   refine m.inductionOn fun _ => ?_
   simp only [insertMany_list_mk]
   exact DHashMap.size_le_size_insertMany_list
 
-theorem size_le_size_insertMany {l : ρ} : m.size ≤ (m.insertMany l).size :=
+theorem size_le_size_insertMany [EquivBEq α] [LawfulHashable α] {l : ρ} : m.size ≤ (m.insertMany l).size :=
   insertMany_ind m l (Nat.le_refl _) fun _ _ _ h => Nat.le_trans h size_le_size_insert
 
-theorem size_insertMany_list_le
+theorem size_insertMany_list_le [EquivBEq α] [LawfulHashable α]
     {l : List ((a : α) × β a)} :
     (m.insertMany l).size ≤ m.size + l.length := by
   refine m.inductionOn fun _ => ?_
@@ -1145,14 +1151,14 @@ theorem size_insertMany_list_le
   exact DHashMap.size_insertMany_list_le
 
 @[simp]
-theorem insertMany_list_eq_empty_iff {l : List ((a : α) × β a)} :
+theorem insertMany_list_eq_empty_iff [EquivBEq α] [LawfulHashable α] {l : List ((a : α) × β a)} :
     m.insertMany l = ∅ ↔ m = ∅ ∧ l = [] := by
   refine m.inductionOn fun _ => ?_
   simp only [insertMany_list_mk, ← isEmpty_iff, ← List.isEmpty_iff,
     Bool.coe_iff_coe, ← Bool.and_eq_true]
   exact DHashMap.isEmpty_insertMany_list
 
-theorem eq_empty_of_insertMany_eq_empty {l : ρ} :
+theorem eq_empty_of_insertMany_eq_empty [EquivBEq α] [LawfulHashable α] {l : ρ} :
     m.insertMany l = ∅ → m = ∅ :=
   insertMany_ind m l id fun _ _ _ _ h => absurd h not_insert_eq_empty
 
@@ -1162,14 +1168,14 @@ variable {β : Type v} {m : ExtDHashMap α (fun _ => β)}
 variable {ρ : Type w} [ForIn Id ρ (α × β)]
 
 @[simp]
-theorem insertMany_nil : insertMany m [] = m :=
+theorem insertMany_nil [EquivBEq α] [LawfulHashable α] : insertMany m [] = m :=
   rfl
 
 @[simp]
-theorem insertMany_list_singleton {k : α} {v : β} :
+theorem insertMany_list_singleton [EquivBEq α] [LawfulHashable α] {k : α} {v : β} :
     insertMany m [⟨k, v⟩] = m.insert k v := rfl
 
-theorem insertMany_cons {l : List (α × β)} {p : α × β} :
+theorem insertMany_cons [EquivBEq α] [LawfulHashable α] {l : List (α × β)} {p : α × β} :
     insertMany m (p :: l) = insertMany (m.insert p.1 p.2) l := by
   rcases p with ⟨k, v⟩
   unfold insertMany
@@ -1178,7 +1184,8 @@ theorem insertMany_cons {l : List (α × β)} {p : α × β} :
   exact (List.foldl_hom (f := Subtype.val) fun x y => rfl).symm
   exact (List.foldl_hom (f := Subtype.val) fun x y => rfl).symm
 
-private theorem insertMany_list_mk {m : DHashMap α fun _ => β} {l : List (α × β)} :
+private theorem insertMany_list_mk [EquivBEq α] [LawfulHashable α]
+    {m : DHashMap α fun _ => β} {l : List (α × β)} :
     (insertMany (Quotient.mk _ m) l : ExtDHashMap α fun _ => β) =
       Quotient.mk _ (DHashMap.Const.insertMany m l) := by
   simp only [Quotient.mk]
@@ -1190,7 +1197,7 @@ private theorem insertMany_list_mk {m : DHashMap α fun _ => β} {l : List (α �
       Quotient.mk', Quotient.mk, Quotient.lift, ih]
 
 @[elab_as_elim]
-theorem insertMany_ind {motive : ExtDHashMap α (fun _ => β) → Prop}
+theorem insertMany_ind [EquivBEq α] [LawfulHashable α] {motive : ExtDHashMap α (fun _ => β) → Prop}
     (m : ExtDHashMap α fun _ => β) (l : ρ)
     (init : motive m) (insert : ∀ m a b, motive m → motive (m.insert a b)) :
     motive (insertMany m l) := by
@@ -1198,7 +1205,7 @@ theorem insertMany_ind {motive : ExtDHashMap α (fun _ => β) → Prop}
   exact Subtype.property ?my_mvar motive init (insert _ _ _)
 
 @[simp]
-theorem contains_insertMany_list
+theorem contains_insertMany_list [EquivBEq α] [LawfulHashable α]
     {l : List (α × β)} {k : α} :
     (Const.insertMany m l).contains k = (m.contains k || (l.map Prod.fst).contains k) := by
   refine m.inductionOn fun _ => ?_
@@ -1206,14 +1213,14 @@ theorem contains_insertMany_list
   exact DHashMap.Const.contains_insertMany_list
 
 @[simp]
-theorem mem_insertMany_list
+theorem mem_insertMany_list [EquivBEq α] [LawfulHashable α]
     {l : List (α × β)} {k : α} :
     k ∈ insertMany m l ↔ k ∈ m ∨ (l.map Prod.fst).contains k := by
   refine m.inductionOn fun _ => ?_
   simp only [insertMany_list_mk]
   exact DHashMap.Const.mem_insertMany_list
 
-theorem mem_of_mem_insertMany_list
+theorem mem_of_mem_insertMany_list [EquivBEq α] [LawfulHashable α]
     {l : List (α × β)} {k : α} (mem : k ∈ insertMany m l)
     (contains_eq_false : (l.map Prod.fst).contains k = false) :
     k ∈ m := by
@@ -1221,10 +1228,10 @@ theorem mem_of_mem_insertMany_list
   simp only [insertMany_list_mk] at mem
   exact DHashMap.Const.mem_of_mem_insertMany_list mem contains_eq_false
 
-theorem mem_insertMany_of_mem {l : ρ} {k : α} (h' : k ∈ m) : k ∈ insertMany m l :=
+theorem mem_insertMany_of_mem [EquivBEq α] [LawfulHashable α] {l : ρ} {k : α} (h' : k ∈ m) : k ∈ insertMany m l :=
   insertMany_ind m l h' fun _ _ _ h => mem_insert.mpr (.inr h)
 
-theorem getKey?_insertMany_list_of_contains_eq_false
+theorem getKey?_insertMany_list_of_contains_eq_false [EquivBEq α] [LawfulHashable α]
     {l : List (α × β)} {k : α}
     (contains_eq_false : (l.map Prod.fst).contains k = false) :
     (insertMany m l).getKey? k = m.getKey? k := by
@@ -1232,7 +1239,7 @@ theorem getKey?_insertMany_list_of_contains_eq_false
   simp only [insertMany_list_mk]
   exact DHashMap.Const.getKey?_insertMany_list_of_contains_eq_false contains_eq_false
 
-theorem getKey?_insertMany_list_of_mem
+theorem getKey?_insertMany_list_of_mem [EquivBEq α] [LawfulHashable α]
     {l : List (α × β)}
     {k k' : α} (k_beq : k == k')
     (distinct : l.Pairwise (fun a b => (a.1 == b.1) = false))
@@ -1242,7 +1249,7 @@ theorem getKey?_insertMany_list_of_mem
   simp only [insertMany_list_mk]
   exact DHashMap.Const.getKey?_insertMany_list_of_mem k_beq distinct mem
 
-theorem getKey_insertMany_list_of_contains_eq_false
+theorem getKey_insertMany_list_of_contains_eq_false [EquivBEq α] [LawfulHashable α]
     {l : List (α × β)} {k : α}
     (contains_eq_false : (l.map Prod.fst).contains k = false)
     {h} :
@@ -1252,7 +1259,7 @@ theorem getKey_insertMany_list_of_contains_eq_false
   simp only [insertMany_list_mk]
   exact DHashMap.Const.getKey_insertMany_list_of_contains_eq_false contains_eq_false
 
-theorem getKey_insertMany_list_of_mem
+theorem getKey_insertMany_list_of_mem [EquivBEq α] [LawfulHashable α]
     {l : List (α × β)}
     {k k' : α} (k_beq : k == k')
     (distinct : l.Pairwise (fun a b => (a.1 == b.1) = false))
@@ -1263,7 +1270,7 @@ theorem getKey_insertMany_list_of_mem
   simp only [insertMany_list_mk]
   exact DHashMap.Const.getKey_insertMany_list_of_mem k_beq distinct mem
 
-theorem getKey!_insertMany_list_of_contains_eq_false [Inhabited α]
+theorem getKey!_insertMany_list_of_contains_eq_false [EquivBEq α] [LawfulHashable α] [Inhabited α]
     {l : List (α × β)} {k : α}
     (contains_eq_false : (l.map Prod.fst).contains k = false) :
     (insertMany m l).getKey! k = m.getKey! k := by
@@ -1271,7 +1278,7 @@ theorem getKey!_insertMany_list_of_contains_eq_false [Inhabited α]
   simp only [insertMany_list_mk]
   exact DHashMap.Const.getKey!_insertMany_list_of_contains_eq_false contains_eq_false
 
-theorem getKey!_insertMany_list_of_mem [Inhabited α]
+theorem getKey!_insertMany_list_of_mem [EquivBEq α] [LawfulHashable α] [Inhabited α]
     {l : List (α × β)}
     {k k' : α} (k_beq : k == k')
     (distinct : l.Pairwise (fun a b => (a.1 == b.1) = false))
@@ -1281,7 +1288,7 @@ theorem getKey!_insertMany_list_of_mem [Inhabited α]
   simp only [insertMany_list_mk]
   exact DHashMap.Const.getKey!_insertMany_list_of_mem k_beq distinct mem
 
-theorem getKeyD_insertMany_list_of_contains_eq_false
+theorem getKeyD_insertMany_list_of_contains_eq_false [EquivBEq α] [LawfulHashable α]
     {l : List (α × β)} {k fallback : α}
     (contains_eq_false : (l.map Prod.fst).contains k = false) :
     (insertMany m l).getKeyD k fallback = m.getKeyD k fallback := by
@@ -1289,7 +1296,7 @@ theorem getKeyD_insertMany_list_of_contains_eq_false
   simp only [insertMany_list_mk]
   exact DHashMap.Const.getKeyD_insertMany_list_of_contains_eq_false contains_eq_false
 
-theorem getKeyD_insertMany_list_of_mem
+theorem getKeyD_insertMany_list_of_mem [EquivBEq α] [LawfulHashable α]
     {l : List (α × β)}
     {k k' fallback : α} (k_beq : k == k')
     (distinct : l.Pairwise (fun a b => (a.1 == b.1) = false))
@@ -1299,7 +1306,7 @@ theorem getKeyD_insertMany_list_of_mem
   simp only [insertMany_list_mk]
   exact DHashMap.Const.getKeyD_insertMany_list_of_mem k_beq distinct mem
 
-theorem size_insertMany_list
+theorem size_insertMany_list [EquivBEq α] [LawfulHashable α]
     {l : List (α × β)}
     (distinct : l.Pairwise (fun a b => (a.1 == b.1) = false)) :
     (∀ (a : α), a ∈ m → (l.map Prod.fst).contains a = false) →
@@ -1308,17 +1315,17 @@ theorem size_insertMany_list
   simp only [insertMany_list_mk]
   exact DHashMap.Const.size_insertMany_list distinct
 
-theorem size_le_size_insertMany_list
+theorem size_le_size_insertMany_list [EquivBEq α] [LawfulHashable α]
     {l : List (α × β)} :
     m.size ≤ (insertMany m l).size := by
   refine m.inductionOn fun _ => ?_
   simp only [insertMany_list_mk]
   exact DHashMap.Const.size_le_size_insertMany_list
 
-theorem size_le_size_insertMany {l : ρ} : m.size ≤ (insertMany m l).size :=
+theorem size_le_size_insertMany [EquivBEq α] [LawfulHashable α] {l : ρ} : m.size ≤ (insertMany m l).size :=
   insertMany_ind m l (Nat.le_refl _) fun _ _ _ h => Nat.le_trans h size_le_size_insert
 
-theorem size_insertMany_list_le
+theorem size_insertMany_list_le [EquivBEq α] [LawfulHashable α]
     {l : List (α × β)} :
     (insertMany m l).size ≤ m.size + l.length := by
   refine m.inductionOn fun _ => ?_
@@ -1326,17 +1333,17 @@ theorem size_insertMany_list_le
   exact DHashMap.Const.size_insertMany_list_le
 
 @[simp]
-theorem insertMany_list_eq_empty_iff {l : List (α × β)} :
+theorem insertMany_list_eq_empty_iff [EquivBEq α] [LawfulHashable α] {l : List (α × β)} :
     insertMany m l = ∅ ↔ m = ∅ ∧ l = [] := by
   refine m.inductionOn fun _ => ?_
   simp only [insertMany_list_mk, ← isEmpty_iff, ← List.isEmpty_iff,
     Bool.coe_iff_coe, ← Bool.and_eq_true]
   exact DHashMap.Const.isEmpty_insertMany_list
 
-theorem eq_empty_of_insertMany_eq_empty {l : ρ} : insertMany m l = ∅ → m = ∅ :=
+theorem eq_empty_of_insertMany_eq_empty [EquivBEq α] [LawfulHashable α] {l : ρ} : insertMany m l = ∅ → m = ∅ :=
   insertMany_ind m l id fun _ _ _ _ h => absurd h not_insert_eq_empty
 
-theorem get?_insertMany_list_of_contains_eq_false
+theorem get?_insertMany_list_of_contains_eq_false [EquivBEq α] [LawfulHashable α]
     {l : List (α × β)} {k : α}
     (contains_eq_false : (l.map Prod.fst).contains k = false) :
     get? (insertMany m l) k = get? m k := by
@@ -1344,7 +1351,7 @@ theorem get?_insertMany_list_of_contains_eq_false
   simp only [insertMany_list_mk]
   exact DHashMap.Const.get?_insertMany_list_of_contains_eq_false contains_eq_false
 
-theorem get?_insertMany_list_of_mem
+theorem get?_insertMany_list_of_mem [EquivBEq α] [LawfulHashable α]
     {l : List (α × β)} {k k' : α} (k_beq : k == k') {v : β}
     (distinct : l.Pairwise (fun a b => (a.1 == b.1) = false)) (mem : ⟨k, v⟩ ∈ l) :
     get? (insertMany m l) k' = some v := by
@@ -1352,7 +1359,7 @@ theorem get?_insertMany_list_of_mem
   simp only [insertMany_list_mk]
   exact DHashMap.Const.get?_insertMany_list_of_mem k_beq distinct mem
 
-theorem get_insertMany_list_of_contains_eq_false
+theorem get_insertMany_list_of_contains_eq_false [EquivBEq α] [LawfulHashable α]
     {l : List (α × β)} {k : α}
     (contains_eq_false : (l.map Prod.fst).contains k = false)
     {h} :
@@ -1361,7 +1368,7 @@ theorem get_insertMany_list_of_contains_eq_false
   simp only [insertMany_list_mk]
   exact DHashMap.Const.get_insertMany_list_of_contains_eq_false contains_eq_false
 
-theorem get_insertMany_list_of_mem
+theorem get_insertMany_list_of_mem [EquivBEq α] [LawfulHashable α]
     {l : List (α × β)} {k k' : α} (k_beq : k == k') {v : β}
     (distinct : l.Pairwise (fun a b => (a.1 == b.1) = false)) (mem : ⟨k, v⟩ ∈ l) {h} :
     get (insertMany m l) k' h = v := by
@@ -1369,7 +1376,7 @@ theorem get_insertMany_list_of_mem
   simp only [insertMany_list_mk]
   exact DHashMap.Const.get_insertMany_list_of_mem k_beq distinct mem
 
-theorem get!_insertMany_list_of_contains_eq_false
+theorem get!_insertMany_list_of_contains_eq_false [EquivBEq α] [LawfulHashable α]
     [Inhabited β] {l : List (α × β)} {k : α}
     (contains_eq_false : (l.map Prod.fst).contains k = false) :
     get! (insertMany m l) k = get! m k := by
@@ -1377,7 +1384,7 @@ theorem get!_insertMany_list_of_contains_eq_false
   simp only [insertMany_list_mk]
   exact DHashMap.Const.get!_insertMany_list_of_contains_eq_false contains_eq_false
 
-theorem get!_insertMany_list_of_mem [Inhabited β]
+theorem get!_insertMany_list_of_mem [EquivBEq α] [LawfulHashable α] [Inhabited β]
     {l : List (α × β)} {k k' : α} (k_beq : k == k') {v : β}
     (distinct : l.Pairwise (fun a b => (a.1 == b.1) = false)) (mem : ⟨k, v⟩ ∈ l) :
     get! (insertMany m l) k' = v := by
@@ -1385,7 +1392,7 @@ theorem get!_insertMany_list_of_mem [Inhabited β]
   simp only [insertMany_list_mk]
   exact DHashMap.Const.get!_insertMany_list_of_mem k_beq distinct mem
 
-theorem getD_insertMany_list_of_contains_eq_false
+theorem getD_insertMany_list_of_contains_eq_false [EquivBEq α] [LawfulHashable α]
     {l : List (α × β)} {k : α} {fallback : β}
     (contains_eq_false : (l.map Prod.fst).contains k = false) :
     getD (insertMany m l) k fallback = getD m k fallback := by
@@ -1393,7 +1400,7 @@ theorem getD_insertMany_list_of_contains_eq_false
   simp only [insertMany_list_mk]
   exact DHashMap.Const.getD_insertMany_list_of_contains_eq_false contains_eq_false
 
-theorem getD_insertMany_list_of_mem
+theorem getD_insertMany_list_of_mem [EquivBEq α] [LawfulHashable α]
     {l : List (α × β)} {k k' : α} (k_beq : k == k') {v fallback : β}
     (distinct : l.Pairwise (fun a b => (a.1 == b.1) = false)) (mem : ⟨k, v⟩ ∈ l) :
     getD (insertMany m l) k' fallback = v := by
@@ -1405,15 +1412,15 @@ variable {m : ExtDHashMap α (fun _ => Unit)}
 variable {ρ : Type w} [ForIn Id ρ α]
 
 @[simp]
-theorem insertManyIfNewUnit_nil :
+theorem insertManyIfNewUnit_nil [EquivBEq α] [LawfulHashable α] :
     insertManyIfNewUnit m [] = m :=
   rfl
 
 @[simp]
-theorem insertManyIfNewUnit_list_singleton {k : α} :
+theorem insertManyIfNewUnit_list_singleton [EquivBEq α] [LawfulHashable α] {k : α} :
     insertManyIfNewUnit m [k] = m.insertIfNew k () := rfl
 
-theorem insertManyIfNewUnit_cons {l : List α} {k : α} :
+theorem insertManyIfNewUnit_cons [EquivBEq α] [LawfulHashable α] {l : List α} {k : α} :
     insertManyIfNewUnit m (k :: l) = insertManyIfNewUnit (m.insertIfNew k ()) l := by
   unfold insertManyIfNewUnit
   simp only [Id.pure_eq, Id.bind_eq, Id.run, List.forIn_yield_eq_foldl, List.foldl_cons]
@@ -1421,7 +1428,8 @@ theorem insertManyIfNewUnit_cons {l : List α} {k : α} :
   exact (List.foldl_hom (f := Subtype.val) fun x y => rfl).symm
   exact (List.foldl_hom (f := Subtype.val) fun x y => rfl).symm
 
-private theorem insertManyIfNewUnit_list_mk {m : DHashMap α fun _ => Unit} {l : List α} :
+private theorem insertManyIfNewUnit_list_mk [EquivBEq α] [LawfulHashable α]
+    {m : DHashMap α fun _ => Unit} {l : List α} :
     (insertManyIfNewUnit (Quotient.mk _ m) l : ExtDHashMap α fun _ => Unit) =
       Quotient.mk _ (DHashMap.Const.insertManyIfNewUnit m l) := by
   simp only [Quotient.mk]
@@ -1432,7 +1440,7 @@ private theorem insertManyIfNewUnit_list_mk {m : DHashMap α fun _ => Unit} {l :
       Quotient.mk', Quotient.mk, Quotient.lift, ih]
 
 @[elab_as_elim]
-theorem insertManyIfNewUnit_ind {motive : ExtDHashMap α (fun _ => Unit) → Prop}
+theorem insertManyIfNewUnit_ind [EquivBEq α] [LawfulHashable α] {motive : ExtDHashMap α (fun _ => Unit) → Prop}
     (m : ExtDHashMap α fun _ => Unit) (l : ρ)
     (init : motive m) (insert : ∀ m a, motive m → motive (m.insertIfNew a ())) :
     motive (insertManyIfNewUnit m l) := by
@@ -1440,7 +1448,7 @@ theorem insertManyIfNewUnit_ind {motive : ExtDHashMap α (fun _ => Unit) → Pro
   exact Subtype.property ?my_mvar motive init (insert _ _)
 
 @[simp]
-theorem contains_insertManyIfNewUnit_list
+theorem contains_insertManyIfNewUnit_list [EquivBEq α] [LawfulHashable α]
     {l : List α} {k : α} :
     (insertManyIfNewUnit m l).contains k = (m.contains k || l.contains k) := by
   refine m.inductionOn fun _ => ?_
@@ -1448,25 +1456,25 @@ theorem contains_insertManyIfNewUnit_list
   exact DHashMap.Const.contains_insertManyIfNewUnit_list
 
 @[simp]
-theorem mem_insertManyIfNewUnit_list
+theorem mem_insertManyIfNewUnit_list [EquivBEq α] [LawfulHashable α]
     {l : List α} {k : α} :
     k ∈ insertManyIfNewUnit m l ↔ k ∈ m ∨ l.contains k := by
   refine m.inductionOn fun _ => ?_
   simp only [insertManyIfNewUnit_list_mk]
   exact DHashMap.Const.mem_insertManyIfNewUnit_list
 
-theorem mem_of_mem_insertManyIfNewUnit_list
+theorem mem_of_mem_insertManyIfNewUnit_list [EquivBEq α] [LawfulHashable α]
     {l : List α} {k : α} (contains_eq_false : l.contains k = false) :
     k ∈ insertManyIfNewUnit m l → k ∈ m := by
   refine m.inductionOn (fun _ contains_eq_false => ?_) contains_eq_false
   simp only [insertManyIfNewUnit_list_mk]
   exact DHashMap.Const.mem_of_mem_insertManyIfNewUnit_list contains_eq_false
 
-theorem mem_insertManyIfNewUnit_of_mem {l : ρ} {k : α} (h : k ∈ m) :
+theorem mem_insertManyIfNewUnit_of_mem [EquivBEq α] [LawfulHashable α] {l : ρ} {k : α} (h : k ∈ m) :
     k ∈ insertManyIfNewUnit m l :=
   insertManyIfNewUnit_ind m l h fun _ _ h => mem_insertIfNew.mpr (.inr h)
 
-theorem getKey?_insertManyIfNewUnit_list_of_not_mem_of_contains_eq_false
+theorem getKey?_insertManyIfNewUnit_list_of_not_mem_of_contains_eq_false [EquivBEq α] [LawfulHashable α]
     {l : List α} {k : α}
     (not_mem : ¬ k ∈ m) (contains_eq_false : l.contains k = false) :
     getKey? (insertManyIfNewUnit m l) k = none := by
@@ -1474,7 +1482,7 @@ theorem getKey?_insertManyIfNewUnit_list_of_not_mem_of_contains_eq_false
   simp only [insertManyIfNewUnit_list_mk]
   exact DHashMap.Const.getKey?_insertManyIfNewUnit_list_of_not_mem_of_contains_eq_false not_mem contains_eq_false
 
-theorem getKey?_insertManyIfNewUnit_list_of_not_mem_of_mem
+theorem getKey?_insertManyIfNewUnit_list_of_not_mem_of_mem [EquivBEq α] [LawfulHashable α]
     {l : List α} {k k' : α} (k_beq : k == k')
     (not_mem : ¬ k ∈ m)
     (distinct : l.Pairwise (fun a b => (a == b) = false)) (mem : k ∈ l) :
@@ -1483,14 +1491,14 @@ theorem getKey?_insertManyIfNewUnit_list_of_not_mem_of_mem
   simp only [insertManyIfNewUnit_list_mk]
   exact DHashMap.Const.getKey?_insertManyIfNewUnit_list_of_not_mem_of_mem k_beq not_mem distinct mem
 
-theorem getKey?_insertManyIfNewUnit_list_of_mem
+theorem getKey?_insertManyIfNewUnit_list_of_mem [EquivBEq α] [LawfulHashable α]
     {l : List α} {k : α} (h' : k ∈ m) :
     getKey? (insertManyIfNewUnit m l) k = getKey? m k := by
   refine m.inductionOn (fun _ h' => ?_) h'
   simp only [insertManyIfNewUnit_list_mk]
   exact DHashMap.Const.getKey?_insertManyIfNewUnit_list_of_mem h'
 
-theorem getKey_insertManyIfNewUnit_list_of_not_mem_of_mem
+theorem getKey_insertManyIfNewUnit_list_of_not_mem_of_mem [EquivBEq α] [LawfulHashable α]
     {l : List α}
     {k k' : α} (k_beq : k == k')
     (not_mem : ¬ k ∈ m) (distinct : l.Pairwise (fun a b => (a == b) = false))
@@ -1500,14 +1508,14 @@ theorem getKey_insertManyIfNewUnit_list_of_not_mem_of_mem
   simp only [insertManyIfNewUnit_list_mk]
   exact DHashMap.Const.getKey_insertManyIfNewUnit_list_of_not_mem_of_mem k_beq not_mem distinct mem
 
-theorem getKey_insertManyIfNewUnit_list_of_mem
+theorem getKey_insertManyIfNewUnit_list_of_mem [EquivBEq α] [LawfulHashable α]
     {l : List α} {k : α} (mem : k ∈ m) {h} :
     getKey (insertManyIfNewUnit m l) k h = getKey m k mem := by
   refine m.inductionOn (fun _ mem _ => ?_) mem h
   simp only [insertManyIfNewUnit_list_mk]
   exact DHashMap.Const.getKey_insertManyIfNewUnit_list_of_mem mem
 
-theorem getKey!_insertManyIfNewUnit_list_of_not_mem_of_contains_eq_false
+theorem getKey!_insertManyIfNewUnit_list_of_not_mem_of_contains_eq_false [EquivBEq α] [LawfulHashable α]
     [Inhabited α] {l : List α} {k : α}
     (not_mem : ¬ k ∈ m) (contains_eq_false : l.contains k = false) :
     getKey! (insertManyIfNewUnit m l) k = default := by
@@ -1515,7 +1523,7 @@ theorem getKey!_insertManyIfNewUnit_list_of_not_mem_of_contains_eq_false
   simp only [insertManyIfNewUnit_list_mk]
   exact DHashMap.Const.getKey!_insertManyIfNewUnit_list_of_not_mem_of_contains_eq_false not_mem contains_eq_false
 
-theorem getKey!_insertManyIfNewUnit_list_of_not_mem_of_mem
+theorem getKey!_insertManyIfNewUnit_list_of_not_mem_of_mem [EquivBEq α] [LawfulHashable α]
     [Inhabited α] {l : List α} {k k' : α} (k_beq : k == k')
     (not_mem : ¬ k ∈ m) (distinct : l.Pairwise (fun a b => (a == b) = false))
     (mem : k ∈ l) :
@@ -1524,14 +1532,14 @@ theorem getKey!_insertManyIfNewUnit_list_of_not_mem_of_mem
   simp only [insertManyIfNewUnit_list_mk]
   exact DHashMap.Const.getKey!_insertManyIfNewUnit_list_of_not_mem_of_mem k_beq not_mem distinct mem
 
-theorem getKey!_insertManyIfNewUnit_list_of_mem
+theorem getKey!_insertManyIfNewUnit_list_of_mem [EquivBEq α] [LawfulHashable α]
     [Inhabited α] {l : List α} {k : α} (mem : k ∈ m) :
     getKey! (insertManyIfNewUnit m l) k = getKey! m k := by
   refine m.inductionOn (fun _ mem => ?_) mem
   simp only [insertManyIfNewUnit_list_mk]
   exact DHashMap.Const.getKey!_insertManyIfNewUnit_list_of_mem mem
 
-theorem getKeyD_insertManyIfNewUnit_list_of_not_mem_of_contains_eq_false
+theorem getKeyD_insertManyIfNewUnit_list_of_not_mem_of_contains_eq_false [EquivBEq α] [LawfulHashable α]
     {l : List α} {k fallback : α}
     (not_mem : ¬ k ∈ m) (contains_eq_false : l.contains k = false) :
     getKeyD (insertManyIfNewUnit m l) k fallback = fallback := by
@@ -1539,7 +1547,7 @@ theorem getKeyD_insertManyIfNewUnit_list_of_not_mem_of_contains_eq_false
   simp only [insertManyIfNewUnit_list_mk]
   exact DHashMap.Const.getKeyD_insertManyIfNewUnit_list_of_not_mem_of_contains_eq_false not_mem contains_eq_false
 
-theorem getKeyD_insertManyIfNewUnit_list_of_not_mem_of_mem
+theorem getKeyD_insertManyIfNewUnit_list_of_not_mem_of_mem [EquivBEq α] [LawfulHashable α]
     {l : List α} {k k' fallback : α} (k_beq : k == k')
     (not_mem : ¬ k ∈ m)
     (distinct : l.Pairwise (fun a b => (a == b) = false)) (mem : k ∈ l) :
@@ -1548,14 +1556,14 @@ theorem getKeyD_insertManyIfNewUnit_list_of_not_mem_of_mem
   simp only [insertManyIfNewUnit_list_mk]
   exact DHashMap.Const.getKeyD_insertManyIfNewUnit_list_of_not_mem_of_mem k_beq not_mem distinct mem
 
-theorem getKeyD_insertManyIfNewUnit_list_of_mem
+theorem getKeyD_insertManyIfNewUnit_list_of_mem [EquivBEq α] [LawfulHashable α]
     {l : List α} {k fallback : α} (mem : k ∈ m) :
     getKeyD (insertManyIfNewUnit m l) k fallback = getKeyD m k fallback := by
   refine m.inductionOn (fun _ mem => ?_) mem
   simp only [insertManyIfNewUnit_list_mk]
   exact DHashMap.Const.getKeyD_insertManyIfNewUnit_list_of_mem mem
 
-theorem size_insertManyIfNewUnit_list
+theorem size_insertManyIfNewUnit_list [EquivBEq α] [LawfulHashable α]
     {l : List α}
     (distinct : l.Pairwise (fun a b => (a == b) = false)) :
     (∀ (a : α), a ∈ m → l.contains a = false) →
@@ -1564,18 +1572,18 @@ theorem size_insertManyIfNewUnit_list
   simp only [insertManyIfNewUnit_list_mk]
   exact DHashMap.Const.size_insertManyIfNewUnit_list distinct
 
-theorem size_le_size_insertManyIfNewUnit_list
+theorem size_le_size_insertManyIfNewUnit_list [EquivBEq α] [LawfulHashable α]
     {l : List α} :
     m.size ≤ (insertManyIfNewUnit m l).size := by
   refine m.inductionOn fun _ => ?_
   simp only [insertManyIfNewUnit_list_mk]
   exact DHashMap.Const.size_le_size_insertManyIfNewUnit_list
 
-theorem size_le_size_insertManyIfNewUnit
+theorem size_le_size_insertManyIfNewUnit [EquivBEq α] [LawfulHashable α]
     {l : ρ} : m.size ≤ (insertManyIfNewUnit m l).size :=
   insertManyIfNewUnit_ind m l (Nat.le_refl _) fun _ _ h => Nat.le_trans h size_le_size_insertIfNew
 
-theorem size_insertManyIfNewUnit_list_le
+theorem size_insertManyIfNewUnit_list_le [EquivBEq α] [LawfulHashable α]
     {l : List α} :
     (insertManyIfNewUnit m l).size ≤ m.size + l.length := by
   refine m.inductionOn fun _ => ?_
@@ -1583,18 +1591,18 @@ theorem size_insertManyIfNewUnit_list_le
   exact DHashMap.Const.size_insertManyIfNewUnit_list_le
 
 @[simp]
-theorem insertManyIfNewUnit_list_eq_empty_iff {l : List α} :
+theorem insertManyIfNewUnit_list_eq_empty_iff [EquivBEq α] [LawfulHashable α] {l : List α} :
     insertManyIfNewUnit m l = ∅ ↔ m = ∅ ∧ l = [] := by
   refine m.inductionOn fun _ => ?_
   simp only [insertManyIfNewUnit_list_mk, ← isEmpty_iff, ← List.isEmpty_iff,
     Bool.coe_iff_coe, ← Bool.and_eq_true]
   exact DHashMap.Const.isEmpty_insertManyIfNewUnit_list
 
-theorem eq_empty_of_insertManyIfNewUnit_eq_empty {l : ρ} :
+theorem eq_empty_of_insertManyIfNewUnit_eq_empty [EquivBEq α] [LawfulHashable α] {l : ρ} :
     insertManyIfNewUnit m l = ∅ → m = ∅ :=
   insertManyIfNewUnit_ind m l id fun _ _ _ h => absurd h not_insertIfNew_eq_empty
 
-theorem get?_insertManyIfNewUnit_list
+theorem get?_insertManyIfNewUnit_list [EquivBEq α] [LawfulHashable α]
     {l : List α} {k : α} :
     get? (insertManyIfNewUnit m l) k =
       if k ∈ m ∨ l.contains k then some () else none := by
@@ -1602,17 +1610,17 @@ theorem get?_insertManyIfNewUnit_list
   simp only [insertManyIfNewUnit_list_mk]
   exact DHashMap.Const.get?_insertManyIfNewUnit_list
 
-theorem get_insertManyIfNewUnit_list
+theorem get_insertManyIfNewUnit_list [EquivBEq α] [LawfulHashable α]
     {l : List α} {k : α} {h} :
     get (insertManyIfNewUnit m l) k h = () :=
   rfl
 
-theorem get!_insertManyIfNewUnit_list
+theorem get!_insertManyIfNewUnit_list [EquivBEq α] [LawfulHashable α]
     {l : List α} {k : α} :
     get! (insertManyIfNewUnit m l) k = () :=
   rfl
 
-theorem getD_insertManyIfNewUnit_list
+theorem getD_insertManyIfNewUnit_list [EquivBEq α] [LawfulHashable α]
     {l : List α} {k : α} {fallback : Unit} :
     getD (insertManyIfNewUnit m l) k fallback = () :=
   rfl
@@ -1626,466 +1634,403 @@ end ExtDHashMap
 namespace ExtDHashMap
 
 @[simp]
-theorem ofList_nil :
+theorem ofList_nil [EquivBEq α] [LawfulHashable α] :
     ofList ([] : List ((a : α) × β a)) = ∅ := rfl
 
 @[simp]
-theorem ofList_singleton {k : α} {v : β k} :
+theorem ofList_singleton [EquivBEq α] [LawfulHashable α] {k : α} {v : β k} :
     ofList [⟨k, v⟩] = (∅ : ExtDHashMap α β).insert k v := rfl
 
-theorem ofList_cons {k : α} {v : β k} {tl : List ((a : α) × β a)} :
-    ofList (⟨k, v⟩ :: tl) = ((∅ : ExtDHashMap α β).insert k v).insertMany tl :=
-  insertMany_cons
-
-private theorem ofList_eq_mk {l : List ((a : α) × β a)} :
-    (ofList l : ExtDHashMap α β) = Quotient.mk _ (DHashMap.ofList l) := by
-  change insertMany (Quotient.mk _ _) _ = _
-  rw [insertMany_list_mk]
-  rfl
+theorem ofList_cons [EquivBEq α] [LawfulHashable α] {k : α} {v : β k} {tl : List ((a : α) × β a)} :
+    ofList (⟨k, v⟩ :: tl) = ((∅ : ExtDHashMap α β).insert k v).insertMany tl := by
+  conv => rhs; apply insertMany_list_mk
+  exact congrArg Quotient.mk' DHashMap.ofList_cons
 
 @[simp]
-theorem contains_ofList
+theorem contains_ofList [EquivBEq α] [LawfulHashable α]
     {l : List ((a : α) × β a)} {k : α} :
-    (ofList l).contains k = (l.map Sigma.fst).contains k := by
-  simp only [ofList_eq_mk]
-  exact DHashMap.contains_ofList
+    (ofList l).contains k = (l.map Sigma.fst).contains k :=
+  DHashMap.contains_ofList
 
 @[simp]
-theorem mem_ofList
+theorem mem_ofList [EquivBEq α] [LawfulHashable α]
     {l : List ((a : α) × β a)} {k : α} :
-    k ∈ ofList l ↔ (l.map Sigma.fst).contains k := by
-  simp only [ofList_eq_mk]
-  exact DHashMap.mem_ofList
+    k ∈ ofList l ↔ (l.map Sigma.fst).contains k :=
+  DHashMap.mem_ofList
 
 theorem get?_ofList_of_contains_eq_false [LawfulBEq α]
     {l : List ((a : α) × β a)} {k : α}
     (contains_eq_false : (l.map Sigma.fst).contains k = false) :
-    (ofList l).get? k = none := by
-  simp only [ofList_eq_mk]
-  exact DHashMap.get?_ofList_of_contains_eq_false contains_eq_false
+    (ofList l).get? k = none :=
+  DHashMap.get?_ofList_of_contains_eq_false contains_eq_false
 
 theorem get?_ofList_of_mem [LawfulBEq α]
     {l : List ((a : α) × β a)} {k k' : α} (k_beq : k == k') {v : β k}
     (distinct : l.Pairwise (fun a b => (a.1 == b.1) = false))
     (mem : ⟨k, v⟩ ∈ l) :
-    (ofList l).get? k' = some (cast (by congr; apply LawfulBEq.eq_of_beq k_beq) v) := by
-  simp only [ofList_eq_mk]
-  exact DHashMap.get?_ofList_of_mem k_beq distinct mem
+    (ofList l).get? k' = some (cast (by congr; apply LawfulBEq.eq_of_beq k_beq) v) :=
+  DHashMap.get?_ofList_of_mem k_beq distinct mem
 
 theorem get_ofList_of_mem [LawfulBEq α]
     {l : List ((a : α) × β a)} {k k' : α} (k_beq : k == k') {v : β k}
     (distinct : l.Pairwise (fun a b => (a.1 == b.1) = false))
     (mem : ⟨k, v⟩ ∈ l)
     {h} :
-    (ofList l).get k' h = cast (by congr; apply LawfulBEq.eq_of_beq k_beq) v := by
-  simp only [ofList_eq_mk]
-  exact DHashMap.get_ofList_of_mem k_beq distinct mem
+    (ofList l).get k' h = cast (by congr; apply LawfulBEq.eq_of_beq k_beq) v :=
+  DHashMap.get_ofList_of_mem k_beq distinct mem
 
 theorem get!_ofList_of_contains_eq_false [LawfulBEq α]
     {l : List ((a : α) × β a)} {k : α} [Inhabited (β k)]
     (contains_eq_false : (l.map Sigma.fst).contains k = false) :
-    (ofList l).get! k = default := by
-  simp only [ofList_eq_mk]
-  exact DHashMap.get!_ofList_of_contains_eq_false contains_eq_false
+    (ofList l).get! k = default :=
+  DHashMap.get!_ofList_of_contains_eq_false contains_eq_false
 
 theorem get!_ofList_of_mem [LawfulBEq α]
     {l : List ((a : α) × β a)} {k k' : α} (k_beq : k == k') {v : β k} [Inhabited (β k')]
     (distinct : l.Pairwise (fun a b => (a.1 == b.1) = false))
     (mem : ⟨k, v⟩ ∈ l) :
-    (ofList l).get! k' = cast (by congr; apply LawfulBEq.eq_of_beq k_beq) v := by
-  simp only [ofList_eq_mk]
-  exact DHashMap.get!_ofList_of_mem k_beq distinct mem
+    (ofList l).get! k' = cast (by congr; apply LawfulBEq.eq_of_beq k_beq) v :=
+  DHashMap.get!_ofList_of_mem k_beq distinct mem
 
 theorem getD_ofList_of_contains_eq_false [LawfulBEq α]
     {l : List ((a : α) × β a)} {k : α} {fallback : β k}
     (contains_eq_false : (l.map Sigma.fst).contains k = false) :
-    (ofList l).getD k fallback = fallback := by
-  simp only [ofList_eq_mk]
-  exact DHashMap.getD_ofList_of_contains_eq_false contains_eq_false
+    (ofList l).getD k fallback = fallback :=
+  DHashMap.getD_ofList_of_contains_eq_false contains_eq_false
 
 theorem getD_ofList_of_mem [LawfulBEq α]
     {l : List ((a : α) × β a)} {k k' : α} (k_beq : k == k') {v : β k} {fallback : β k'}
     (distinct : l.Pairwise (fun a b => (a.1 == b.1) = false))
     (mem : ⟨k, v⟩ ∈ l) :
-    (ofList l).getD k' fallback = cast (by congr; apply LawfulBEq.eq_of_beq k_beq) v := by
-  simp only [ofList_eq_mk]
-  exact DHashMap.getD_ofList_of_mem k_beq distinct mem
+    (ofList l).getD k' fallback = cast (by congr; apply LawfulBEq.eq_of_beq k_beq) v :=
+  DHashMap.getD_ofList_of_mem k_beq distinct mem
 
-theorem getKey?_ofList_of_contains_eq_false
+theorem getKey?_ofList_of_contains_eq_false [EquivBEq α] [LawfulHashable α]
     {l : List ((a : α) × β a)} {k : α}
     (contains_eq_false : (l.map Sigma.fst).contains k = false) :
-    (ofList l).getKey? k = none := by
-  simp only [ofList_eq_mk]
-  exact DHashMap.getKey?_ofList_of_contains_eq_false contains_eq_false
+    (ofList l).getKey? k = none :=
+  DHashMap.getKey?_ofList_of_contains_eq_false contains_eq_false
 
-theorem getKey?_ofList_of_mem
+theorem getKey?_ofList_of_mem [EquivBEq α] [LawfulHashable α]
     {l : List ((a : α) × β a)}
     {k k' : α} (k_beq : k == k')
     (distinct : l.Pairwise (fun a b => (a.1 == b.1) = false))
     (mem : k ∈ l.map Sigma.fst) :
-    (ofList l).getKey? k' = some k := by
-  simp only [ofList_eq_mk]
-  exact DHashMap.getKey?_ofList_of_mem k_beq distinct mem
+    (ofList l).getKey? k' = some k :=
+  DHashMap.getKey?_ofList_of_mem k_beq distinct mem
 
-theorem getKey_ofList_of_mem
+theorem getKey_ofList_of_mem [EquivBEq α] [LawfulHashable α]
     {l : List ((a : α) × β a)}
     {k k' : α} (k_beq : k == k')
     (distinct : l.Pairwise (fun a b => (a.1 == b.1) = false))
     (mem : k ∈ l.map Sigma.fst)
     {h} :
-    (ofList l).getKey k' h = k := by
-  simp only [ofList_eq_mk]
-  exact DHashMap.getKey_ofList_of_mem k_beq distinct mem
+    (ofList l).getKey k' h = k :=
+  DHashMap.getKey_ofList_of_mem k_beq distinct mem
 
-theorem getKey!_ofList_of_contains_eq_false [Inhabited α]
+theorem getKey!_ofList_of_contains_eq_false [EquivBEq α] [LawfulHashable α] [Inhabited α]
     {l : List ((a : α) × β a)} {k : α}
     (contains_eq_false : (l.map Sigma.fst).contains k = false) :
-    (ofList l).getKey! k = default := by
-  simp only [ofList_eq_mk]
-  exact DHashMap.getKey!_ofList_of_contains_eq_false contains_eq_false
+    (ofList l).getKey! k = default :=
+  DHashMap.getKey!_ofList_of_contains_eq_false contains_eq_false
 
-theorem getKey!_ofList_of_mem [Inhabited α]
+theorem getKey!_ofList_of_mem [EquivBEq α] [LawfulHashable α] [Inhabited α]
     {l : List ((a : α) × β a)}
     {k k' : α} (k_beq : k == k')
     (distinct : l.Pairwise (fun a b => (a.1 == b.1) = false))
     (mem : k ∈ l.map Sigma.fst) :
-    (ofList l).getKey! k' = k := by
-  simp only [ofList_eq_mk]
-  exact DHashMap.getKey!_ofList_of_mem k_beq distinct mem
+    (ofList l).getKey! k' = k :=
+  DHashMap.getKey!_ofList_of_mem k_beq distinct mem
 
-theorem getKeyD_ofList_of_contains_eq_false
+theorem getKeyD_ofList_of_contains_eq_false [EquivBEq α] [LawfulHashable α]
     {l : List ((a : α) × β a)} {k fallback : α}
     (contains_eq_false : (l.map Sigma.fst).contains k = false) :
-    (ofList l).getKeyD k fallback = fallback := by
-  simp only [ofList_eq_mk]
-  exact DHashMap.getKeyD_ofList_of_contains_eq_false contains_eq_false
+    (ofList l).getKeyD k fallback = fallback :=
+  DHashMap.getKeyD_ofList_of_contains_eq_false contains_eq_false
 
-theorem getKeyD_ofList_of_mem
+theorem getKeyD_ofList_of_mem [EquivBEq α] [LawfulHashable α]
     {l : List ((a : α) × β a)}
     {k k' fallback : α} (k_beq : k == k')
     (distinct : l.Pairwise (fun a b => (a.1 == b.1) = false))
     (mem : k ∈ l.map Sigma.fst) :
-    (ofList l).getKeyD k' fallback = k := by
-  simp only [ofList_eq_mk]
-  exact DHashMap.getKeyD_ofList_of_mem k_beq distinct mem
+    (ofList l).getKeyD k' fallback = k :=
+  DHashMap.getKeyD_ofList_of_mem k_beq distinct mem
 
-theorem size_ofList
+theorem size_ofList [EquivBEq α] [LawfulHashable α]
     {l : List ((a : α) × β a)} (distinct : l.Pairwise (fun a b => (a.1 == b.1) = false)) :
-    (ofList l).size = l.length := by
-  simp only [ofList_eq_mk]
-  exact DHashMap.size_ofList distinct
+    (ofList l).size = l.length :=
+  DHashMap.size_ofList distinct
 
-theorem size_ofList_le
+theorem size_ofList_le [EquivBEq α] [LawfulHashable α]
     {l : List ((a : α) × β a)} :
-    (ofList l).size ≤ l.length := by
-  simp only [ofList_eq_mk]
-  exact DHashMap.size_ofList_le
+    (ofList l).size ≤ l.length :=
+  DHashMap.size_ofList_le
 
 @[simp]
-theorem ofList_eq_empty_iff {l : List ((a : α) × β a)} :
+theorem ofList_eq_empty_iff [EquivBEq α] [LawfulHashable α] {l : List ((a : α) × β a)} :
     ofList l = ∅ ↔ l = [] := by
-  simp only [ofList_eq_mk, ← isEmpty_iff, ← List.isEmpty_iff, Bool.coe_iff_coe]
-  exact DHashMap.isEmpty_ofList
+  simpa only [← isEmpty_iff, ← List.isEmpty_iff, Bool.coe_iff_coe] using
+    DHashMap.isEmpty_ofList
 
 namespace Const
 
 variable {β : Type v}
 
 @[simp]
-theorem ofList_nil :
+theorem ofList_nil [EquivBEq α] [LawfulHashable α] :
     ofList ([] : List (α × β)) = ∅ :=
   rfl
 
 @[simp]
-theorem ofList_singleton {k : α} {v : β} :
+theorem ofList_singleton [EquivBEq α] [LawfulHashable α] {k : α} {v : β} :
     ofList [⟨k, v⟩] = (∅ : ExtDHashMap α (fun _ => β)).insert k v :=
   rfl
 
-theorem ofList_cons {k : α} {v : β} {tl : List (α × β)} :
-    ofList (⟨k, v⟩ :: tl) = insertMany ((∅ : ExtDHashMap α (fun _ => β)).insert k v) tl :=
-  insertMany_cons
-
-private theorem ofList_eq_mk {l : List (α × β)} :
-    (ofList l : ExtDHashMap α fun _ => β) = Quotient.mk _ (DHashMap.Const.ofList l) := by
-  change insertMany (Quotient.mk _ _) _ = _
-  rw [insertMany_list_mk]
-  rfl
+theorem ofList_cons [EquivBEq α] [LawfulHashable α] {k : α} {v : β} {tl : List (α × β)} :
+    ofList (⟨k, v⟩ :: tl) = insertMany ((∅ : ExtDHashMap α (fun _ => β)).insert k v) tl := by
+  conv => rhs; apply insertMany_list_mk
+  exact congrArg Quotient.mk' DHashMap.Const.ofList_cons
 
 @[simp]
-theorem contains_ofList
+theorem contains_ofList [EquivBEq α] [LawfulHashable α]
     {l : List (α × β)} {k : α} :
-    (ofList l).contains k = (l.map Prod.fst).contains k := by
-  simp only [ofList_eq_mk]
-  exact DHashMap.Const.contains_ofList
+    (ofList l).contains k = (l.map Prod.fst).contains k :=
+  DHashMap.Const.contains_ofList
 
 @[simp]
-theorem mem_ofList
+theorem mem_ofList [EquivBEq α] [LawfulHashable α]
     {l : List (α × β)} {k : α} :
-    k ∈ ofList l ↔ (l.map Prod.fst).contains k := by
-  simp only [ofList_eq_mk]
-  exact DHashMap.Const.mem_ofList
+    k ∈ ofList l ↔ (l.map Prod.fst).contains k :=
+  DHashMap.Const.mem_ofList
 
-theorem get?_ofList_of_contains_eq_false
+theorem get?_ofList_of_contains_eq_false [EquivBEq α] [LawfulHashable α]
     {l : List (α × β)} {k : α}
     (contains_eq_false : (l.map Prod.fst).contains k = false) :
-    get? (ofList l) k = none := by
-  simp only [ofList_eq_mk]
-  exact DHashMap.Const.get?_ofList_of_contains_eq_false contains_eq_false
+    get? (ofList l) k = none :=
+  DHashMap.Const.get?_ofList_of_contains_eq_false contains_eq_false
 
-theorem get?_ofList_of_mem
+theorem get?_ofList_of_mem [EquivBEq α] [LawfulHashable α]
     {l : List (α × β)} {k k' : α} (k_beq : k == k') {v : β}
     (distinct : l.Pairwise (fun a b => (a.1 == b.1) = false))
     (mem : ⟨k, v⟩ ∈ l) :
-    get? (ofList l) k' = some v := by
-  simp only [ofList_eq_mk]
-  exact DHashMap.Const.get?_ofList_of_mem k_beq distinct mem
+    get? (ofList l) k' = some v :=
+  DHashMap.Const.get?_ofList_of_mem k_beq distinct mem
 
-theorem get_ofList_of_mem
+theorem get_ofList_of_mem [EquivBEq α] [LawfulHashable α]
     {l : List (α × β)} {k k' : α} (k_beq : k == k') {v : β}
     (distinct : l.Pairwise (fun a b => (a.1 == b.1) = false))
     (mem : ⟨k, v⟩ ∈ l)
     {h} :
-    get (ofList l) k' h = v := by
-  simp only [ofList_eq_mk]
-  exact DHashMap.Const.get_ofList_of_mem k_beq distinct mem
+    get (ofList l) k' h = v :=
+  DHashMap.Const.get_ofList_of_mem k_beq distinct mem
 
-theorem get!_ofList_of_contains_eq_false
+theorem get!_ofList_of_contains_eq_false [EquivBEq α] [LawfulHashable α]
     {l : List (α × β)} {k : α} [Inhabited β]
     (contains_eq_false : (l.map Prod.fst).contains k = false) :
-    get! (ofList l) k = (default : β) := by
-  simp only [ofList_eq_mk]
-  exact DHashMap.Const.get!_ofList_of_contains_eq_false contains_eq_false
+    get! (ofList l) k = (default : β) :=
+  DHashMap.Const.get!_ofList_of_contains_eq_false contains_eq_false
 
-theorem get!_ofList_of_mem
+theorem get!_ofList_of_mem [EquivBEq α] [LawfulHashable α]
     {l : List (α × β)} {k k' : α} (k_beq : k == k') {v : β} [Inhabited β]
     (distinct : l.Pairwise (fun a b => (a.1 == b.1) = false))
     (mem : ⟨k, v⟩ ∈ l) :
-    get! (ofList l) k' = v := by
-  simp only [ofList_eq_mk]
-  exact DHashMap.Const.get!_ofList_of_mem k_beq distinct mem
+    get! (ofList l) k' = v :=
+  DHashMap.Const.get!_ofList_of_mem k_beq distinct mem
 
-theorem getD_ofList_of_contains_eq_false
+theorem getD_ofList_of_contains_eq_false [EquivBEq α] [LawfulHashable α]
     {l : List (α × β)} {k : α} {fallback : β}
     (contains_eq_false : (l.map Prod.fst).contains k = false) :
-    getD (ofList l) k fallback = fallback := by
-  simp only [ofList_eq_mk]
-  exact DHashMap.Const.getD_ofList_of_contains_eq_false contains_eq_false
+    getD (ofList l) k fallback = fallback :=
+  DHashMap.Const.getD_ofList_of_contains_eq_false contains_eq_false
 
-theorem getD_ofList_of_mem
+theorem getD_ofList_of_mem [EquivBEq α] [LawfulHashable α]
     {l : List (α × β)} {k k' : α} (k_beq : k == k') {v : β} {fallback : β}
     (distinct : l.Pairwise (fun a b => (a.1 == b.1) = false))
     (mem : ⟨k, v⟩ ∈ l) :
-    getD (ofList l) k' fallback = v := by
-  simp only [ofList_eq_mk]
-  exact DHashMap.Const.getD_ofList_of_mem k_beq distinct mem
+    getD (ofList l) k' fallback = v :=
+  DHashMap.Const.getD_ofList_of_mem k_beq distinct mem
 
-theorem getKey?_ofList_of_contains_eq_false
+theorem getKey?_ofList_of_contains_eq_false [EquivBEq α] [LawfulHashable α]
     {l : List (α × β)} {k : α}
     (contains_eq_false : (l.map Prod.fst).contains k = false) :
-    (ofList l).getKey? k = none := by
-  simp only [ofList_eq_mk]
-  exact DHashMap.Const.getKey?_ofList_of_contains_eq_false contains_eq_false
+    (ofList l).getKey? k = none :=
+  DHashMap.Const.getKey?_ofList_of_contains_eq_false contains_eq_false
 
-theorem getKey?_ofList_of_mem
+theorem getKey?_ofList_of_mem [EquivBEq α] [LawfulHashable α]
     {l : List (α × β)}
     {k k' : α} (k_beq : k == k')
     (distinct : l.Pairwise (fun a b => (a.1 == b.1) = false))
     (mem : k ∈ l.map Prod.fst) :
-    (ofList l).getKey? k' = some k := by
-  simp only [ofList_eq_mk]
-  exact DHashMap.Const.getKey?_ofList_of_mem k_beq distinct mem
+    (ofList l).getKey? k' = some k :=
+  DHashMap.Const.getKey?_ofList_of_mem k_beq distinct mem
 
-theorem getKey_ofList_of_mem
+theorem getKey_ofList_of_mem [EquivBEq α] [LawfulHashable α]
     {l : List (α × β)}
     {k k' : α} (k_beq : k == k')
     (distinct : l.Pairwise (fun a b => (a.1 == b.1) = false))
     (mem : k ∈ l.map Prod.fst)
     {h} :
-    (ofList l).getKey k' h = k := by
-  simp only [ofList_eq_mk]
-  exact DHashMap.Const.getKey_ofList_of_mem k_beq distinct mem
+    (ofList l).getKey k' h = k :=
+  DHashMap.Const.getKey_ofList_of_mem k_beq distinct mem
 
-theorem getKey!_ofList_of_contains_eq_false
+theorem getKey!_ofList_of_contains_eq_false [EquivBEq α] [LawfulHashable α]
     [Inhabited α] {l : List (α × β)} {k : α}
     (contains_eq_false : (l.map Prod.fst).contains k = false) :
-    (ofList l).getKey! k = default := by
-  simp only [ofList_eq_mk]
-  exact DHashMap.Const.getKey!_ofList_of_contains_eq_false contains_eq_false
+    (ofList l).getKey! k = default :=
+  DHashMap.Const.getKey!_ofList_of_contains_eq_false contains_eq_false
 
-theorem getKey!_ofList_of_mem [Inhabited α]
+theorem getKey!_ofList_of_mem [EquivBEq α] [LawfulHashable α] [Inhabited α]
     {l : List (α × β)}
     {k k' : α} (k_beq : k == k')
     (distinct : l.Pairwise (fun a b => (a.1 == b.1) = false))
     (mem : k ∈ l.map Prod.fst) :
-    (ofList l).getKey! k' = k := by
-  simp only [ofList_eq_mk]
-  exact DHashMap.Const.getKey!_ofList_of_mem k_beq distinct mem
+    (ofList l).getKey! k' = k :=
+  DHashMap.Const.getKey!_ofList_of_mem k_beq distinct mem
 
-theorem getKeyD_ofList_of_contains_eq_false
+theorem getKeyD_ofList_of_contains_eq_false [EquivBEq α] [LawfulHashable α]
     {l : List (α × β)} {k fallback : α}
     (contains_eq_false : (l.map Prod.fst).contains k = false) :
-    (ofList l).getKeyD k fallback = fallback := by
-  simp only [ofList_eq_mk]
-  exact DHashMap.Const.getKeyD_ofList_of_contains_eq_false contains_eq_false
+    (ofList l).getKeyD k fallback = fallback :=
+  DHashMap.Const.getKeyD_ofList_of_contains_eq_false contains_eq_false
 
-theorem getKeyD_ofList_of_mem
+theorem getKeyD_ofList_of_mem [EquivBEq α] [LawfulHashable α]
     {l : List (α × β)}
     {k k' fallback : α} (k_beq : k == k')
     (distinct : l.Pairwise (fun a b => (a.1 == b.1) = false))
     (mem : k ∈ l.map Prod.fst) :
-    (ofList l).getKeyD k' fallback = k := by
-  simp only [ofList_eq_mk]
-  exact DHashMap.Const.getKeyD_ofList_of_mem k_beq distinct mem
+    (ofList l).getKeyD k' fallback = k :=
+  DHashMap.Const.getKeyD_ofList_of_mem k_beq distinct mem
 
-theorem size_ofList
+theorem size_ofList [EquivBEq α] [LawfulHashable α]
     {l : List (α × β)} (distinct : l.Pairwise (fun a b => (a.1 == b.1) = false)) :
-    (ofList l).size = l.length := by
-  simp only [ofList_eq_mk]
-  exact DHashMap.Const.size_ofList distinct
+    (ofList l).size = l.length :=
+  DHashMap.Const.size_ofList distinct
 
-theorem size_ofList_le
+theorem size_ofList_le [EquivBEq α] [LawfulHashable α]
     {l : List (α × β)} :
-    (ofList l).size ≤ l.length := by
-  simp only [ofList_eq_mk]
-  exact DHashMap.Const.size_ofList_le
+    (ofList l).size ≤ l.length :=
+  DHashMap.Const.size_ofList_le
 
 @[simp]
-theorem ofList_eq_empty_iff {l : List (α × β)} :
+theorem ofList_eq_empty_iff [EquivBEq α] [LawfulHashable α] {l : List (α × β)} :
     ofList l = ∅ ↔ l = [] := by
-  simp only [ofList_eq_mk, ← isEmpty_iff, ← List.isEmpty_iff, Bool.coe_iff_coe]
-  exact DHashMap.Const.isEmpty_ofList
+  simpa only [← isEmpty_iff, ← List.isEmpty_iff, Bool.coe_iff_coe] using
+    DHashMap.Const.isEmpty_ofList
 
 @[simp]
-theorem unitOfList_nil :
+theorem unitOfList_nil [EquivBEq α] [LawfulHashable α] :
     unitOfList ([] : List α) = ∅ :=
-  rfl
+  congrArg Quotient.mk' DHashMap.Const.unitOfList_nil
 
 @[simp]
-theorem unitOfList_singleton {k : α} :
+theorem unitOfList_singleton [EquivBEq α] [LawfulHashable α] {k : α} :
     unitOfList [k] = (∅ : ExtDHashMap α (fun _ => Unit)).insertIfNew k () :=
-  rfl
+  congrArg Quotient.mk' DHashMap.Const.unitOfList_singleton
 
-theorem unitOfList_cons {hd : α} {tl : List α} :
+theorem unitOfList_cons [EquivBEq α] [LawfulHashable α] {hd : α} {tl : List α} :
     unitOfList (hd :: tl) =
-      insertManyIfNewUnit ((∅ : ExtDHashMap α (fun _ => Unit)).insertIfNew hd ()) tl :=
-  insertManyIfNewUnit_cons
-
-private theorem unitOfList_eq_mk {l : List α} :
-    (unitOfList l : ExtDHashMap α fun _ => Unit) = Quotient.mk _ (DHashMap.Const.unitOfList l) := by
-  change insertManyIfNewUnit (Quotient.mk _ _) _ = _
-  rw [insertManyIfNewUnit_list_mk]
-  rfl
+      insertManyIfNewUnit ((∅ : ExtDHashMap α (fun _ => Unit)).insertIfNew hd ()) tl := by
+  conv => rhs; apply insertManyIfNewUnit_list_mk
+  exact congrArg Quotient.mk' DHashMap.Const.unitOfList_cons
 
 @[simp]
-theorem contains_unitOfList
+theorem contains_unitOfList [EquivBEq α] [LawfulHashable α]
     {l : List α} {k : α} :
-    (unitOfList l).contains k = l.contains k := by
-  simp only [unitOfList_eq_mk]
-  exact DHashMap.Const.contains_unitOfList
+    (unitOfList l).contains k = l.contains k :=
+  DHashMap.Const.contains_unitOfList
 
 @[simp]
-theorem mem_unitOfList
+theorem mem_unitOfList [EquivBEq α] [LawfulHashable α]
     {l : List α} {k : α} :
-    k ∈ unitOfList l ↔ l.contains k := by
-  simp only [unitOfList_eq_mk]
-  exact DHashMap.Const.mem_unitOfList
+    k ∈ unitOfList l ↔ l.contains k :=
+  DHashMap.Const.mem_unitOfList
 
-theorem getKey?_unitOfList_of_contains_eq_false
+theorem getKey?_unitOfList_of_contains_eq_false [EquivBEq α] [LawfulHashable α]
     {l : List α} {k : α} (contains_eq_false : l.contains k = false) :
-    getKey? (unitOfList l) k = none := by
-  simp only [unitOfList_eq_mk]
-  exact DHashMap.Const.getKey?_unitOfList_of_contains_eq_false contains_eq_false
+    getKey? (unitOfList l) k = none :=
+  DHashMap.Const.getKey?_unitOfList_of_contains_eq_false contains_eq_false
 
-theorem getKey?_unitOfList_of_mem
+theorem getKey?_unitOfList_of_mem [EquivBEq α] [LawfulHashable α]
     {l : List α} {k k' : α} (k_beq : k == k')
     (distinct : l.Pairwise (fun a b => (a == b) = false)) (mem : k ∈ l) :
-    getKey? (unitOfList l) k' = some k := by
-  simp only [unitOfList_eq_mk]
-  exact DHashMap.Const.getKey?_unitOfList_of_mem k_beq distinct mem
+    getKey? (unitOfList l) k' = some k :=
+  DHashMap.Const.getKey?_unitOfList_of_mem k_beq distinct mem
 
-theorem getKey_unitOfList_of_mem
+theorem getKey_unitOfList_of_mem [EquivBEq α] [LawfulHashable α]
     {l : List α}
     {k k' : α} (k_beq : k == k')
     (distinct : l.Pairwise (fun a b => (a == b) = false))
     (mem : k ∈ l) {h} :
-    getKey (unitOfList l) k' h = k := by
-  simp only [unitOfList_eq_mk]
-  exact DHashMap.Const.getKey_unitOfList_of_mem k_beq distinct mem
+    getKey (unitOfList l) k' h = k :=
+  DHashMap.Const.getKey_unitOfList_of_mem k_beq distinct mem
 
-theorem getKey!_unitOfList_of_contains_eq_false
+theorem getKey!_unitOfList_of_contains_eq_false [EquivBEq α] [LawfulHashable α]
     [Inhabited α] {l : List α} {k : α}
     (contains_eq_false : l.contains k = false) :
-    getKey! (unitOfList l) k = default := by
-  simp only [unitOfList_eq_mk]
-  exact DHashMap.Const.getKey!_unitOfList_of_contains_eq_false contains_eq_false
+    getKey! (unitOfList l) k = default :=
+  DHashMap.Const.getKey!_unitOfList_of_contains_eq_false contains_eq_false
 
-theorem getKey!_unitOfList_of_mem
+theorem getKey!_unitOfList_of_mem [EquivBEq α] [LawfulHashable α]
     [Inhabited α] {l : List α} {k k' : α} (k_beq : k == k')
     (distinct : l.Pairwise (fun a b => (a == b) = false))
     (mem : k ∈ l) :
-    getKey! (unitOfList l) k' = k := by
-  simp only [unitOfList_eq_mk]
-  exact DHashMap.Const.getKey!_unitOfList_of_mem k_beq distinct mem
+    getKey! (unitOfList l) k' = k :=
+  DHashMap.Const.getKey!_unitOfList_of_mem k_beq distinct mem
 
-theorem getKeyD_unitOfList_of_contains_eq_false
+theorem getKeyD_unitOfList_of_contains_eq_false [EquivBEq α] [LawfulHashable α]
     {l : List α} {k fallback : α}
     (contains_eq_false : l.contains k = false) :
-    getKeyD (unitOfList l) k fallback = fallback := by
-  simp only [unitOfList_eq_mk]
-  exact DHashMap.Const.getKeyD_unitOfList_of_contains_eq_false contains_eq_false
+    getKeyD (unitOfList l) k fallback = fallback :=
+  DHashMap.Const.getKeyD_unitOfList_of_contains_eq_false contains_eq_false
 
-theorem getKeyD_unitOfList_of_mem
+theorem getKeyD_unitOfList_of_mem [EquivBEq α] [LawfulHashable α]
     {l : List α} {k k' fallback : α} (k_beq : k == k')
     (distinct : l.Pairwise (fun a b => (a == b) = false))
     (mem : k ∈ l) :
-    getKeyD (unitOfList l) k' fallback = k := by
-  simp only [unitOfList_eq_mk]
-  exact DHashMap.Const.getKeyD_unitOfList_of_mem k_beq distinct mem
+    getKeyD (unitOfList l) k' fallback = k :=
+  DHashMap.Const.getKeyD_unitOfList_of_mem k_beq distinct mem
 
-theorem size_unitOfList
+theorem size_unitOfList [EquivBEq α] [LawfulHashable α]
     {l : List α}
     (distinct : l.Pairwise (fun a b => (a == b) = false)) :
-    (unitOfList l).size = l.length := by
-  simp only [unitOfList_eq_mk]
-  exact DHashMap.Const.size_unitOfList distinct
+    (unitOfList l).size = l.length :=
+  DHashMap.Const.size_unitOfList distinct
 
-theorem size_unitOfList_le
+theorem size_unitOfList_le [EquivBEq α] [LawfulHashable α]
     {l : List α} :
-    (unitOfList l).size ≤ l.length := by
-  simp only [unitOfList_eq_mk]
-  exact DHashMap.Const.size_unitOfList_le
+    (unitOfList l).size ≤ l.length :=
+  DHashMap.Const.size_unitOfList_le
 
 @[simp]
-theorem unitOfList_eq_empty_iff {l : List α} :
+theorem unitOfList_eq_empty_iff [EquivBEq α] [LawfulHashable α] {l : List α} :
     unitOfList l = ∅ ↔ l = [] := by
-  simp only [unitOfList_eq_mk, ← isEmpty_iff, ← List.isEmpty_iff, Bool.coe_iff_coe]
-  exact DHashMap.Const.isEmpty_unitOfList
+  simpa only [← isEmpty_iff, ← List.isEmpty_iff, Bool.coe_iff_coe] using
+    DHashMap.Const.isEmpty_unitOfList
 
 @[simp]
-theorem get?_unitOfList
+theorem get?_unitOfList [EquivBEq α] [LawfulHashable α]
     {l : List α} {k : α} :
     get? (unitOfList l) k =
-    if l.contains k then some () else none := by
-  simp only [unitOfList_eq_mk]
-  exact DHashMap.Const.get?_unitOfList
+    if l.contains k then some () else none :=
+  DHashMap.Const.get?_unitOfList
 
 @[simp]
-theorem get_unitOfList
+theorem get_unitOfList [EquivBEq α] [LawfulHashable α]
     {l : List α} {k : α} {h} :
     get (unitOfList l) k h = () :=
-  rfl
+  DHashMap.Const.get_unitOfList
 
 @[simp]
-theorem get!_unitOfList
+theorem get!_unitOfList [EquivBEq α] [LawfulHashable α]
     {l : List α} {k : α} :
     get! (unitOfList l) k = () :=
-  rfl
+  DHashMap.Const.get!_unitOfList
 
 @[simp]
-theorem getD_unitOfList
+theorem getD_unitOfList [EquivBEq α] [LawfulHashable α]
     {l : List α} {k : α} {fallback : Unit} :
     getD (unitOfList l) k fallback = () :=
-  rfl
+  DHashMap.Const.getD_unitOfList
 
 end Const
 
@@ -2286,7 +2231,7 @@ namespace Const
 
 variable {β : Type v} {m : ExtDHashMap α (fun _ => β)}
 
-theorem alter_eq_empty_iff_erase_eq_empty {k : α} {f : Option β → Option β} :
+theorem alter_eq_empty_iff_erase_eq_empty [EquivBEq α] [LawfulHashable α] {k : α} {f : Option β → Option β} :
     alter m k f = ∅ ↔ m.erase k = ∅ ∧ f (get? m k) = none := by
   rcases m with ⟨m⟩
   simp only [← isEmpty_iff]
@@ -2296,43 +2241,43 @@ theorem alter_eq_empty_iff_erase_eq_empty {k : α} {f : Option β → Option β}
   rfl
 
 @[simp]
-theorem alter_eq_empty_iff {k : α} {f : Option β → Option β} :
+theorem alter_eq_empty_iff [EquivBEq α] [LawfulHashable α] {k : α} {f : Option β → Option β} :
     alter m k f = ∅ ↔ (m = ∅ ∨ (m.size = 1 ∧ k ∈ m)) ∧ f (get? m k) = none := by
   simp only [alter_eq_empty_iff_erase_eq_empty, erase_eq_empty_iff]
 
-theorem contains_alter {k k': α} {f : Option β → Option β} :
+theorem contains_alter [EquivBEq α] [LawfulHashable α] {k k': α} {f : Option β → Option β} :
     (Const.alter m k f).contains k' =
       if k == k' then (f (Const.get? m k)).isSome else m.contains k' :=
   m.inductionOn fun _ => DHashMap.Const.contains_alter
 
-theorem mem_alter {k k': α} {f : Option β → Option β} :
+theorem mem_alter [EquivBEq α] [LawfulHashable α] {k k': α} {f : Option β → Option β} :
     k' ∈ Const.alter m k f ↔ if k == k' then (f (Const.get? m k)).isSome = true else k' ∈ m :=
   m.inductionOn fun _ => DHashMap.Const.mem_alter
 
-theorem mem_alter_of_beq {k k': α} {f : Option β → Option β}
+theorem mem_alter_of_beq [EquivBEq α] [LawfulHashable α] {k k': α} {f : Option β → Option β}
     (h : k == k') : k' ∈ Const.alter m k f ↔ (f (Const.get? m k)).isSome :=
   m.inductionOn (fun _ h => DHashMap.Const.mem_alter_of_beq h) h
 
 @[simp]
-theorem contains_alter_self {k : α} {f : Option β → Option β} :
+theorem contains_alter_self [EquivBEq α] [LawfulHashable α] {k : α} {f : Option β → Option β} :
     (Const.alter m k f).contains k = (f (Const.get? m k)).isSome :=
   m.inductionOn fun _ => DHashMap.Const.contains_alter_self
 
 @[simp]
-theorem mem_alter_self {k : α} {f : Option β → Option β} :
+theorem mem_alter_self [EquivBEq α] [LawfulHashable α] {k : α} {f : Option β → Option β} :
     k ∈ Const.alter m k f ↔ (f (Const.get? m k)).isSome :=
   m.inductionOn fun _ => DHashMap.Const.mem_alter_self
 
-theorem contains_alter_of_beq_eq_false {k k' : α}
+theorem contains_alter_of_beq_eq_false [EquivBEq α] [LawfulHashable α] {k k' : α}
     {f : Option β → Option β} (h : (k == k') = false) :
     (Const.alter m k f).contains k' = m.contains k' :=
   m.inductionOn (fun _ h => DHashMap.Const.contains_alter_of_beq_eq_false h) h
 
-theorem mem_alter_of_beq_eq_false {k k' : α}
+theorem mem_alter_of_beq_eq_false [EquivBEq α] [LawfulHashable α] {k k' : α}
     {f : Option β → Option β} (h : (k == k') = false) : k' ∈ Const.alter m k f ↔ k' ∈ m :=
   m.inductionOn (fun _ h => DHashMap.Const.mem_alter_of_beq_eq_false h) h
 
-theorem size_alter {k : α} {f : Option β → Option β} :
+theorem size_alter [EquivBEq α] [LawfulHashable α] {k : α} {f : Option β → Option β} :
     (Const.alter m k f).size =
       if k ∈ m ∧ (f (Const.get? m k)).isNone then
         m.size - 1
@@ -2342,33 +2287,33 @@ theorem size_alter {k : α} {f : Option β → Option β} :
         m.size :=
   m.inductionOn fun _ => DHashMap.Const.size_alter
 
-theorem size_alter_eq_add_one {k : α} {f : Option β → Option β}
+theorem size_alter_eq_add_one [EquivBEq α] [LawfulHashable α] {k : α} {f : Option β → Option β}
     (h : k ∉ m) (h' : (f (Const.get? m k)).isSome) :
     (Const.alter m k f).size = m.size + 1 :=
   m.inductionOn (fun _ h h' => DHashMap.Const.size_alter_eq_add_one h h') h h'
 
-theorem size_alter_eq_sub_one {k : α} {f : Option β → Option β}
+theorem size_alter_eq_sub_one [EquivBEq α] [LawfulHashable α] {k : α} {f : Option β → Option β}
     (h : k ∈ m) (h' : (f (Const.get? m k)).isNone) :
     (Const.alter m k f).size = m.size - 1 :=
   m.inductionOn (fun _ h h' => DHashMap.Const.size_alter_eq_sub_one h h') h h'
 
-theorem size_alter_eq_self_of_not_mem {k : α} {f : Option β → Option β}
+theorem size_alter_eq_self_of_not_mem [EquivBEq α] [LawfulHashable α] {k : α} {f : Option β → Option β}
     (h : k ∉ m) (h' : (f (Const.get? m k)).isNone) : (Const.alter m k f).size = m.size :=
   m.inductionOn (fun _ h h' => DHashMap.Const.size_alter_eq_self_of_not_mem h h') h h'
 
-theorem size_alter_eq_self_of_mem {k : α} {f : Option β → Option β}
+theorem size_alter_eq_self_of_mem [EquivBEq α] [LawfulHashable α] {k : α} {f : Option β → Option β}
     (h : k ∈ m) (h' : (f (Const.get? m k)).isSome) : (Const.alter m k f).size = m.size :=
   m.inductionOn (fun _ h h' => DHashMap.Const.size_alter_eq_self_of_mem h h') h h'
 
-theorem size_alter_le_size {k : α} {f : Option β → Option β} :
+theorem size_alter_le_size [EquivBEq α] [LawfulHashable α] {k : α} {f : Option β → Option β} :
     (Const.alter m k f).size ≤ m.size + 1 :=
   m.inductionOn fun _ => DHashMap.Const.size_alter_le_size
 
-theorem size_le_size_alter {k : α} {f : Option β → Option β} :
+theorem size_le_size_alter [EquivBEq α] [LawfulHashable α] {k : α} {f : Option β → Option β} :
     m.size - 1 ≤ (Const.alter m k f).size :=
   m.inductionOn fun _ => DHashMap.Const.size_le_size_alter
 
-theorem get?_alter {k k' : α} {f : Option β → Option β} :
+theorem get?_alter [EquivBEq α] [LawfulHashable α] {k k' : α} {f : Option β → Option β} :
     Const.get? (Const.alter m k f) k' =
       if k == k' then
         f (Const.get? m k)
@@ -2377,11 +2322,11 @@ theorem get?_alter {k k' : α} {f : Option β → Option β} :
   m.inductionOn fun _ => DHashMap.Const.get?_alter
 
 @[simp]
-theorem get?_alter_self {k : α} {f : Option β → Option β} :
+theorem get?_alter_self [EquivBEq α] [LawfulHashable α] {k : α} {f : Option β → Option β} :
     Const.get? (Const.alter m k f) k = f (Const.get? m k) :=
   m.inductionOn fun _ => DHashMap.Const.get?_alter_self
 
-theorem get_alter {k k' : α} {f : Option β → Option β}
+theorem get_alter [EquivBEq α] [LawfulHashable α] {k k' : α} {f : Option β → Option β}
     {h : k' ∈ Const.alter m k f} :
     Const.get (Const.alter m k f) k' h =
       if heq : k == k' then
@@ -2393,13 +2338,13 @@ theorem get_alter {k k' : α} {f : Option β → Option β}
   m.inductionOn (fun _ _ => DHashMap.Const.get_alter) h
 
 @[simp]
-theorem get_alter_self {k : α} {f : Option β → Option β}
+theorem get_alter_self [EquivBEq α] [LawfulHashable α] {k : α} {f : Option β → Option β}
     {h : k ∈ Const.alter m k f} :
     haveI h' : (f (Const.get? m k)).isSome := mem_alter_self.mp h
     Const.get (Const.alter m k f) k h = (f (Const.get? m k)).get h' :=
   m.inductionOn (fun _ _ => DHashMap.Const.get_alter_self) h
 
-theorem get!_alter {k k' : α} [Inhabited β]
+theorem get!_alter [EquivBEq α] [LawfulHashable α] {k k' : α} [Inhabited β]
     {f : Option β → Option β} : Const.get! (Const.alter m k f) k' =
       if k == k' then
         f (Const.get? m k) |>.get!
@@ -2408,11 +2353,11 @@ theorem get!_alter {k k' : α} [Inhabited β]
   m.inductionOn fun _ => DHashMap.Const.get!_alter
 
 @[simp]
-theorem get!_alter_self {k : α} [Inhabited β]
+theorem get!_alter_self [EquivBEq α] [LawfulHashable α] {k : α} [Inhabited β]
     {f : Option β → Option β} : Const.get! (Const.alter m k f) k = (f (Const.get? m k)).get! :=
   m.inductionOn fun _ => DHashMap.Const.get!_alter_self
 
-theorem getD_alter {k k' : α} {fallback : β}
+theorem getD_alter [EquivBEq α] [LawfulHashable α] {k k' : α} {fallback : β}
     {f : Option β → Option β} :
     Const.getD (Const.alter m k f) k' fallback =
       if k == k' then
@@ -2422,12 +2367,12 @@ theorem getD_alter {k k' : α} {fallback : β}
   m.inductionOn fun _ => DHashMap.Const.getD_alter
 
 @[simp]
-theorem getD_alter_self {k : α} {fallback : β}
+theorem getD_alter_self [EquivBEq α] [LawfulHashable α] {k : α} {fallback : β}
     {f : Option β → Option β} :
     Const.getD (Const.alter m k f) k fallback = (f (Const.get? m k)).getD fallback :=
   m.inductionOn fun _ => DHashMap.Const.getD_alter_self
 
-theorem getKey?_alter {k k' : α} {f : Option β → Option β} :
+theorem getKey?_alter [EquivBEq α] [LawfulHashable α] {k k' : α} {f : Option β → Option β} :
     (Const.alter m k f).getKey? k' =
       if k == k' then
         if (f (Const.get? m k)).isSome then some k else none
@@ -2435,11 +2380,11 @@ theorem getKey?_alter {k k' : α} {f : Option β → Option β} :
         m.getKey? k' :=
   m.inductionOn fun _ => DHashMap.Const.getKey?_alter
 
-theorem getKey?_alter_self {k : α} {f : Option β → Option β} :
+theorem getKey?_alter_self [EquivBEq α] [LawfulHashable α] {k : α} {f : Option β → Option β} :
     (Const.alter m k f).getKey? k = if (f (Const.get? m k)).isSome then some k else none :=
   m.inductionOn fun _ => DHashMap.Const.getKey?_alter_self
 
-theorem getKey!_alter [Inhabited α] {k k' : α}
+theorem getKey!_alter [EquivBEq α] [LawfulHashable α] [Inhabited α] {k k' : α}
     {f : Option β → Option β} : (Const.alter m k f).getKey! k' =
       if k == k' then
         if (f (Const.get? m k)).isSome then k else default
@@ -2447,12 +2392,12 @@ theorem getKey!_alter [Inhabited α] {k k' : α}
         m.getKey! k' :=
   m.inductionOn fun _ => DHashMap.Const.getKey!_alter
 
-theorem getKey!_alter_self [Inhabited α] {k : α}
+theorem getKey!_alter_self [EquivBEq α] [LawfulHashable α] [Inhabited α] {k : α}
     {f : Option β → Option β} :
     (Const.alter m k f).getKey! k = if (f (Const.get? m k)).isSome then k else default :=
   m.inductionOn fun _ => DHashMap.Const.getKey!_alter_self
 
-theorem getKey_alter [Inhabited α] {k k' : α}
+theorem getKey_alter [EquivBEq α] [LawfulHashable α] [Inhabited α] {k k' : α}
     {f : Option β → Option β} {h : k' ∈ Const.alter m k f} :
     (Const.alter m k f).getKey k' h =
       if heq : k == k' then
@@ -2463,12 +2408,12 @@ theorem getKey_alter [Inhabited α] {k k' : α}
   m.inductionOn (fun _ _ => DHashMap.Const.getKey_alter) h
 
 @[simp]
-theorem getKey_alter_self [Inhabited α] {k : α}
+theorem getKey_alter_self [EquivBEq α] [LawfulHashable α] [Inhabited α] {k : α}
     {f : Option β → Option β} {h : k ∈ Const.alter m k f} :
     (Const.alter m k f).getKey k h = k :=
   m.inductionOn (fun _ _ => DHashMap.Const.getKey_alter_self) h
 
-theorem getKeyD_alter {k k' fallback : α} {f : Option β → Option β} :
+theorem getKeyD_alter [EquivBEq α] [LawfulHashable α] {k k' fallback : α} {f : Option β → Option β} :
     (Const.alter m k f).getKeyD k' fallback =
       if k == k' then
         if (f (Const.get? m k)).isSome then k else fallback
@@ -2476,7 +2421,7 @@ theorem getKeyD_alter {k k' fallback : α} {f : Option β → Option β} :
         m.getKeyD k' fallback :=
   m.inductionOn fun _ => DHashMap.Const.getKeyD_alter
 
-theorem getKeyD_alter_self [Inhabited α] {k fallback : α}
+theorem getKeyD_alter_self [EquivBEq α] [LawfulHashable α] [Inhabited α] {k fallback : α}
     {f : Option β → Option β} :
     (Const.alter m k f).getKeyD k fallback =
       if (f (Const.get? m k)).isSome then k else fallback :=
@@ -2618,27 +2563,27 @@ namespace Const
 variable {β : Type v} {m : ExtDHashMap α (fun _ => β)}
 
 @[simp]
-theorem modify_eq_empty_iff {k : α} {f : β → β} :
+theorem modify_eq_empty_iff [EquivBEq α] [LawfulHashable α] {k : α} {f : β → β} :
     Const.modify m k f = ∅ ↔ m = ∅ := by
   simp only [← isEmpty_iff, Bool.coe_iff_coe]
   exact m.inductionOn fun _ => DHashMap.Const.isEmpty_modify
 
 @[simp]
-theorem contains_modify {k k': α} {f : β → β} :
+theorem contains_modify [EquivBEq α] [LawfulHashable α] {k k': α} {f : β → β} :
     (Const.modify m k f).contains k' = m.contains k' :=
   m.inductionOn fun _ => DHashMap.Const.contains_modify
 
 @[simp]
-theorem mem_modify {k k': α} {f : β → β} :
+theorem mem_modify [EquivBEq α] [LawfulHashable α] {k k': α} {f : β → β} :
     k' ∈ Const.modify m k f ↔ k' ∈ m :=
   m.inductionOn fun _ => DHashMap.Const.mem_modify
 
 @[simp]
-theorem size_modify {k : α} {f : β → β} :
+theorem size_modify [EquivBEq α] [LawfulHashable α] {k : α} {f : β → β} :
     (Const.modify m k f).size = m.size :=
   m.inductionOn fun _ => DHashMap.Const.size_modify
 
-theorem get?_modify {k k' : α} {f : β → β} :
+theorem get?_modify [EquivBEq α] [LawfulHashable α] {k k' : α} {f : β → β} :
     Const.get? (Const.modify m k f) k' = if k == k' then
       Const.get? m k |>.map f
     else
@@ -2646,11 +2591,11 @@ theorem get?_modify {k k' : α} {f : β → β} :
   m.inductionOn fun _ => DHashMap.Const.get?_modify
 
 @[simp]
-theorem get?_modify_self {k : α} {f : β → β} :
+theorem get?_modify_self [EquivBEq α] [LawfulHashable α] {k : α} {f : β → β} :
     Const.get? (Const.modify m k f) k = (Const.get? m k).map f :=
   m.inductionOn fun _ => DHashMap.Const.get?_modify_self
 
-theorem get_modify {k k' : α} {f : β → β}
+theorem get_modify [EquivBEq α] [LawfulHashable α] {k k' : α} {f : β → β}
     {h : k' ∈ Const.modify m k f} :
     Const.get (Const.modify m k f) k' h =
       if heq : k == k' then
@@ -2662,13 +2607,13 @@ theorem get_modify {k k' : α} {f : β → β}
   m.inductionOn (fun _ _ => DHashMap.Const.get_modify) h
 
 @[simp]
-theorem get_modify_self {k : α} {f : β → β}
+theorem get_modify_self [EquivBEq α] [LawfulHashable α] {k : α} {f : β → β}
     {h : k ∈ Const.modify m k f} :
     haveI h' : k ∈ m := mem_modify.mp h
     Const.get (Const.modify m k f) k h = f (Const.get m k h') :=
   m.inductionOn (fun _ _ => DHashMap.Const.get_modify_self) h
 
-theorem get!_modify {k k' : α} [Inhabited β] {f : β → β} :
+theorem get!_modify [EquivBEq α] [LawfulHashable α] {k k' : α} [Inhabited β] {f : β → β} :
     Const.get! (Const.modify m k f) k' =
       if k == k' then
         Const.get? m k |>.map f |>.get!
@@ -2677,11 +2622,11 @@ theorem get!_modify {k k' : α} [Inhabited β] {f : β → β} :
   m.inductionOn fun _ => DHashMap.Const.get!_modify
 
 @[simp]
-theorem get!_modify_self {k : α} [Inhabited β] {f : β → β} :
+theorem get!_modify_self [EquivBEq α] [LawfulHashable α] {k : α} [Inhabited β] {f : β → β} :
     Const.get! (Const.modify m k f) k = ((Const.get? m k).map f).get! :=
   m.inductionOn fun _ => DHashMap.Const.get!_modify_self
 
-theorem getD_modify {k k' : α} {fallback : β} {f : β → β} :
+theorem getD_modify [EquivBEq α] [LawfulHashable α] {k k' : α} {fallback : β} {f : β → β} :
     Const.getD (Const.modify m k f) k' fallback =
       if k == k' then
         Const.get? m k |>.map f |>.getD fallback
@@ -2690,11 +2635,11 @@ theorem getD_modify {k k' : α} {fallback : β} {f : β → β} :
   m.inductionOn fun _ => DHashMap.Const.getD_modify
 
 @[simp]
-theorem getD_modify_self {k : α} {fallback : β} {f : β → β} :
+theorem getD_modify_self [EquivBEq α] [LawfulHashable α] {k : α} {fallback : β} {f : β → β} :
     Const.getD (Const.modify m k f) k fallback = ((Const.get? m k).map f).getD fallback :=
   m.inductionOn fun _ => DHashMap.Const.getD_modify_self
 
-theorem getKey?_modify {k k' : α} {f : β → β} :
+theorem getKey?_modify [EquivBEq α] [LawfulHashable α] {k k' : α} {f : β → β} :
     (Const.modify m k f).getKey? k' =
       if k == k' then
         if k ∈ m then some k else none
@@ -2702,11 +2647,11 @@ theorem getKey?_modify {k k' : α} {f : β → β} :
         m.getKey? k' :=
   m.inductionOn fun _ => DHashMap.Const.getKey?_modify
 
-theorem getKey?_modify_self {k : α} {f : β → β} :
+theorem getKey?_modify_self [EquivBEq α] [LawfulHashable α] {k : α} {f : β → β} :
     (Const.modify m k f).getKey? k = if k ∈ m then some k else none :=
   m.inductionOn fun _ => DHashMap.Const.getKey?_modify_self
 
-theorem getKey!_modify [Inhabited α] {k k' : α} {f : β → β} :
+theorem getKey!_modify [EquivBEq α] [LawfulHashable α] [Inhabited α] {k k' : α} {f : β → β} :
     (Const.modify m k f).getKey! k' =
       if k == k' then
         if k ∈ m then k else default
@@ -2714,11 +2659,11 @@ theorem getKey!_modify [Inhabited α] {k k' : α} {f : β → β} :
         m.getKey! k' :=
   m.inductionOn fun _ => DHashMap.Const.getKey!_modify
 
-theorem getKey!_modify_self [Inhabited α] {k : α} {f : β → β} :
+theorem getKey!_modify_self [EquivBEq α] [LawfulHashable α] [Inhabited α] {k : α} {f : β → β} :
     (Const.modify m k f).getKey! k = if k ∈ m then k else default :=
   m.inductionOn fun _ => DHashMap.Const.getKey!_modify_self
 
-theorem getKey_modify [Inhabited α] {k k' : α} {f : β → β}
+theorem getKey_modify [EquivBEq α] [LawfulHashable α] [Inhabited α] {k k' : α} {f : β → β}
     {h : k' ∈ Const.modify m k f} :
     (Const.modify m k f).getKey k' h =
       if k == k' then
@@ -2729,11 +2674,11 @@ theorem getKey_modify [Inhabited α] {k k' : α} {f : β → β}
   m.inductionOn (fun _ _ => DHashMap.Const.getKey_modify) h
 
 @[simp]
-theorem getKey_modify_self [Inhabited α] {k : α} {f : β → β}
+theorem getKey_modify_self [EquivBEq α] [LawfulHashable α] [Inhabited α] {k : α} {f : β → β}
     {h : k ∈ Const.modify m k f} : (Const.modify m k f).getKey k h = k :=
   m.inductionOn (fun _ _ => DHashMap.Const.getKey_modify_self) h
 
-theorem getKeyD_modify {k k' fallback : α} {f : β → β} :
+theorem getKeyD_modify [EquivBEq α] [LawfulHashable α] {k k' fallback : α} {f : β → β} :
     (Const.modify m k f).getKeyD k' fallback =
       if k == k' then
         if k ∈ m then k else fallback
@@ -2741,7 +2686,7 @@ theorem getKeyD_modify {k k' fallback : α} {f : β → β} :
         m.getKeyD k' fallback :=
   m.inductionOn fun _ => DHashMap.Const.getKeyD_modify
 
-theorem getKeyD_modify_self [Inhabited α] {k fallback : α} {f : β → β} :
+theorem getKeyD_modify_self [EquivBEq α] [LawfulHashable α] [Inhabited α] {k fallback : α} {f : β → β} :
     (Const.modify m k f).getKeyD k fallback = if k ∈ m then k else fallback :=
   m.inductionOn fun _ => DHashMap.Const.getKeyD_modify_self
 
@@ -2760,12 +2705,12 @@ namespace Const
 
 variable {β : Type v} {m₁ m₂ : ExtDHashMap α fun _ => β}
 
-theorem ext_getKey?_get? (hk : ∀ k, m₁.getKey? k = m₂.getKey? k)
+theorem ext_getKey?_get? [EquivBEq α] [LawfulHashable α] (hk : ∀ k, m₁.getKey? k = m₂.getKey? k)
     (hv : ∀ k, Const.get? m₁ k = Const.get? m₂ k) : m₁ = m₂ :=
   m₁.inductionOn₂ m₂ (fun _ _ hk hv => Quotient.sound
     (.of_forall_getKey?_eq_of_forall_constGet?_eq hk hv)) hk hv
 
-theorem ext_getKey?_unit {m₁ m₂ : ExtDHashMap α fun _ => Unit}
+theorem ext_getKey?_unit [EquivBEq α] [LawfulHashable α] {m₁ m₂ : ExtDHashMap α fun _ => Unit}
     (h : ∀ k, m₁.getKey? k = m₂.getKey? k) : m₁ = m₂ :=
   m₁.inductionOn₂ m₂ (fun _ _ h => Quotient.sound (.of_forall_getKey?_unit_eq h)) h
 
@@ -2800,17 +2745,17 @@ theorem mem_filterMap [LawfulBEq α]
     k ∈ m.filterMap f ↔ ∃ h, (f k (m.get k h)).isSome :=
   m.inductionOn fun _ => DHashMap.mem_filterMap
 
-theorem contains_of_contains_filterMap
+theorem contains_of_contains_filterMap [EquivBEq α] [LawfulHashable α]
     {f : (a : α) → β a → Option (γ a)} {k : α} :
     (m.filterMap f).contains k = true → m.contains k = true :=
   m.inductionOn fun _ => DHashMap.contains_of_contains_filterMap
 
-theorem mem_of_mem_filterMap
+theorem mem_of_mem_filterMap [EquivBEq α] [LawfulHashable α]
     {f : (a : α) → β a → Option (γ a)} {k : α} :
     k ∈ m.filterMap f → k ∈ m :=
   m.inductionOn fun _ => DHashMap.mem_of_mem_filterMap
 
-theorem size_filterMap_le_size
+theorem size_filterMap_le_size [EquivBEq α] [LawfulHashable α]
     {f : (a : α) → β a → Option (γ a)} :
     (m.filterMap f).size ≤ m.size :=
   m.inductionOn fun _ => DHashMap.size_filterMap_le_size
@@ -2858,7 +2803,7 @@ theorem getKey?_filterMap [LawfulBEq α]
   m.inductionOn fun _ => DHashMap.getKey?_filterMap
 
 @[simp]
-theorem getKey_filterMap
+theorem getKey_filterMap [EquivBEq α] [LawfulHashable α]
     {f : (a : α) → β a → Option (γ a)} {k : α} {h'} :
     (m.filterMap f).getKey k h' = m.getKey k (mem_of_mem_filterMap h') :=
   m.inductionOn (fun _ _ => DHashMap.getKey_filterMap) h'
@@ -2881,32 +2826,32 @@ namespace Const
 
 variable {β : Type v} {γ : Type w} {m : ExtDHashMap α (fun _ => β)}
 
-theorem filterMap_eq_empty_iff {f : α → β → Option γ} :
+theorem filterMap_eq_empty_iff [EquivBEq α] [LawfulHashable α] {f : α → β → Option γ} :
     m.filterMap f = ∅ ↔ ∀ k h, f (m.getKey k h) (get m k h) = none :=
   isEmpty_iff.symm.trans <| m.inductionOn fun _ => DHashMap.Const.isEmpty_filterMap_iff
 
-theorem mem_filterMap
+theorem mem_filterMap [EquivBEq α] [LawfulHashable α]
     {f : α → β → Option γ} {k : α} :
     k ∈ m.filterMap f ↔ ∃ h, (f (m.getKey k h) (Const.get m k h)).isSome :=
   m.inductionOn fun _ => DHashMap.Const.mem_filterMap
 
-theorem size_filterMap_eq_size_iff
+theorem size_filterMap_eq_size_iff [EquivBEq α] [LawfulHashable α]
     {f : α → β → Option γ} :
     (m.filterMap f).size = m.size ↔ ∀ k h, (f (m.getKey k h) (Const.get m k h)).isSome :=
   m.inductionOn fun _ => DHashMap.Const.size_filterMap_eq_size_iff
 
-theorem get?_filterMap
+theorem get?_filterMap [EquivBEq α] [LawfulHashable α]
     {f : α → β → Option γ} {k : α} :
     Const.get? (m.filterMap f) k = (Const.get? m k).pbind (fun x h' =>
       f (m.getKey k (mem_iff_isSome_get?.mpr (Option.isSome_of_eq_some h'))) x) :=
   m.inductionOn fun _ => DHashMap.Const.get?_filterMap
 
-theorem get?_filterMap_of_getKey?_eq_some
+theorem get?_filterMap_of_getKey?_eq_some [EquivBEq α] [LawfulHashable α]
     {f : α → β → Option γ} {k k' : α} (h : m.getKey? k = some k') :
     Const.get? (m.filterMap f) k = (Const.get? m k).bind (f k') :=
   m.inductionOn (fun _ h => DHashMap.Const.get?_filterMap_of_getKey?_eq_some h) h
 
-theorem isSome_apply_of_mem_filterMap
+theorem isSome_apply_of_mem_filterMap [EquivBEq α] [LawfulHashable α]
     {f : α → β → Option γ} {k : α} :
     ∀ (h : k ∈ m.filterMap f),
       (f (m.getKey k (mem_of_mem_filterMap h))
@@ -2914,7 +2859,7 @@ theorem isSome_apply_of_mem_filterMap
   m.inductionOn fun _ => DHashMap.Const.isSome_apply_of_mem_filterMap
 
 @[simp]
-theorem get_filterMap
+theorem get_filterMap [EquivBEq α] [LawfulHashable α]
     {f : α → β → Option γ} {k : α} {h} :
     Const.get (m.filterMap f) k h =
       (f (m.getKey k (mem_of_mem_filterMap h))
@@ -2922,45 +2867,45 @@ theorem get_filterMap
           (isSome_apply_of_mem_filterMap h) :=
   m.inductionOn (fun _ _ => DHashMap.Const.get_filterMap) h
 
-theorem get!_filterMap [Inhabited γ]
+theorem get!_filterMap [EquivBEq α] [LawfulHashable α] [Inhabited γ]
     {f : α → β → Option γ} {k : α} :
     Const.get! (m.filterMap f) k =
       ((Const.get? m k).pbind (fun x h' =>
         f (m.getKey k (mem_iff_isSome_get?.mpr (Option.isSome_of_eq_some h'))) x)).get! :=
   m.inductionOn fun _ => DHashMap.Const.get!_filterMap
 
-theorem get!_filterMap_of_getKey?_eq_some [Inhabited γ]
+theorem get!_filterMap_of_getKey?_eq_some [EquivBEq α] [LawfulHashable α] [Inhabited γ]
     {f : α → β → Option γ} {k k' : α} (h : m.getKey? k = some k') :
     Const.get! (m.filterMap f) k = ((Const.get? m k).bind (f k')).get! :=
   m.inductionOn (fun _ h => DHashMap.Const.get!_filterMap_of_getKey?_eq_some h) h
 
-theorem getD_filterMap
+theorem getD_filterMap [EquivBEq α] [LawfulHashable α]
     {f : α → β → Option γ} {k : α} {fallback : γ} :
     Const.getD (m.filterMap f) k fallback =
       ((Const.get? m k).pbind (fun x h' =>
       f (m.getKey k (mem_iff_isSome_get?.mpr (Option.isSome_of_eq_some h'))) x)).getD fallback :=
   m.inductionOn fun _ => DHashMap.Const.getD_filterMap
 
-theorem getD_filterMap_of_getKey?_eq_some
+theorem getD_filterMap_of_getKey?_eq_some [EquivBEq α] [LawfulHashable α]
     {f : α → β → Option γ} {k k' : α} {fallback : γ} (h : m.getKey? k = some k') :
     Const.getD (m.filterMap f) k fallback = ((Const.get? m k).bind (f k')).getD fallback :=
   m.inductionOn (fun _ h => DHashMap.Const.getD_filterMap_of_getKey?_eq_some h) h
 
-theorem getKey?_filterMap
+theorem getKey?_filterMap [EquivBEq α] [LawfulHashable α]
     {f : α → β → Option γ} {k : α} :
     (m.filterMap f).getKey? k =
     (m.getKey? k).pfilter (fun x h' =>
       (f x (Const.get m x (mem_of_getKey?_eq_some h'))).isSome) :=
   m.inductionOn fun _ => DHashMap.Const.getKey?_filterMap
 
-theorem getKey!_filterMap [Inhabited α]
+theorem getKey!_filterMap [EquivBEq α] [LawfulHashable α] [Inhabited α]
     {f : α → β → Option γ} {k : α} :
     (m.filterMap f).getKey! k =
     ((m.getKey? k).pfilter (fun x h' =>
       (f x (Const.get m x (mem_of_getKey?_eq_some h'))).isSome)).get! :=
   m.inductionOn fun _ => DHashMap.Const.getKey!_filterMap
 
-theorem getKeyD_filterMap
+theorem getKeyD_filterMap [EquivBEq α] [LawfulHashable α]
     {f : α → β → Option γ} {k fallback : α} :
     (m.filterMap f).getKeyD k fallback =
     ((m.getKey? k).pfilter (fun x h' =>
@@ -2973,7 +2918,7 @@ end filterMap
 
 section filter
 
-theorem filterMap_eq_filter {f : (a : α) → β a → Bool} :
+theorem filterMap_eq_filter [EquivBEq α] [LawfulHashable α] {f : (a : α) → β a → Bool} :
     m.filterMap (fun k => Option.guard (fun v => f k v)) = m.filter f :=
   m.inductionOn fun _ => Quotient.sound DHashMap.filterMap_equiv_filter
 
@@ -2983,7 +2928,7 @@ theorem filter_eq_empty_iff [LawfulBEq α]
     m.filter f = ∅ ↔ ∀ k h, f k (m.get k h) = false :=
   isEmpty_iff.symm.trans <| m.inductionOn fun _ => DHashMap.isEmpty_filter_iff
 
-theorem filter_key_eq_empty_iff {f : α → Bool} :
+theorem filter_key_eq_empty_iff [EquivBEq α] [LawfulHashable α] {f : α → Bool} :
     m.filter (fun a _ => f a) = ∅ ↔ ∀ k h, f (m.getKey k h) = false :=
   isEmpty_iff.symm.trans <| m.inductionOn fun _ => DHashMap.isEmpty_filter_key_iff
 
@@ -2995,19 +2940,19 @@ theorem mem_filter [LawfulBEq α] {f : (a : α) → β a → Bool} {k : α} :
     k ∈ m.filter f ↔ ∃ h, f k (m.get k h) :=
   m.inductionOn fun _ => DHashMap.mem_filter
 
-theorem mem_filter_key {f : α → Bool} {k : α} :
+theorem mem_filter_key [EquivBEq α] [LawfulHashable α] {f : α → Bool} {k : α} :
     k ∈ m.filter (fun a _ => f a) ↔ ∃ h, f (m.getKey k h) :=
   m.inductionOn fun _ => DHashMap.mem_filter_key
 
-theorem contains_of_contains_filter {f : (a : α) → β a → Bool} {k : α} :
+theorem contains_of_contains_filter [EquivBEq α] [LawfulHashable α] {f : (a : α) → β a → Bool} {k : α} :
     (m.filter f).contains k = true → m.contains k = true :=
   m.inductionOn fun _ => DHashMap.contains_of_contains_filter
 
-theorem mem_of_mem_filter {f : (a : α) → β a → Bool} {k : α} :
+theorem mem_of_mem_filter [EquivBEq α] [LawfulHashable α] {f : (a : α) → β a → Bool} {k : α} :
     k ∈ (m.filter f) → k ∈ m :=
   m.inductionOn fun _ => DHashMap.mem_of_mem_filter
 
-theorem size_filter_le_size {f : (a : α) → β a → Bool} :
+theorem size_filter_le_size [EquivBEq α] [LawfulHashable α] {f : (a : α) → β a → Bool} :
     (m.filter f).size ≤ m.size :=
   m.inductionOn fun _ => DHashMap.size_filter_le_size
 
@@ -3019,11 +2964,11 @@ theorem filter_eq_self_iff [LawfulBEq α] {f : (a : α) → β a → Bool} :
     m.filter f = m ↔ ∀ k h, f k (m.get k h) :=
   m.inductionOn fun _ => Iff.trans ⟨Quotient.exact, Quotient.sound⟩ DHashMap.filter_equiv_self_iff
 
-theorem filter_key_equiv_self_iff {f : (a : α) → Bool} :
+theorem filter_key_equiv_self_iff [EquivBEq α] [LawfulHashable α] {f : (a : α) → Bool} :
     m.filter (fun k _ => f k) = m ↔ ∀ k h, f (m.getKey k h) :=
   m.inductionOn fun _ => Iff.trans ⟨Quotient.exact, Quotient.sound⟩ DHashMap.filter_key_equiv_self_iff
 
-theorem size_filter_key_eq_size_iff {f : α → Bool} :
+theorem size_filter_key_eq_size_iff [EquivBEq α] [LawfulHashable α] {f : α → Bool} :
     (m.filter fun k _ => f k).size = m.size ↔ ∀ k h, f (m.getKey k h) :=
   m.inductionOn fun _ => DHashMap.size_filter_key_eq_size_iff
 
@@ -3056,13 +3001,13 @@ theorem getKey?_filter [LawfulBEq α]
       f x (m.get x (mem_of_getKey?_eq_some h'))) :=
   m.inductionOn fun _ => DHashMap.getKey?_filter
 
-theorem getKey?_filter_key
+theorem getKey?_filter_key [EquivBEq α] [LawfulHashable α]
     {f : α → Bool} {k : α} :
     (m.filter fun k _ => f k).getKey? k = (m.getKey? k).filter f :=
   m.inductionOn fun _ => DHashMap.getKey?_filter_key
 
 @[simp]
-theorem getKey_filter
+theorem getKey_filter [EquivBEq α] [LawfulHashable α]
     {f : (a : α) → β a → Bool} {k : α} {h'} :
     (m.filter f).getKey k h' = m.getKey k (mem_of_mem_filter h') :=
   m.inductionOn (fun _ _ => DHashMap.getKey_filter) h'
@@ -3074,7 +3019,7 @@ theorem getKey!_filter [LawfulBEq α] [Inhabited α]
       f x (m.get x (mem_of_getKey?_eq_some h')))).get! :=
   m.inductionOn fun _ => DHashMap.getKey!_filter
 
-theorem getKey!_filter_key [Inhabited α]
+theorem getKey!_filter_key [EquivBEq α] [LawfulHashable α] [Inhabited α]
     {f : α → Bool} {k : α} :
     (m.filter fun k _ => f k).getKey! k = ((m.getKey? k).filter f).get! :=
   m.inductionOn fun _ => DHashMap.getKey!_filter_key
@@ -3086,7 +3031,7 @@ theorem getKeyD_filter [LawfulBEq α]
       f x (m.get x (mem_of_getKey?_eq_some h')))).getD fallback :=
   m.inductionOn fun _ => DHashMap.getKeyD_filter
 
-theorem getKeyD_filter_key
+theorem getKeyD_filter_key [EquivBEq α] [LawfulHashable α]
     {f : α → Bool} {k fallback : α} :
     (m.filter fun k _ => f k).getKeyD k fallback = ((m.getKey? k).filter f).getD fallback :=
   m.inductionOn fun _ => DHashMap.getKeyD_filter_key
@@ -3095,90 +3040,90 @@ namespace Const
 
 variable {β : Type v} {γ : Type w} {m : ExtDHashMap α (fun _ => β)}
 
-theorem filter_eq_empty_iff {f : α → β → Bool} :
+theorem filter_eq_empty_iff [EquivBEq α] [LawfulHashable α] {f : α → β → Bool} :
     m.filter f = ∅ ↔ ∀ k h, f (m.getKey k h) (Const.get m k h) = false :=
   isEmpty_iff.symm.trans <| m.inductionOn fun _ => DHashMap.Const.isEmpty_filter_iff
 
-theorem mem_filter
+theorem mem_filter [EquivBEq α] [LawfulHashable α]
     {f : α → β → Bool} {k : α} :
     k ∈ m.filter f ↔ ∃ (h' : k ∈ m),
       f (m.getKey k h') (Const.get m k h') :=
   m.inductionOn fun _ => DHashMap.Const.mem_filter
 
-theorem size_filter_le_size
+theorem size_filter_le_size [EquivBEq α] [LawfulHashable α]
     {f : α → β → Bool} :
     (m.filter f).size ≤ m.size :=
   m.inductionOn fun _ => DHashMap.Const.size_filter_le_size
 
-theorem size_filter_eq_size_iff
+theorem size_filter_eq_size_iff [EquivBEq α] [LawfulHashable α]
     {f : α → β → Bool} :
     (m.filter f).size = m.size ↔ ∀ (a : α) (h : a ∈ m),
       f (m.getKey a h) (Const.get m a h) :=
   m.inductionOn fun _ => DHashMap.Const.size_filter_eq_size_iff
 
-theorem filter_eq_self_iff {f : α → β → Bool} :
+theorem filter_eq_self_iff [EquivBEq α] [LawfulHashable α] {f : α → β → Bool} :
     m.filter f = m ↔ ∀ k h, f (m.getKey k h) (Const.get m k h) :=
   m.inductionOn fun _ => Iff.trans ⟨Quotient.exact, Quotient.sound⟩ DHashMap.Const.filter_equiv_self_iff
 
-theorem get?_filter
+theorem get?_filter [EquivBEq α] [LawfulHashable α]
     {f : α → β → Bool} {k : α} :
     Const.get? (m.filter f) k = (Const.get? m k).pfilter (fun x h' =>
       f (m.getKey k (mem_iff_isSome_get?.mpr (Option.isSome_of_eq_some h'))) x) :=
   m.inductionOn fun _ => DHashMap.Const.get?_filter
 
-theorem get?_filter_of_getKey?_eq_some
+theorem get?_filter_of_getKey?_eq_some [EquivBEq α] [LawfulHashable α]
     {f : α → β → Bool} {k k' : α} :
     m.getKey? k = some k' →
       Const.get? (m.filter f) k = (Const.get? m k).filter (fun x => f k' x) :=
   m.inductionOn fun _ => DHashMap.Const.get?_filter_of_getKey?_eq_some
 
 @[simp]
-theorem get_filter
+theorem get_filter [EquivBEq α] [LawfulHashable α]
     {f : α → β → Bool} {k : α} {h'} :
     Const.get (m.filter f) k h' = Const.get m k (mem_of_mem_filter h') :=
   m.inductionOn (fun _ _ => DHashMap.Const.get_filter) h'
 
-theorem get!_filter [Inhabited β]
+theorem get!_filter [EquivBEq α] [LawfulHashable α] [Inhabited β]
     {f : α → β → Bool} {k : α} :
     Const.get! (m.filter f) k =
       ((Const.get? m k).pfilter (fun x h' =>
       f (m.getKey k (mem_iff_isSome_get?.mpr (Option.isSome_of_eq_some h'))) x)).get! :=
   m.inductionOn fun _ => DHashMap.Const.get!_filter
 
-theorem get!_filter_of_getKey?_eq_some [Inhabited β]
+theorem get!_filter_of_getKey?_eq_some [EquivBEq α] [LawfulHashable α] [Inhabited β]
     {f : α → β → Bool} {k k' : α} :
     m.getKey? k = some k' →
       Const.get! (m.filter f) k = ((Const.get? m k).filter (fun x => f k' x)).get! :=
   m.inductionOn fun _ => DHashMap.Const.get!_filter_of_getKey?_eq_some
 
-theorem getD_filter
+theorem getD_filter [EquivBEq α] [LawfulHashable α]
     {f : α → β → Bool} {k : α} {fallback : β} :
     Const.getD (m.filter f) k fallback = ((Const.get? m k).pfilter (fun x h' =>
       f (m.getKey k (mem_iff_isSome_get?.mpr (Option.isSome_of_eq_some h'))) x)).getD fallback :=
   m.inductionOn fun _ => DHashMap.Const.getD_filter
 
-theorem getD_filter_of_getKey?_eq_some
+theorem getD_filter_of_getKey?_eq_some [EquivBEq α] [LawfulHashable α]
     {f : α → β → Bool} {k k' : α} {fallback : β} :
     m.getKey? k = some k' →
       Const.getD (m.filter f) k fallback =
         ((Const.get? m k).filter (fun x => f k' x)).getD fallback :=
   m.inductionOn fun _ => DHashMap.Const.getD_filter_of_getKey?_eq_some
 
-theorem getKey?_filter
+theorem getKey?_filter [EquivBEq α] [LawfulHashable α]
     {f : α → β → Bool} {k : α} :
     (m.filter f).getKey? k =
     (m.getKey? k).pfilter (fun x h' =>
       (f x (Const.get m x (mem_of_getKey?_eq_some h')))) :=
   m.inductionOn fun _ => DHashMap.Const.getKey?_filter
 
-theorem getKey!_filter [Inhabited α]
+theorem getKey!_filter [EquivBEq α] [LawfulHashable α] [Inhabited α]
     {f : α → β → Bool} {k : α} :
     (m.filter f).getKey! k =
     ((m.getKey? k).pfilter (fun x h' =>
       (f x (Const.get m x (mem_of_getKey?_eq_some h'))))).get! :=
   m.inductionOn fun _ => DHashMap.Const.getKey!_filter
 
-theorem getKeyD_filter
+theorem getKeyD_filter [EquivBEq α] [LawfulHashable α]
     {f : α → β → Bool} {k fallback : α} :
     (m.filter f).getKeyD k fallback =
     ((m.getKey? k).pfilter (fun x h' =>
@@ -3194,47 +3139,47 @@ section map
 variable {γ : α → Type w} {δ : α → Type w'}
 
 @[simp]
-theorem map_id_fun : m.map (fun _ v => v) = m :=
+theorem map_id_fun [EquivBEq α] [LawfulHashable α] : m.map (fun _ v => v) = m :=
   m.inductionOn fun _ => Quotient.sound DHashMap.map_id_equiv
 
 @[simp]
-theorem map_map {f : (a : α) → β a → γ a} {g : (a : α) → γ a → δ a} :
+theorem map_map [EquivBEq α] [LawfulHashable α] {f : (a : α) → β a → γ a} {g : (a : α) → γ a → δ a} :
     (m.map f).map g = m.map fun k v => g k (f k v) :=
   m.inductionOn fun _ => Quotient.sound DHashMap.map_map_equiv
 
-theorem filterMap_eq_map {f : (a : α) → β a → γ a} :
+theorem filterMap_eq_map [EquivBEq α] [LawfulHashable α] {f : (a : α) → β a → γ a} :
     (m.filterMap (fun k v => some (f k v))) = m.map f :=
   m.inductionOn fun _ => Quotient.sound DHashMap.filterMap_equiv_map
 
 @[simp]
-theorem map_eq_empty_iff {f : (a : α) → β a → γ a} :
+theorem map_eq_empty_iff [EquivBEq α] [LawfulHashable α] {f : (a : α) → β a → γ a} :
     m.map f = ∅ ↔ m = ∅ := by
   simp only [← isEmpty_iff, Bool.coe_iff_coe]
   exact m.inductionOn fun _ => DHashMap.isEmpty_map
 
-theorem contains_map
+theorem contains_map [EquivBEq α] [LawfulHashable α]
     {f : (a : α) → β a → γ a} {k : α} :
     (m.map f).contains k = m.contains k :=
   m.inductionOn fun _ => DHashMap.contains_map
 
-theorem contains_of_contains_map
+theorem contains_of_contains_map [EquivBEq α] [LawfulHashable α]
     {f : (a : α) → β a → γ a} {k : α} :
     (m.map f).contains k = true → m.contains k = true :=
   m.inductionOn fun _ => DHashMap.contains_of_contains_map
 
 @[simp]
-theorem mem_map
+theorem mem_map [EquivBEq α] [LawfulHashable α]
     {f : (a : α) → β a → γ a} {k : α} :
     k ∈ m.map f ↔ k ∈ m :=
   m.inductionOn fun _ => DHashMap.mem_map
 
-theorem mem_of_mem_map
+theorem mem_of_mem_map [EquivBEq α] [LawfulHashable α]
     {f : (a : α) → β a → γ a} {k : α} :
     k ∈ m.map f → k ∈ m :=
   m.inductionOn fun _ => DHashMap.mem_of_mem_map
 
 @[simp]
-theorem size_map
+theorem size_map [EquivBEq α] [LawfulHashable α]
     {f : (a : α) → β a → γ a} :
     (m.map f).size = m.size :=
   m.inductionOn fun _ => DHashMap.size_map
@@ -3262,25 +3207,25 @@ theorem getD_map [LawfulBEq α]
   m.inductionOn fun _ => DHashMap.getD_map
 
 @[simp]
-theorem getKey?_map
+theorem getKey?_map [EquivBEq α] [LawfulHashable α]
     {f : (a : α) → β a → γ a} {k : α} :
     (m.map f).getKey? k = m.getKey? k :=
   m.inductionOn fun _ => DHashMap.getKey?_map
 
 @[simp]
-theorem getKey_map
+theorem getKey_map [EquivBEq α] [LawfulHashable α]
     {f : (a : α) → β a → γ a} {k : α} {h'} :
     (m.map f).getKey k h' = m.getKey k (mem_of_mem_map h') :=
   m.inductionOn (fun _ _ => DHashMap.getKey_map) h'
 
 @[simp]
-theorem getKey!_map [Inhabited α]
+theorem getKey!_map [EquivBEq α] [LawfulHashable α] [Inhabited α]
     {f : (a : α) → β a → γ a} {k : α} :
     (m.map f).getKey! k = m.getKey! k :=
   m.inductionOn fun _ => DHashMap.getKey!_map
 
 @[simp]
-theorem getKeyD_map
+theorem getKeyD_map [EquivBEq α] [LawfulHashable α]
     {f : (a : α) → β a → γ a} {k fallback : α} :
     (m.map f).getKeyD k fallback = m.getKeyD k fallback :=
   m.inductionOn fun _ => DHashMap.getKeyD_map
@@ -3289,44 +3234,44 @@ namespace Const
 
 variable {β : Type v} {γ : Type w} {m : ExtDHashMap α fun _ => β}
 
-theorem get?_map
+theorem get?_map [EquivBEq α] [LawfulHashable α]
     {f : α → β → γ} {k : α} :
     Const.get? (m.map f) k = (Const.get? m k).pmap (fun v h' => f (m.getKey k h') v)
       (fun _ h' => mem_iff_isSome_get?.mpr (Option.isSome_of_eq_some h')) :=
   m.inductionOn fun _ => DHashMap.Const.get?_map
 
-theorem get?_map_of_getKey?_eq_some
+theorem get?_map_of_getKey?_eq_some [EquivBEq α] [LawfulHashable α]
     {f : α → β → γ} {k k' : α} (h : m.getKey? k = some k') :
     Const.get? (m.map f) k = (Const.get? m k).map (f k') :=
   m.inductionOn (fun _ h => DHashMap.Const.get?_map_of_getKey?_eq_some h) h
 
 @[simp]
-theorem get_map
+theorem get_map [EquivBEq α] [LawfulHashable α]
     {f : α → β → γ} {k : α} {h'} :
     Const.get (m.map f) k h' =
       f (m.getKey k (mem_of_mem_map h')) (Const.get m k (mem_of_mem_map h')) :=
   m.inductionOn (fun _ _ => DHashMap.Const.get_map) h'
 
-theorem get!_map [Inhabited γ]
+theorem get!_map [EquivBEq α] [LawfulHashable α] [Inhabited γ]
     {f : α → β → γ} {k : α} :
     Const.get! (m.map f) k =
       ((get? m k).pmap (fun v h => f (m.getKey k h) v)
         (fun _ h' => mem_iff_isSome_get?.mpr (Option.isSome_of_mem h'))).get! :=
   m.inductionOn fun _ => DHashMap.Const.get!_map
 
-theorem get!_map_of_getKey?_eq_some [Inhabited γ]
+theorem get!_map_of_getKey?_eq_some [EquivBEq α] [LawfulHashable α] [Inhabited γ]
     {f : α → β → γ} {k k' : α} (h : m.getKey? k = some k') :
     Const.get! (m.map f) k = ((Const.get? m k).map (f k')).get! :=
   m.inductionOn (fun _ h => DHashMap.Const.get!_map_of_getKey?_eq_some h) h
 
-theorem getD_map
+theorem getD_map [EquivBEq α] [LawfulHashable α]
     {f : α → β → γ} {k : α} {fallback : γ} :
     Const.getD (m.map f) k fallback =
       ((get? m k).pmap (fun v h => f (m.getKey k h) v)
         (fun _ h' => mem_iff_isSome_get?.mpr (Option.isSome_of_eq_some h'))).getD fallback :=
   m.inductionOn fun _ => DHashMap.Const.getD_map
 
-theorem getD_map_of_getKey?_eq_some [Inhabited γ]
+theorem getD_map_of_getKey?_eq_some [EquivBEq α] [LawfulHashable α] [Inhabited γ]
     {f : α → β → γ} {k k' : α} {fallback : γ} (h : m.getKey? k = some k') :
     Const.getD (m.map f) k fallback = ((Const.get? m k).map (f k')).getD fallback :=
   m.inductionOn (fun _ h => DHashMap.Const.getD_map_of_getKey?_eq_some h) h
